theories/examples/macros.v
@@ -1,19 +1,13 @@
 From iris.algebra Require Import frac.
 From iris.proofmode Require Import tactics.
 Require Import Eqdep_dec List.
-From cap_machine Require Import rules logrel monotone stack_macros_helpers.
-From cap_machine Require Export iris_extra addr_reg_sample region_macros contiguous malloc.
+From cap_machine Require Import rules logrel macros_helpers.
+From cap_machine Require Export iris_extra addr_reg_sample contiguous malloc.
 
-Section stack_macros.
+Section macros.
   Context {Σ:gFunctors} {memg:memG Σ} {regg:regG Σ}
-          {stsg : STSG Addr region_type Σ} {heapg : heapG Σ}
-          `{MonRef: MonRefG (leibnizO _) CapR_rtc Σ} {nainv: logrel_na_invs Σ}
+          {nainv: logrel_na_invs Σ}
           `{MP: MachineParameters}.
-
-  Notation STS := (leibnizO (STS_states * STS_rels)).
-  Notation STS_STD := (leibnizO (STS_std_states Addr region_type)).
-  Notation WORLD := (prodO STS_STD STS). 
-  Implicit Types W : WORLD.
   
 
   (* -------------------------------- LTACS ------------------------------------------- *)
@@ -63,36 +57,35 @@ Section stack_macros.
     move_z r_t3 0;
     load_r r_t1 r_t1]. 
 
-  Definition fetch f a p : iProp Σ :=
-    ([∗ list] a_i;w_i ∈ a;(fetch_instrs f), a_i ↦ₐ[p] w_i)%I. 
+  Definition fetch f a : iProp Σ :=
+    ([∗ list] a_i;w_i ∈ a;(fetch_instrs f), a_i ↦ₐ w_i)%I. 
 
   (* fetch spec *)
-  Lemma fetch_spec f a pc_p pc_p' pc_g pc_b pc_e a_first a_last b_link e_link a_link entry_a wentry φ w1 w2 w3:
-    isCorrectPC_range pc_p pc_g pc_b pc_e a_first a_last ->
-    PermFlows pc_p pc_p' ->
+  Lemma fetch_spec f a pc_p pc_b pc_e a_first a_last b_link e_link a_link entry_a wentry φ w1 w2 w3:
+    isCorrectPC_range pc_p pc_b pc_e a_first a_last ->
     contiguous_between a a_first a_last ->
-    withinBounds (RW, Global, b_link, e_link, entry_a) = true ->
+    withinBounds (RW, b_link, e_link, entry_a) = true ->
     (a_link + f)%a = Some entry_a ->
 
-      ▷ fetch f a pc_p'
-    ∗ ▷ PC ↦ᵣ inr (pc_p,pc_g,pc_b,pc_e,a_first)
-    ∗ ▷ pc_b ↦ₐ[pc_p'] inr (RO,Global,b_link,e_link,a_link)
-    ∗ ▷ entry_a ↦ₐ[RO] wentry
+      ▷ fetch f a 
+    ∗ ▷ PC ↦ᵣ inr (pc_p,pc_b,pc_e,a_first)
+    ∗ ▷ pc_b ↦ₐ inr (RO,b_link,e_link,a_link)
+    ∗ ▷ entry_a ↦ₐ wentry
     ∗ ▷ r_t1 ↦ᵣ w1
     ∗ ▷ r_t2 ↦ᵣ w2
     ∗ ▷ r_t3 ↦ᵣ w3
     (* if the capability is global, we want to be able to continue *)
     (* if w is not a global capability, we will fail, and must now show that Phi holds at failV *)
-    ∗ ▷ (PC ↦ᵣ inr (pc_p,pc_g,pc_b,pc_e,a_last) ∗ fetch f a pc_p'
+    ∗ ▷ (PC ↦ᵣ inr (pc_p,pc_b,pc_e,a_last) ∗ fetch f a 
             (* the newly allocated region *)
             ∗ r_t1 ↦ᵣ wentry ∗ r_t2 ↦ᵣ inl 0%Z ∗ r_t3 ↦ᵣ inl 0%Z
-            ∗ pc_b ↦ₐ[pc_p'] inr (RO,Global,b_link,e_link,a_link)
-            ∗ entry_a ↦ₐ[RO] wentry
+            ∗ pc_b ↦ₐ inr (RO,b_link,e_link,a_link)
+            ∗ entry_a ↦ₐ wentry
             -∗ WP Seq (Instr Executable) {{ φ }})
     ⊢
       WP Seq (Instr Executable) {{ φ }}.
   Proof.
-    iIntros (Hvpc Hfl Hcont Hwb Hentry) "(>Hprog & >HPC & >Hpc_b & >Ha_entry & >Hr_t1 & >Hr_t2 & >Hr_t3 & Hφ)".
+    iIntros (Hvpc Hcont Hwb Hentry) "(>Hprog & >HPC & >Hpc_b & >Ha_entry & >Hr_t1 & >Hr_t2 & >Hr_t3 & Hφ)".
     iDestruct (big_sepL2_length with "Hprog") as %Hlength.
     destruct a as [|a l];[inversion Hlength|].
     apply contiguous_between_cons_inv_first in Hcont as Heq. subst.
@@ -100,82 +93,73 @@ Section stack_macros.
     destruct l;[inversion Hlength|].
     iPrologue "Hprog".
     iApply (wp_move_success_reg_fromPC with "[$HPC $Hi $Hr_t1]");
-      [apply decode_encode_instrW_inv|apply Hfl|iCorrectPC a_first a_last|iContiguous_next Hcont 0|auto|..].
+      [apply decode_encode_instrW_inv|iCorrectPC a_first a_last|iContiguous_next Hcont 0|auto|..].
     iEpilogue "(HPC & Hprog_done & Hr_t1)".
     (* getb r_t2 r_t1 *)
     destruct l;[inversion Hlength|]. 
     iPrologue "Hprog".
     iApply (wp_Get_success with "[$HPC $Hi $Hr_t2 $Hr_t1]");
-      [apply decode_encode_instrW_inv|auto|apply Hfl|iCorrectPC a_first a_last|iContiguous_next Hcont 1|auto..].
+      [apply decode_encode_instrW_inv|auto|iCorrectPC a_first a_last|iContiguous_next Hcont 1|auto..].
     iEpilogue "(HPC & Hi & Hr_t1 & Hr_t2) /="; iCombine "Hi" "Hprog_done" as "Hprog_done". 
     (* geta r_t3 r_t1 *)
     destruct l;[inversion Hlength|]. 
     iPrologue "Hprog".
     iApply (wp_Get_success with "[$HPC $Hi $Hr_t3 $Hr_t1]");
-      [apply decode_encode_instrW_inv|auto|apply Hfl|iCorrectPC a_first a_last|iContiguous_next Hcont 2|auto..].
+      [apply decode_encode_instrW_inv|auto|iCorrectPC a_first a_last|iContiguous_next Hcont 2|auto..].
     iEpilogue "(HPC & Hi & Hr_t1 & Hr_t3) /="; iCombine "Hi" "Hprog_done" as "Hprog_done". 
     (* sub r_t2 r_t2 r_t3 *)
     destruct l;[inversion Hlength|]. 
     iPrologue "Hprog".
     iApply (wp_add_sub_lt_success_dst_r with "[$HPC $Hi $Hr_t3 $Hr_t2]");
-      [apply decode_encode_instrW_inv|auto|iContiguous_next Hcont 3|apply Hfl|iCorrectPC a_first a_last|..].
+      [apply decode_encode_instrW_inv|auto|iContiguous_next Hcont 3|iCorrectPC a_first a_last|..].
     iEpilogue "(HPC & Hi & Hr_t3 & Hr_t2) /="; iCombine "Hi" "Hprog_done" as "Hprog_done". 
     (* lea r_t1 r_t2 *)
     destruct l;[inversion Hlength|]. 
     iPrologue "Hprog".
     assert ((a_first + (pc_b - a_first))%a = Some pc_b) as Hlea;[solve_addr|]. 
     iApply (wp_lea_success_reg with "[$HPC $Hi $Hr_t1 $Hr_t2]");
-      [apply decode_encode_instrW_inv|auto|iCorrectPC a_first a_last|iContiguous_next Hcont 4|apply Hlea|auto..].
+      [apply decode_encode_instrW_inv|iCorrectPC a_first a_last|iContiguous_next Hcont 4|apply Hlea|auto..].
     { apply contiguous_between_length in Hcont.
       apply isCorrectPC_range_perm in Hvpc; [|revert Hcont; clear; solve_addr].
-      destruct Hvpc as [-> | [-> | ->] ]; auto. }
-    { apply contiguous_between_length in Hcont.
-      assert (a_first < a_last)%Z as Hlt;[simpl in Hcont;solve_addr|].
-      apply isCorrectPC_inrange with (a:=a_first) in Hvpc;[|lia].
-      destruct pc_p;auto;inversion Hvpc;solve_addr. }
+      destruct Hvpc as [-> | ->]; auto. }
     iEpilogue "(HPC & Hi & Hr_t2 & Hr_t1) /="; iCombine "Hi" "Hprog_done" as "Hprog_done". 
     (* load r_t1 r_t1 *)
     destruct l;[inversion Hlength|]. 
     iPrologue "Hprog".
     iAssert (⌜(pc_b ≠ a3)%Z⌝)%I as %Hneq.
     { iIntros (Hcontr);subst.
-      iDestruct (cap_duplicate_false with "[$Hi $Hpc_b]") as %Hne; auto.
-      apply contiguous_between_length in Hcont.
-      apply isCorrectPC_range_perm in Hvpc; [|revert Hcont; clear; solve_addr].
-      destruct pc_p'; auto. destruct pc_p; inversion Hfl.
-      destruct Hvpc as [Hcontr | [Hcontr | Hcontr] ]; done.
-    }
+      iDestruct (mapsto_valid_2 with "Hi Hpc_b") as %?. done. }
     iApply (wp_load_success_same with "[$HPC $Hi $Hr_t1 Hpc_b]");
-      [|apply decode_encode_instrW_inv|auto|iCorrectPC a_first a_last| |iContiguous_next Hcont 5|..].
-    { exact (inr (RW, Global, b_link, e_link, a_link)). }
+      [|apply decode_encode_instrW_inv|iCorrectPC a_first a_last| |iContiguous_next Hcont 5|..].
+    { exact (inr (RW, b_link, e_link, a_link)). }
     { apply contiguous_between_length in Hcont as Hlen.
       assert (pc_b < pc_e)%Z as Hle.
       { eapply isCorrectPC_contiguous_range in Hvpc as Hwb';[|eauto|apply elem_of_cons;left;eauto].
         inversion Hwb'. solve_addr. }
       apply isCorrectPC_range_perm in Hvpc as Heq; [|revert Hlen; clear; solve_addr].      
-      split;[destruct Heq as [-> | [-> | ->] ]; auto|].
+      split;[destruct Heq as [-> | ->]; auto|].
       apply andb_true_intro. split;[apply Z.leb_le;solve_addr|apply Z.ltb_lt;auto].
     }
-    { destruct (pc_b =? a3)%a; [done|iFrame]. auto. }
+    { destruct (pc_b =? a3)%a; [done|iFrame]. }
     destruct ((pc_b =? a3)%a) eqn:Hcontr;[apply Z.eqb_eq in Hcontr;apply z_of_eq in Hcontr;congruence|clear Hcontr]. 
     iEpilogue "(HPC & Hr_t1 & Hi & Hpc_b)"; iCombine "Hi" "Hprog_done" as "Hprog_done".
     (* lea r_t1 f *)
     destruct l;[inversion Hlength|]. 
     iPrologue "Hprog".
     iApply (wp_lea_success_z with "[$HPC $Hi $Hr_t1]");
-      [apply decode_encode_instrW_inv|auto|iCorrectPC a_first a_last|iContiguous_next Hcont 6|apply Hentry|simpl;auto..].
+      [apply decode_encode_instrW_inv|iCorrectPC a_first a_last|iContiguous_next Hcont 6|apply Hentry|simpl;auto..].
     iEpilogue "(HPC & Hi & Hr_t1)"; iCombine "Hi" "Hprog_done" as "Hprog_done".
     (* move r_t2 0 *)
     destruct l;[inversion Hlength|]. 
     iPrologue "Hprog".
     iApply (wp_move_success_z with "[$HPC $Hi $Hr_t2]");
-      [apply decode_encode_instrW_inv|apply Hfl|iCorrectPC a_first a_last|iContiguous_next Hcont 7|auto|..].
+      [apply decode_encode_instrW_inv|iCorrectPC a_first a_last|iContiguous_next Hcont 7|auto|..].
     iEpilogue "(HPC & Hi & Hr_t2)"; iCombine "Hi" "Hprog_done" as "Hprog_done".
     (* move r_t3 0 *)
     destruct l;[inversion Hlength|]. 
     iPrologue "Hprog".
     iApply (wp_move_success_z with "[$HPC $Hi $Hr_t3]");
-      [apply decode_encode_instrW_inv|apply Hfl|iCorrectPC a_first a_last|iContiguous_next Hcont 8|auto|..].
+      [apply decode_encode_instrW_inv|iCorrectPC a_first a_last|iContiguous_next Hcont 8|auto|..].
     iEpilogue "(HPC & Hi & Hr_t3)"; iCombine "Hi" "Hprog_done" as "Hprog_done".
     (* load r_t1 r_t1 *)
     destruct l;[|inversion Hlength].
@@ -183,21 +167,16 @@ Section stack_macros.
     iPrologue "Hprog".
     iAssert (⌜(entry_a ≠ a7)%Z⌝)%I as %Hneq'.
     { iIntros (Hcontr);subst.
-      iDestruct (cap_duplicate_false with "[$Hi $Ha_entry]") as %Hne; auto.
-      apply contiguous_between_length in Hcont.
-      apply isCorrectPC_range_perm in Hvpc; [|revert Hcont; clear; solve_addr].
-      destruct pc_p'; auto. destruct pc_p; inversion Hfl.
-      destruct Hvpc as [Hcontr | [Hcontr | Hcontr] ]; done.
-    }
+      iDestruct (mapsto_valid_2 with "Hi Ha_entry") as %?. done. }
     iApply (wp_load_success_same with "[$HPC $Hi $Hr_t1 Ha_entry]");
-      [exact wentry|apply decode_encode_instrW_inv|auto|iCorrectPC a_first a_last|auto|apply Hlink|..].
+      [exact wentry|apply decode_encode_instrW_inv|iCorrectPC a_first a_last|auto|apply Hlink|..].
     { destruct (entry_a =? a7)%a; auto. }
     destruct ((entry_a =? a7)%a) eqn:Hcontr;[apply Z.eqb_eq in Hcontr;apply z_of_eq in Hcontr;congruence|clear Hcontr]. 
     iEpilogue "(HPC & Hr_t1 & Hi & Hentry_a)"; iCombine "Hi" "Hprog_done" as "Hprog_done".
     (* continuation *)
     iApply "Hφ".
     iFrame. 
-    repeat iDestruct "Hprog_done" as "[$ Hprog_done]". 
+    do 9 iDestruct "Hprog_done" as "[$ Hprog_done]". 
     iFrame.
   Qed.
 
@@ -219,8 +198,8 @@ Section stack_macros.
     move_z r_t1 0;
     fail_end].
 
-  Definition assert_fail a p :=
-    ([∗ list] a_i;w_i ∈ a;(assert_fail_instrs), a_i ↦ₐ[p] w_i)%I. 
+  Definition assert_fail a :=
+    ([∗ list] a_i;w_i ∈ a;(assert_fail_instrs), a_i ↦ₐ w_i)%I. 
 
   (* f_a is the offset of the failure subroutine in the linking table *)
   (* assert r z asserts that the register r contains the integer z *)
@@ -231,39 +210,38 @@ Section stack_macros.
     jnz r_t1 r;
     move_z r_t1 0].
 
-  Definition assert_r_z a f_a r z p :=
-    ([∗ list] a_i;w_i ∈ a;(assert_r_z_instrs f_a r z), a_i ↦ₐ[p] w_i)%I. 
+  Definition assert_r_z a f_a r z :=
+    ([∗ list] a_i;w_i ∈ a;(assert_r_z_instrs f_a r z), a_i ↦ₐ w_i)%I. 
 
   (* Spec for assertion success *)
   (* Since we are not jumping to the failure subroutine, we do not need any assumptions 
      about the failure subroutine *)
-  Lemma assert_r_z_success a f_a r z pc_p pc_p' pc_g pc_b pc_e a_first a_last
+  Lemma assert_r_z_success a f_a r z pc_p pc_b pc_e a_first a_last
         b_link e_link a_link a_entry fail_cap w_r φ :
-    isCorrectPC_range pc_p pc_g pc_b pc_e a_first a_last →
-    PermFlows pc_p pc_p' →
+    isCorrectPC_range pc_p pc_b pc_e a_first a_last →
     contiguous_between a a_first a_last →
     (* linking table assumptions *)
-    withinBounds (RW, Global, b_link, e_link, a_entry) = true →
+    withinBounds (RW, b_link, e_link, a_entry) = true →
     (a_link + f_a)%a = Some a_entry ->
     (* condition for assertion success *)
     (w_r = inl z) ->
 
-    ▷ assert_r_z a f_a r z pc_p'
-    ∗ ▷ PC ↦ᵣ inr (pc_p,pc_g,pc_b,pc_e,a_first)
-    ∗ ▷ pc_b ↦ₐ[pc_p'] inr (RO,Global,b_link,e_link,a_link)
-    ∗ ▷ a_entry ↦ₐ[RO] fail_cap
+    ▷ assert_r_z a f_a r z
+    ∗ ▷ PC ↦ᵣ inr (pc_p,pc_b,pc_e,a_first)
+    ∗ ▷ pc_b ↦ₐ inr (RO,b_link,e_link,a_link)
+    ∗ ▷ a_entry ↦ₐ fail_cap
     ∗ ▷ r ↦ᵣ w_r
     ∗ ▷ (∃ w, r_t1 ↦ᵣ w)
     ∗ ▷ (∃ w, r_t2 ↦ᵣ w)
     ∗ ▷ (∃ w, r_t3 ↦ᵣ w)
     ∗ ▷ (r_t1 ↦ᵣ inl 0%Z ∗ r_t2 ↦ᵣ inl 0%Z ∗ r_t3 ↦ᵣ inl 0%Z ∗ r ↦ᵣ inl 0%Z
-         ∗ PC ↦ᵣ inr (pc_p,pc_g,pc_b,pc_e,a_last) ∗ assert_r_z a f_a r z pc_p'
-         ∗ pc_b ↦ₐ[pc_p'] inr (RO,Global,b_link,e_link,a_link) ∗ a_entry ↦ₐ[RO] fail_cap
+         ∗ PC ↦ᵣ inr (pc_p,pc_b,pc_e,a_last) ∗ assert_r_z a f_a r z 
+         ∗ pc_b ↦ₐ inr (RO,b_link,e_link,a_link) ∗ a_entry ↦ₐ fail_cap
          -∗ WP Seq (Instr Executable) {{ φ }})
     ⊢
     WP Seq (Instr Executable) {{ φ }}.
   Proof.
-    iIntros (Hvpc Hfl Hcont Hwb Htable Hsuccess)
+    iIntros (Hvpc Hcont Hwb Htable Hsuccess)
             "(>Hprog & >HPC & >Hpc_b & >Ha_entry & >Hr & >Hr_t1 & >Hr_t2 & >Hr_t3 & Hφ)".
      (* fetch f *)
     iDestruct (contiguous_between_program_split with "Hprog") as (fetch_prog rest link)
@@ -273,12 +251,12 @@ Section stack_macros.
     iDestruct "Hr_t2" as (w2) "Hr_t2".
     iDestruct "Hr_t3" as (w3) "Hr_t3". 
     iApply (fetch_spec with "[$HPC $Hfetch $Hr_t1 $Hr_t2 $Hr_t3 $Ha_entry $Hpc_b Hφ Hprog Hr]");
-      [|apply Hfl|apply Hcont_fetch|apply Hwb|apply Htable|]. 
+      [|apply Hcont_fetch|apply Hwb|apply Htable|]. 
     { intros mid Hmid. apply isCorrectPC_inrange with a_first a_last; auto.
       apply contiguous_between_bounds in Hcont_rest. revert Hcont_rest Hmid; clear. solve_addr. }
     iNext. iIntros "(HPC & Hfetch& Hr_t1 & Hr_t2 & Hr_t3 & Hpc_b & Ha_entry)".
     iDestruct (big_sepL2_length with "Hprog") as %Hlength_rest.
-    assert (isCorrectPC_range pc_p pc_g pc_b pc_e link a_last) as Hvpc_rest.
+    assert (isCorrectPC_range pc_p pc_b pc_e link a_last) as Hvpc_rest.
     { intros mid Hmid. apply isCorrectPC_inrange with a_first a_last; auto. revert Hmid Hlink;clear. solve_addr. }
     destruct rest as [|a0 l'];[inversion Hlength_rest|].
     apply contiguous_between_cons_inv_first in Hcont_rest as Heq. subst a0.
@@ -287,21 +265,21 @@ Section stack_macros.
     inversion Hsuccess. subst w_r.  
     iPrologue "Hprog".
     iApply (wp_add_sub_lt_success_dst_z with "[$HPC $Hi $Hr]");
-      [apply decode_encode_instrW_inv|right;left;eauto|iContiguous_next Hcont_rest 0|apply Hfl|iCorrectPC link a_last|..].
+      [apply decode_encode_instrW_inv|right;left;eauto|iContiguous_next Hcont_rest 0|iCorrectPC link a_last|..].
     iEpilogue "(HPC & Hi & Hr)"; iCombine "Hfetch" "Hi" as "Hprog_done". 
     (* jnz r_t1 r *)
     rewrite /= Z.sub_diag. 
     destruct l';[inversion Hlength_rest|].
     iPrologue "Hprog".
     iApply (wp_jnz_success_next with "[$HPC $Hi $Hr_t1 $Hr]");
-      [apply decode_encode_instrW_inv|apply Hfl|iCorrectPC link a_last|iContiguous_next Hcont_rest 1|].
+      [apply decode_encode_instrW_inv|iCorrectPC link a_last|iContiguous_next Hcont_rest 1|].
     iEpilogue "(HPC & Hinstr & Hr_t1 & Hr)". iCombine "Hinstr" "Hprog_done" as "Hprog_done".  
     (* move r_t1 0 *)
     destruct l';[|inversion Hlength_rest].
     apply contiguous_between_last with (ai:=a1) in Hcont_rest as Hlink';[|auto].
     iPrologue "Hprog".
     iApply (wp_move_success_z with "[$HPC $Hi $Hr_t1]");
-      [apply decode_encode_instrW_inv|apply Hfl|iCorrectPC link a_last|apply Hlink'|auto|..].
+      [apply decode_encode_instrW_inv|iCorrectPC link a_last|apply Hlink'|auto|..].
     iEpilogue "(HPC & Hi & Hr_t1)"; iCombine "Hi" "Hprog_done" as "Hprog_done".
     (* Continuation *)
     iApply "Hφ". iFrame.
@@ -311,36 +289,34 @@ Section stack_macros.
   (* Spec for assertion failure *)
   (* When the assertion fails, the program jumps to the failure subroutine, sets the 
      flag (which by convention is one address after subroutine) and Fails *)
-  Lemma assert_r_z_fail a f_a r z pc_p pc_p' pc_g pc_b pc_e a_first a_last z_r
+  Lemma assert_r_z_fail a f_a r z pc_p pc_b pc_e a_first a_last z_r
         b_link e_link a_link a_entry
         f_b f_e f_a_first f_a_last a' a_env (* fail subroutine *)
-        flag_p flag_p' flag_b flag_e flag_a (* flag capability *) :
-    isCorrectPC_range pc_p pc_g pc_b pc_e a_first a_last →
-    PermFlows pc_p pc_p' → 
+        flag_p flag_b flag_e flag_a (* flag capability *) :
+    isCorrectPC_range pc_p pc_b pc_e a_first a_last →
     contiguous_between a a_first a_last →
     (* linking table assumptions *)
-    withinBounds (RW, Global, b_link, e_link, a_entry) = true →
+    withinBounds (RW, b_link, e_link, a_entry) = true →
     (a_link + f_a)%a = Some a_entry ->
     (* failure subroutine assumptions *)
-    isCorrectPC_range RX Global f_b f_e f_a_first f_a_last →
+    isCorrectPC_range RX f_b f_e f_a_first f_a_last →
     contiguous_between a' f_a_first f_a_last →
     (f_a_first + (length a'))%a = Some a_env ->
-    withinBounds (RX,Global,f_b,f_e,a_env) = true ->
+    withinBounds (RX,f_b,f_e,a_env) = true ->
     (* flag assumptions *)
-    PermFlows flag_p flag_p' →
-    withinBounds (flag_p,Global,flag_b,flag_e,flag_a) = true ∧ writeAllowed flag_p = true ->
+    withinBounds (flag_p,flag_b,flag_e,flag_a) = true ∧ writeAllowed flag_p = true ->
     (* condition for assertion success *)
     (z_r ≠ z) ->
 
     (* the assert and assert failure subroutine programs *)
-    {{{ ▷ assert_r_z a f_a r z pc_p'
-    ∗ ▷ assert_fail a' RX
-    ∗ ▷ PC ↦ᵣ inr (pc_p,pc_g,pc_b,pc_e,a_first)
+    {{{ ▷ assert_r_z a f_a r z
+    ∗ ▷ assert_fail a' 
+    ∗ ▷ PC ↦ᵣ inr (pc_p,pc_b,pc_e,a_first)
     (* linking table and assertion flag *)
-    ∗ ▷ pc_b ↦ₐ[pc_p'] inr (RO,Global,b_link,e_link,a_link) (* the linking table capability *)
-    ∗ ▷ a_entry ↦ₐ[RO] inr (E,Global,f_b,f_e,f_a_first) (* the capability to the failure subroutine *)
-    ∗ ▷ a_env ↦ₐ[RX] inr (flag_p,Global,flag_b,flag_e,flag_a) (* the assertion flag capability *)
-    ∗ ▷ (∃ w, flag_a ↦ₐ[flag_p'] w) (* the assertion flag *)
+    ∗ ▷ pc_b ↦ₐ inr (RO,b_link,e_link,a_link) (* the linking table capability *)
+    ∗ ▷ a_entry ↦ₐ inr (E,f_b,f_e,f_a_first) (* the capability to the failure subroutine *)
+    ∗ ▷ a_env ↦ₐ inr (flag_p,flag_b,flag_e,flag_a) (* the assertion flag capability *)
+    ∗ ▷ (∃ w, flag_a ↦ₐ w) (* the assertion flag *)
     (* registers *)
     ∗ ▷ r ↦ᵣ inl z_r
     ∗ ▷ (∃ w, r_t1 ↦ᵣ w)
@@ -350,12 +326,12 @@ Section stack_macros.
       Seq (Instr Executable)
       
     {{{ RET FailedV; r_t1 ↦ᵣ inl 0%Z ∗ r_t2 ↦ᵣ inl 0%Z ∗ r_t3 ↦ᵣ inl 0%Z ∗ (∃ z, r ↦ᵣ inl z ∧ ⌜z ≠ 0⌝)
-         ∗ PC ↦ᵣ inr (RX, Global, f_b, f_e,^(f_a_last + (-1))%a)
-         ∗ assert_r_z a f_a r z pc_p' ∗ assert_fail a' RX
-         ∗ pc_b ↦ₐ[pc_p'] inr (RO,Global,b_link,e_link,a_link) ∗ a_entry ↦ₐ[RO] inr (E,Global,f_b,f_e,f_a_first)
-         ∗ a_env ↦ₐ[RX] inr (flag_p,Global,flag_b,flag_e,flag_a) ∗ flag_a ↦ₐ[flag_p'] inl 1%Z }}}. 
+         ∗ PC ↦ᵣ inr (RX, f_b, f_e,^(f_a_last + (-1))%a)
+         ∗ assert_r_z a f_a r z ∗ assert_fail a' 
+         ∗ pc_b ↦ₐ inr (RO,b_link,e_link,a_link) ∗ a_entry ↦ₐ inr (E,f_b,f_e,f_a_first)
+         ∗ a_env ↦ₐ inr (flag_p,flag_b,flag_e,flag_a) ∗ flag_a ↦ₐ inl 1%Z }}}. 
   Proof.
-    iIntros (Hvpc Hfl Hcont Hwb Htable Hvpc' Hcont' Henv Henvwb Hfl' [Hwb' Hwa] Hfailure φ) 
+    iIntros (Hvpc Hcont Hwb Htable Hvpc' Hcont' Henv Henvwb [Hwb' Hwa] Hfailure φ) 
             "(>Hprog & >Hprog' & >HPC & >Hpc_b & >Ha_entry & >Ha_env & >Hflag & >Hr & >Hr_t1 & >Hr_t2 & >Hr_t3) Hφ".
     iDestruct "Hflag" as (flag_w) "Hflag". 
     (* fetch f *)
@@ -366,12 +342,12 @@ Section stack_macros.
     iDestruct "Hr_t2" as (w2) "Hr_t2".
     iDestruct "Hr_t3" as (w3) "Hr_t3". 
     iApply (fetch_spec with "[$HPC $Hfetch $Hr_t1 $Hr_t2 $Hr_t3 $Ha_entry $Hpc_b Hφ Hprog Hr Hprog' Ha_env Hflag]");
-      [|apply Hfl|apply Hcont_fetch|apply Hwb|apply Htable|]. 
+      [|apply Hcont_fetch|apply Hwb|apply Htable|]. 
     { intros mid Hmid. apply isCorrectPC_inrange with a_first a_last; auto.
       apply contiguous_between_bounds in Hcont_rest. revert Hcont_rest Hmid; clear. solve_addr. }
     iNext. iIntros "(HPC & Hfetch& Hr_t1 & Hr_t2 & Hr_t3 & Hpc_b & Ha_entry)".
     iDestruct (big_sepL2_length with "Hprog") as %Hlength_rest.
-    assert (isCorrectPC_range pc_p pc_g pc_b pc_e link a_last) as Hvpc_rest.
+    assert (isCorrectPC_range pc_p pc_b pc_e link a_last) as Hvpc_rest.
     { intros mid Hmid. apply isCorrectPC_inrange with a_first a_last; auto. revert Hmid Hlink;clear. solve_addr. }
     destruct rest as [|a0 l'];[inversion Hlength_rest|].
     apply contiguous_between_cons_inv_first in Hcont_rest as Heq. subst a0.
@@ -379,12 +355,12 @@ Section stack_macros.
     destruct l';[inversion Hlength_rest|].
     iPrologue "Hprog".
     iApply (wp_add_sub_lt_success_dst_z with "[$HPC $Hi $Hr]");
-      [apply decode_encode_instrW_inv|right;left;eauto|iContiguous_next Hcont_rest 0|apply Hfl|iCorrectPC link a_last|..].
+      [apply decode_encode_instrW_inv|right;left;eauto|iContiguous_next Hcont_rest 0|iCorrectPC link a_last|..].
     iEpilogue "(HPC & Hi & Hr)"; iCombine "Hi" "Hfetch" as "Hprog_done". 
     (* jnz r_t1 r *)
     iPrologue "Hprog".
     iApply (wp_jnz_success_jmp with "[$HPC $Hi $Hr_t1 $Hr]");
-      [apply decode_encode_instrW_inv|apply Hfl|iCorrectPC link a_last|simpl;revert Hfailure;clear;intros Hne Hcontr;simplify_eq;lia|..].
+      [apply decode_encode_instrW_inv|iCorrectPC link a_last|simpl;revert Hfailure;clear;intros Hne Hcontr;simplify_eq;lia|..].
     iEpilogue "(HPC & Hi & Hr_t1 & Hr)"; iSimpl in "HPC"; iCombine "Hi" "Hprog_done" as "Hprog_done".
     iCombine "Hprog" "Hprog_done" as "Hprog_done".
     (* FAILURE SUBROUTINE *)
@@ -397,7 +373,7 @@ Section stack_macros.
     { iIntros (Hcontr). rewrite Hcontr. iDestruct (regname_dupl_false with "Hr_t1 HPC") as "H". done. }
     iPrologue "Hprog'".
     iApply (wp_move_success_reg_fromPC with "[$HPC $Hi $Hr_t1]");
-      [apply decode_encode_instrW_inv|apply PermFlows_refl|iCorrectPC f_a_first f_a_last|iContiguous_next Hcont' 0|auto|..].
+      [apply decode_encode_instrW_inv|iCorrectPC f_a_first f_a_last|iContiguous_next Hcont' 0|auto|..].
     iEpilogue "(HPC & Hi & Hr_t1)". iRename "Hi" into "Hprog_done'". 
     (* lea r_t1 5 *)
     destruct a';[inversion Hlength'|].
@@ -405,38 +381,37 @@ Section stack_macros.
     assert ((f_a_first + 6)%a = Some a_env) as Hlea.
     { simpl in Henv. inversion Hlength' as [Heq]. rewrite Heq in Henv. auto. }
     iApply (wp_lea_success_z with "[$HPC $Hi $Hr_t1]");
-      [apply decode_encode_instrW_inv|apply PermFlows_refl|iCorrectPC f_a_first f_a_last|iContiguous_next Hcont' 1|apply Hlea|auto..].
-    { simpl; auto. }
+      [apply decode_encode_instrW_inv|iCorrectPC f_a_first f_a_last|iContiguous_next Hcont' 1|apply Hlea|auto..].
     iEpilogue "(HPC & Hi & Hr_t1)". iCombine "Hi" "Hprog_done'" as "Hprog_done'".
     (* load r_t1 r_t1 *)
     destruct a';[inversion Hlength'|].
     iPrologue "Hprog".
     iAssert (⌜(a_env =? a2)%a = false⌝)%I as %Hne'.
     { destruct (decide (a_env = a2)%Z); [subst|iPureIntro;apply Z.eqb_neq,neq_z_of;auto].
-      iDestruct (cap_duplicate_false with "[$Hi $Ha_env]") as "H";auto. }
+      iDestruct (mapsto_valid_2 with "Hi Ha_env") as %?. done. } 
     iApply (wp_load_success_same with "[$HPC $Hi $Hr_t1 Ha_env]");
-      [|apply decode_encode_instrW_inv|apply PermFlows_refl|iCorrectPC f_a_first f_a_last|split;auto|iContiguous_next Hcont' 2|
+      [|apply decode_encode_instrW_inv|iCorrectPC f_a_first f_a_last|split;auto|iContiguous_next Hcont' 2|
        rewrite Hne';iFrame|rewrite Hne'];auto. 
     iEpilogue "(HPC & Hr_t1 & Hi & Ha_env)". iCombine "Hi" "Hprog_done" as "Hprog_done".
     (* store r_t1 1 *)
     destruct a';[inversion Hlength'|].
     iPrologue "Hprog".
     iApply (wp_store_success_z with "[$HPC $Hi $Hr_t1 $Hflag]");
-      [apply decode_encode_instrW_inv|apply PermFlows_refl|apply Hfl'|iCorrectPC f_a_first f_a_last|iContiguous_next Hcont' 3|
+      [apply decode_encode_instrW_inv|iCorrectPC f_a_first f_a_last|iContiguous_next Hcont' 3|
        split;auto|].    
     iEpilogue "(HPC & Hi & Hr_t1 & Hflag)"; iCombine "Hi" "Hprog_done" as "Hprog_done".
     (* move r_t1 0 *)
     destruct a';[inversion Hlength'|].
     iPrologue "Hprog".
     iApply (wp_move_success_z with "[$HPC $Hi $Hr_t1]");
-      [apply decode_encode_instrW_inv|apply PermFlows_refl|iCorrectPC f_a_first f_a_last|iContiguous_next Hcont' 4|auto|].
+      [apply decode_encode_instrW_inv|iCorrectPC f_a_first f_a_last|iContiguous_next Hcont' 4|].
     iEpilogue "(HPC & Hi & Hr_t1)"; iCombine "Hi" "Hprog_done" as "Hprog_done".
     (* Halt *)
     destruct a';[|inversion Hlength'].
     apply contiguous_between_last with (ai:=a5) in Hcont' as Hlink';[|auto].
     iPrologue "Hprog".
     iApply (wp_fail with "[$HPC $Hi]");
-      [apply decode_encode_instrW_inv|apply PermFlows_refl|iCorrectPC f_a_first f_a_last|].
+      [apply decode_encode_instrW_inv|iCorrectPC f_a_first f_a_last|].
     iEpilogue "(HPC & Hi)".
     iApply wp_value. iApply "Hφ".
     iFrame. iSplitL "Hr".
@@ -464,44 +439,40 @@ Section stack_macros.
     move_r r_t0 r_t5;
     move_z r_t5 0].
 
-  Definition malloc f_m size a p : iProp Σ :=
-    ([∗ list] a_i;w_i ∈ a;(malloc_instrs f_m size), a_i ↦ₐ[p] w_i)%I. 
+  Definition malloc f_m size a : iProp Σ :=
+    ([∗ list] a_i;w_i ∈ a;(malloc_instrs f_m size), a_i ↦ₐ w_i)%I. 
 
   (* malloc spec *)
-  Lemma malloc_spec W size cont a pc_p pc_p' pc_g pc_b pc_e a_first a_last
+  Lemma malloc_spec size cont a pc_p pc_b pc_e a_first a_last
         b_link e_link a_link f_m a_entry mallocN b_m e_m EN rmap φ :
-    isCorrectPC_range pc_p pc_g pc_b pc_e a_first a_last →
-    PermFlows pc_p pc_p' →
+    isCorrectPC_range pc_p pc_b pc_e a_first a_last →
     contiguous_between a a_first a_last →
-    withinBounds (RW, Global, b_link, e_link, a_entry) = true →
+    withinBounds (RW, b_link, e_link, a_entry) = true →
     (a_link + f_m)%a = Some a_entry →
     dom (gset RegName) rmap = all_registers_s ∖ {[ PC; r_t0 ]} →
     ↑mallocN ⊆ EN →
     size > 0 →
 
     (* malloc program and subroutine *)
-    ▷ malloc f_m size a pc_p'
+    ▷ malloc f_m size a
     ∗ na_inv logrel_nais mallocN (malloc_inv b_m e_m)
     ∗ na_own logrel_nais EN
     (* we need to assume that the malloc capability is in the linking table at offset f_m *)
-    ∗ ▷ pc_b ↦ₐ[pc_p'] inr (RO,Global,b_link,e_link,a_link)
-    ∗ ▷ a_entry ↦ₐ[RO] inr (E,Global,b_m,e_m,b_m)
+    ∗ ▷ pc_b ↦ₐ inr (RO,b_link,e_link,a_link)
+    ∗ ▷ a_entry ↦ₐ inr (E,b_m,e_m,b_m)
     (* register state *)
-    ∗ ▷ PC ↦ᵣ inr (pc_p,pc_g,pc_b,pc_e,a_first)
+    ∗ ▷ PC ↦ᵣ inr (pc_p,pc_b,pc_e,a_first)
     ∗ ▷ r_t0 ↦ᵣ cont
     ∗ ▷ ([∗ map] r_i↦w_i ∈ rmap, r_i ↦ᵣ w_i)
-    (* current world *)
-    ∗ ▷ region W
-    ∗ ▷ sts_full_world W
     (* continuation *)
-    ∗ ▷ (PC ↦ᵣ inr (pc_p,pc_g,pc_b,pc_e,a_last) ∗ malloc f_m size a pc_p'
-         ∗ pc_b ↦ₐ[pc_p'] inr (RO,Global,b_link,e_link,a_link)
-         ∗ a_entry ↦ₐ[RO] inr (E,Global,b_m,e_m,b_m)
+    ∗ ▷ (PC ↦ᵣ inr (pc_p,pc_b,pc_e,a_last) ∗ malloc f_m size a 
+         ∗ pc_b ↦ₐ inr (RO,b_link,e_link,a_link)
+         ∗ a_entry ↦ₐ inr (E,b_m,e_m,b_m)
          (* the newly allocated region *)
          ∗ (∃ (b e : Addr),
             ⌜(b + size)%a = Some e⌝
-            ∗ r_t1 ↦ᵣ inr (RWX,Global,b,e,b)
-            ∗ [[b,e]] ↦ₐ[RWX] [[region_addrs_zeroes b e]])
+            ∗ r_t1 ↦ᵣ inr (RWX,b,e,b)
+            ∗ [[b,e]] ↦ₐ [[region_addrs_zeroes b e]])
          ∗ r_t0 ↦ᵣ cont
          ∗ na_own logrel_nais EN
          ∗ ([∗ map] r_i↦w_i ∈ (<[r_t2:=inl 0%Z]>
@@ -510,14 +481,12 @@ Section stack_macros.
                                  (<[r_t5:=inl 0%Z]> (delete r_t1 rmap))))), r_i ↦ᵣ w_i)
          (* the newly allocated region is fresh in the current world *)
          (* ∗ ⌜Forall (λ a, a ∉ dom (gset Addr) (std W)) (region_addrs b e)⌝ *)
-         ∗ region W
-         ∗ sts_full_world W
          -∗ WP Seq (Instr Executable) {{ φ }})
     ⊢
       WP Seq (Instr Executable) {{ λ v, φ v ∨ ⌜v = FailedV⌝ }}.
   Proof.
-    iIntros (Hvpc Hfl Hcont Hwb Ha_entry Hrmap_dom HmallocN Hsize)
-            "(>Hprog & #Hmalloc & Hna & >Hpc_b & >Ha_entry & >HPC & >Hr_t0 & >Hregs & Hr & Hsts & Hφ)".
+    iIntros (Hvpc Hcont Hwb Ha_entry Hrmap_dom HmallocN Hsize)
+            "(>Hprog & #Hmalloc & Hna & >Hpc_b & >Ha_entry & >HPC & >Hr_t0 & >Hregs & Hφ)".
     (* extract necessary registers from regs *)
     iDestruct (big_sepL2_length with "Hprog") as %Hlength.
     assert (is_Some (rmap !! r_t1)) as [rv1 ?]. by rewrite elem_of_gmap_dom Hrmap_dom; set_solver.
@@ -535,12 +504,12 @@ Section stack_macros.
                                                                    "(Hfetch & Hprog & #Hcont)";[apply Hcont|].
     iDestruct "Hcont" as %(Hcont_fetch & Hcont_rest & Heqapp & Hlink).
     iApply (fetch_spec with "[- $HPC $Hfetch $Hr_t1 $Hr_t2 $Hr_t3 $Ha_entry $Hpc_b]");
-      [|apply Hfl|apply Hcont_fetch|apply Hwb|apply Ha_entry|]. 
+      [|apply Hcont_fetch|apply Hwb|apply Ha_entry|]. 
     { intros mid Hmid. apply isCorrectPC_inrange with a_first a_last; auto.
       apply contiguous_between_bounds in Hcont_rest. revert Hcont_rest Hmid; clear. solve_addr. }
     iNext. iIntros "(HPC & Hfetch& Hr_t1 & Hr_t2 & Hr_t3 & Hpc_b & Ha_entry)".
     iDestruct (big_sepL2_length with "Hprog") as %Hlength_rest.
-    assert (isCorrectPC_range pc_p pc_g pc_b pc_e link a_last) as Hvpc_rest.
+    assert (isCorrectPC_range pc_p pc_b pc_e link a_last) as Hvpc_rest.
     { intros mid Hmid. apply isCorrectPC_inrange with a_first a_last; auto. revert Hmid Hlink;clear. solve_addr. }
     destruct rest as [|a l'];[inversion Hlength_rest|].
     apply contiguous_between_cons_inv_first in Hcont_rest as Heq. subst.
@@ -548,25 +517,25 @@ Section stack_macros.
     destruct l';[inversion Hlength_rest|]. 
     iPrologue "Hprog".
     iApply (wp_move_success_reg with "[$HPC $Hi $Hr_t5 $Hr_t0]");
-      [apply decode_encode_instrW_inv|apply Hfl|iCorrectPC link a_last|iContiguous_next Hcont_rest 0|auto|..].
+      [apply decode_encode_instrW_inv|iCorrectPC link a_last|iContiguous_next Hcont_rest 0|auto|..].
     iEpilogue "(HPC & Hprog_done & Hr_t5 & Hr_t0)". iCombine "Hprog_done" "Hfetch" as "Hprog_done".
     (* move r_t3 r_t1 *)
     destruct l';[inversion Hlength_rest|]. 
     iPrologue "Hprog".
     iApply (wp_move_success_reg with "[$HPC $Hi $Hr_t3 $Hr_t1]");
-      [apply decode_encode_instrW_inv|apply Hfl|iCorrectPC link a_last|iContiguous_next Hcont_rest 1|auto|..].
+      [apply decode_encode_instrW_inv|iCorrectPC link a_last|iContiguous_next Hcont_rest 1|auto|..].
     iEpilogue "(HPC & Hi & Hr_t3 & Hr_t1)"; iCombine "Hi" "Hprog_done" as "Hprog_done".
     (* move r_t1 size *)
     destruct l';[inversion Hlength_rest|].
     iPrologue "Hprog".
     iApply (wp_move_success_z with "[$HPC $Hi $Hr_t1]");
-      [apply decode_encode_instrW_inv|apply Hfl|iCorrectPC link a_last|iContiguous_next Hcont_rest 2|auto|..].
+      [apply decode_encode_instrW_inv|iCorrectPC link a_last|iContiguous_next Hcont_rest 2|auto|..].
     iEpilogue "(HPC & Hi & Hr_t1)"; iCombine "Hi" "Hprog_done" as "Hprog_done".
     (* move r_t0 PC *)
     destruct l';[inversion Hlength_rest|].
     iPrologue "Hprog".
     iApply (wp_move_success_reg_fromPC with "[$HPC $Hi $Hr_t0]");
-      [apply decode_encode_instrW_inv|apply Hfl|iCorrectPC link a_last|iContiguous_next Hcont_rest 3|auto|..].
+      [apply decode_encode_instrW_inv|iCorrectPC link a_last|iContiguous_next Hcont_rest 3|auto|..].
     iEpilogue "(HPC & Hi & Hr_t0)"; iCombine "Hi" "Hprog_done" as "Hprog_done".
     (* lea r_t0 3 *)
     destruct l';[inversion Hlength_rest|]. destruct l';[inversion Hlength_rest|].
@@ -574,19 +543,16 @@ Section stack_macros.
     assert ((a1 + 3)%a = Some a4) as Hlea.
     { apply (contiguous_between_incr_addr_middle _ _ _ 3 3 a1 a4) in Hcont_rest; auto. }
     iApply (wp_lea_success_z with "[$HPC $Hi $Hr_t0]");
-      [apply decode_encode_instrW_inv|apply Hfl|iCorrectPC link a_last|iContiguous_next Hcont_rest 4|apply Hlea|auto..].
+      [apply decode_encode_instrW_inv|iCorrectPC link a_last|iContiguous_next Hcont_rest 4|apply Hlea|auto..].
     { apply contiguous_between_length in Hcont.
       apply isCorrectPC_range_perm in Hvpc; [|revert Hcont; clear; solve_addr].
-      destruct Hvpc as [-> | [-> | ->] ]; auto. }
-    { apply contiguous_between_length in Hcont.
-      apply isCorrectPC_range_perm in Hvpc; [|revert Hcont; clear; solve_addr].
-      destruct Hvpc as [-> | [-> | ->] ]; auto. }
+      destruct Hvpc as [-> | -> ]; auto. }
     iEpilogue "(HPC & Hi & Hr_t0)"; iCombine "Hi" "Hprog_done" as "Hprog_done". 
     (* jmp r_t3 *)
     destruct l';[inversion Hlength_rest|].
     iPrologue "Hprog".
     iApply (wp_jmp_success with "[$HPC $Hi $Hr_t3]");
-      [apply decode_encode_instrW_inv|apply Hfl|iCorrectPC link a_last|]. 
+      [apply decode_encode_instrW_inv|iCorrectPC link a_last|]. 
     iEpilogue "(HPC & Hi & Hr_t3) /="; iCombine "Hi" "Hprog_done" as "Hprog_done". 
     (* we are now ready to use the malloc subroutine spec. For this we prepare the registers *)
     iDestruct (big_sepM_insert _ _ r_t3 with "[$Hregs $Hr_t3]") as "Hregs".
@@ -621,14 +587,14 @@ Section stack_macros.
     (* move r_t0 r_t5 *)
     iPrologue "Hprog".
     iApply (wp_move_success_reg with "[$HPC $Hi $Hr_t0 $Hr_t5]");
-      [apply decode_encode_instrW_inv|apply Hfl|iCorrectPC link a_last|iContiguous_next Hcont_rest 6|auto|..].
+      [apply decode_encode_instrW_inv|iCorrectPC link a_last|iContiguous_next Hcont_rest 6|auto|..].
     iEpilogue "(HPC & Hi & Hr_t0 & Hr_t5)"; iCombine "Hi" "Hprog_done" as "Hprog_done".
     (* move r_t5 0 *)
     destruct l';[| by inversion Hlength_rest].
     iPrologue "Hprog".
     apply contiguous_between_last with (ai:=a5) in Hcont_rest as Hlast;[|auto]. 
     iApply (wp_move_success_z with "[$HPC $Hi $Hr_t5]");
-      [apply decode_encode_instrW_inv|apply Hfl|iCorrectPC link a_last|apply Hlast|auto|..].
+      [apply decode_encode_instrW_inv|iCorrectPC link a_last|apply Hlast|auto|..].
     iEpilogue "(HPC & Hi & Hr_t5)"; iCombine "Hi" "Hprog_done" as "Hprog_done".
     (* continuation *)
     iApply "Hφ".
@@ -650,197 +616,7 @@ Section stack_macros.
     iExists b,e. iFrame. auto. auto.
   Qed.
 
-  (* --------------------------------------------------------------------------------- *)
-  (* ------------------------- STACK MACROS AND THEIR SPECS -------------------------- *)
-  (* --------------------------------------------------------------------------------- *)
-
-  (* -------------------------------------- PUSH ------------------------------------- *)
-  (* These versions of stack macros are for a RWLX stack  *)
-
-  Definition push_r_instrs r_stk r := [lea_z r_stk 1 ; store_r r_stk r].
-
-  Definition push_r (a1 a2 : Addr) (p : Perm) (r_stk r : RegName) : iProp Σ :=
-    ([∗ list] a;i ∈ [a1;a2];(push_r_instrs r_stk r), a ↦ₐ[p] i)%I.
-
-  Lemma push_r_spec a1 a2 a3 w w' r p p' g b e stk_b stk_e stk_a stk_a' φ :
-    isCorrectPC (inr ((p,g),b,e,a1)) ∧ isCorrectPC (inr ((p,g),b,e,a2)) →
-    PermFlows p p' ->
-    withinBounds ((RWLX,Local),stk_b,stk_e,stk_a') = true →
-    (a1 + 1)%a = Some a2 →
-    (a2 + 1)%a = Some a3 →
-    (stk_a + 1)%a = Some stk_a' →
-
-      ▷ push_r a1 a2 p' r_stk r
-    ∗ ▷ PC ↦ᵣ inr ((p,g),b,e,a1)
-    ∗ ▷ r_stk ↦ᵣ inr ((RWLX,Local),stk_b,stk_e,stk_a)
-    ∗ ▷ r ↦ᵣ w'
-    ∗ ▷ stk_a' ↦ₐ[RWLX] w
-    ∗ ▷ (PC ↦ᵣ inr ((p,g),b,e,a3) ∗ push_r a1 a2 p' r_stk r ∗
-            r_stk ↦ᵣ inr ((RWLX,Local),stk_b,stk_e,stk_a') ∗ r ↦ᵣ w' ∗ stk_a' ↦ₐ[RWLX] w'
-            -∗ WP Seq (Instr Executable) {{ φ }})
-    ⊢
-      WP Seq (Instr Executable) {{ φ }}.
-  Proof.
-    iIntros ([Hvpc1 Hvpc2] Hfl Hwb Hsuc Hlea Hstk)
-            "([Ha1 [Ha2 _] ] & HPC & Hr_stk & Hr & Hstk_a' & Hφ)".
-    iApply (wp_bind (fill [SeqCtx])).
-    iApply (wp_lea_success_z _ _ _ _ _ a1 a2 _ r_stk RWLX with "[HPC Ha1 Hr_stk]");
-      eauto; try apply decode_encode_instrW_inv; iFrame.
-    iNext. iIntros "(HPC & Ha1 & Hr_stk) /=".
-    iApply wp_pure_step_later; auto. iNext.
-    iApply (wp_bind (fill [SeqCtx])).
-    iApply (wp_store_success_reg _ _ _ _ _ a2 a3 _ r_stk r _ RWLX Local
-              with "[HPC Ha2 Hr_stk Hr Hstk_a']"); eauto; try apply decode_encode_instrW_inv;
-      first apply PermFlows_refl; iFrame.
-    iNext. iIntros "(HPC & Ha2 & Hr & Hr_stk & Hstk_a') /=".
-    iApply wp_pure_step_later; auto. iNext. iApply "Hφ". iFrame. done.
-  Qed.
-
-
-  Definition push_z_instrs r_stk z := [lea_z r_stk 1; store_z r_stk z].
-
-  Definition push_z (a1 a2 : Addr) (p : Perm) (r_stk : RegName) (z : Z) : iProp Σ :=
-    ([∗ list] a;i ∈ [a1;a2];(push_z_instrs r_stk z), a ↦ₐ[p] i)%I.
-
-  Lemma push_z_spec a1 a2 a3 w z p p' g b e stk_b stk_e stk_a stk_a' φ :
-    isCorrectPC (inr ((p,g),b,e,a1)) ∧ isCorrectPC (inr ((p,g),b,e,a2)) →
-    PermFlows p p' ->
-    withinBounds ((RWLX,Local),stk_b,stk_e,stk_a') = true →
-    (a1 + 1)%a = Some a2 →
-    (a2 + 1)%a = Some a3 →
-    (stk_a + 1)%a = Some stk_a' →
-
-      ▷ push_z a1 a2 p' r_stk z
-    ∗ ▷ PC ↦ᵣ inr ((p,g),b,e,a1)
-    ∗ ▷ r_stk ↦ᵣ inr ((RWLX,Local),stk_b,stk_e,stk_a)
-    ∗ ▷ stk_a' ↦ₐ[RWLX] w
-    ∗ ▷ (PC ↦ᵣ inr ((p,g),b,e,a3) ∗ push_z a1 a2 p' r_stk z ∗
-            r_stk ↦ᵣ inr ((RWLX,Local),stk_b,stk_e,stk_a') ∗ stk_a' ↦ₐ[RWLX] inl z
-            -∗ WP Seq (Instr Executable) {{ φ }})
-    ⊢
-      WP Seq (Instr Executable) {{ φ }}.
-  Proof.
-    iIntros ([Hvpc1 Hvpc2] Hfl Hwb Hsuc Hlea Hstk)
-            "([Ha1 [Ha2 _] ] & HPC & Hr_stk & Hstk_a' & Hφ)".
-    iApply (wp_bind (fill [SeqCtx])).
-    iApply (wp_lea_success_z _ _ _ _ _ a1 a2 _ r_stk RWLX with "[HPC Ha1 Hr_stk]");
-      eauto; first apply decode_encode_instrW_inv;iFrame.
-    iNext. iIntros "(HPC & Ha1 & Hr_stk) /=".
-    iApply wp_pure_step_later; auto. iNext.
-    iApply (wp_bind (fill [SeqCtx])).
-    iApply (wp_store_success_z _ _ _ _ _ a2 a3 _ r_stk _ _ RWLX
-              with "[HPC Ha2 Hr_stk Hstk_a']"); eauto; first apply decode_encode_instrW_inv;
-      first apply PermFlows_refl; iFrame.
-    iNext. iIntros "(HPC & Ha2 & Hr_stk & Hstk_a') /=".
-    iApply wp_pure_step_later; auto. iNext. iApply "Hφ". iFrame. done.
-  Qed.
-
-  Lemma push_z_instrs_extract a i j z prog p' :
-    contiguous_between a i j →
-    ([∗ list] a_i;w_i ∈ a; (push_z_instrs r_stk z ++ prog), a_i ↦ₐ[p'] w_i) -∗
-    ∃ a' push2 a_rest,
-      (([∗ list] a_i;w_i ∈ [i; push2];push_z_instrs r_stk z, a_i ↦ₐ[p'] w_i) ∗
-       [∗ list] a_i;w_i ∈ a'; prog, a_i ↦ₐ[p'] w_i) ∗
-       ⌜ a = [i; push2] ++ a'
-         ∧ (i + 1 = Some push2)%a
-         ∧ (push2 + 1 = Some a_rest)%a
-         ∧ contiguous_between a' a_rest j ⌝.
-  Proof.
-    intros. iIntros "HH".
-    iDestruct (contiguous_between_program_split with "HH") as (a_push a' a_rest) "(Hpush & ? & #Hcont)"; eauto.
-    iDestruct "Hcont" as %(Hcont1 & ? & -> & Hrest).
-    iDestruct (big_sepL2_length with "Hpush") as %Hpushlength.
-    destruct (contiguous_2 a_push) as (push1 & push2 & -> & Ha12); auto.
-    { rewrite contiguous_iff_contiguous_between; eauto. }
-    assert (push1 = i) as ->. { inversion Hcont1; auto. }
-    iExists a', push2, a_rest. iFrame. iPureIntro. repeat split; eauto.
-    cbn in Hrest. revert Ha12 Hrest; clear. solve_addr.
-  Qed.
-
-  Lemma push_r_instrs_extract a i j r prog p' :
-    contiguous_between a i j →
-    ([∗ list] a_i;w_i ∈ a; (push_r_instrs r_stk r ++ prog), a_i ↦ₐ[p'] w_i) -∗
-    ∃ a' push2 a_rest,
-      (([∗ list] a_i;w_i ∈ [i; push2];push_r_instrs r_stk r, a_i ↦ₐ[p'] w_i) ∗
-       [∗ list] a_i;w_i ∈ a'; prog, a_i ↦ₐ[p'] w_i) ∗
-       ⌜ a = [i; push2] ++ a'
-         ∧ (i + 1 = Some push2)%a
-         ∧ (push2 + 1 = Some a_rest)%a
-         ∧ contiguous_between a' a_rest j ⌝.
-  Proof.
-    intros. iIntros "HH".
-    iDestruct (contiguous_between_program_split with "HH") as (a_push a' a_rest) "(Hpush & ? & #Hcont)"; eauto.
-    iDestruct "Hcont" as %(Hcont1 & ? & -> & Hrest).
-    iDestruct (big_sepL2_length with "Hpush") as %Hpushlength.
-    destruct (contiguous_2 a_push) as (push1 & push2 & -> & Ha12); auto.
-    { rewrite contiguous_iff_contiguous_between; eauto. }
-    assert (push1 = i) as ->. { inversion Hcont1; auto. }
-    iExists a', push2, a_rest. iFrame. iPureIntro. repeat split; eauto.
-    cbn in Hrest. revert Ha12 Hrest; clear. solve_addr.
-  Qed.
   
-  (* -------------------------------------- POP -------------------------------------- *)
-  Definition pop_instrs r_stk r := [load_r r r_stk; sub_z_z r_t1 0 1; lea_r r_stk r_t1].
-
-  Definition pop (a1 a2 a3 : Addr) (p : Perm) (r_stk r : RegName) : iProp Σ :=
-    ([∗ list] a;i ∈ [a1;a2;a3];(pop_instrs r_stk r), a ↦ₐ[p] i)%I.
-
-  Lemma pop_spec a1 a2 a3 a4 r w w' wt1 p p' g b e stk_b stk_e stk_a stk_a' φ :
-    isCorrectPC (inr ((p,g),b,e,a1)) ∧ isCorrectPC (inr ((p,g),b,e,a2)) ∧
-    isCorrectPC (inr ((p,g),b,e,a3)) →
-    PermFlows p p' ->
-    withinBounds ((RWLX,Local),stk_b,stk_e,stk_a) = true →
-    r ≠ PC →
-    (a1 + 1)%a = Some a2 →
-    (a2 + 1)%a = Some a3 →
-    (a3 + 1)%a = Some a4 →
-    (stk_a + (-1))%a = Some stk_a' →
-
-      ▷ pop a1 a2 a3 p' r_stk r
-    ∗ ▷ PC ↦ᵣ inr ((p,g),b,e,a1)
-    ∗ ▷ r_stk ↦ᵣ inr ((RWLX,Local),stk_b,stk_e,stk_a)
-    ∗ ▷ stk_a ↦ₐ[RWLX] w
-    ∗ ▷ r_t1 ↦ᵣ wt1
-    ∗ ▷ r ↦ᵣ w'
-    ∗ ▷ (PC ↦ᵣ inr ((p,g),b,e,a4)
-            ∗ pop a1 a2 a3 p' r_stk r
-            ∗ r ↦ᵣ w
-            ∗ stk_a ↦ₐ[RWLX] w
-            ∗ r_stk ↦ᵣ inr ((RWLX,Local),stk_b,stk_e,stk_a')
-            ∗ r_t1 ↦ᵣ (inl (-1)%Z)
-            -∗ WP Seq (Instr Executable) {{ φ }})
-    ⊢
-    WP Seq (Instr Executable) {{ φ }}.
-  Proof.
-    iIntros ((Hvpc1 & Hvpc2 & Hvpc3) Hfl Hwb Hne Ha1' Ha2' Ha3' Hstk_a')
-            "((>Ha1 & >Ha2 & >Ha3 & _) & >HPC & >Hr_stk & >Hstk_a & >Hr_t1 & >Hr & Hφ)".
-    iApply (wp_bind (fill [SeqCtx])).
-    iAssert (⌜(stk_a =? a1)%a = false⌝)%I as %Hne'.
-    { rewrite Z.eqb_neq. iIntros (Hcontr); apply z_of_eq in Hcontr; subst.
-      iApply (cap_duplicate_false with "[$Ha1 $Hstk_a]").
-      split; auto. destruct p'; auto. destruct p; inversion Hfl. 
-      inversion Hvpc1 as [?????? [Hcontr | [Hcontr | Hcontr] ] ];inversion Hcontr. }
-    iApply (wp_load_success _ _ _ _ _ _ _ a1 _ _ _ RWLX
-              with "[HPC Ha1 Hr_stk Hr Hstk_a]");
-      eauto; first apply decode_encode_instrW_inv; rewrite Hne'; iFrame.
-    iPureIntro. eapply PermFlows_refl.
-    iNext. iIntros "(HPC & Hr & Ha1 & Hr_stk & Hstk_a) /=".
-    iApply wp_pure_step_later; auto; iNext.
-    iApply (wp_bind (fill [SeqCtx])).
-    iApply (wp_add_sub_lt_success_z_z _ r_t1 _ _ _ _ a2 with "[HPC Ha2 Hr_t1]");
-      try iFrame; first apply decode_encode_instrW_inv; eauto.
-    iNext.
-    (* rewrite sub_z_z_i Ha2'. *)
-    iIntros "(HPC & Ha2 & Hr_t1) /=".
-    iApply wp_pure_step_later; auto; iNext.
-    iApply (wp_bind (fill [SeqCtx])).
-    iApply (wp_lea_success_reg _ _ _ _ _ a3 a4 _ r_stk _ RWLX
-              with "[HPC Ha3 Hr_stk Hr_t1]"); eauto; first apply decode_encode_instrW_inv; iFrame.
-    iNext. iIntros "(HPC & Ha3 & Hr_t1 & Hr_stk) /=".
-    iApply wp_pure_step_later; auto; iNext.
-    iApply "Hφ". iFrame. done.
-  Qed.
-
   (* -------------------------------------- RCLEAR ----------------------------------- *)
   (* the following macro clears registers in r. a denotes the list of addresses
      containing the instructions for the clear: |a| = |r| *)
@@ -849,25 +625,24 @@ Section stack_macros.
   Lemma rclear_instrs_cons rr r: rclear_instrs (rr :: r) = move_z rr 0 :: rclear_instrs r.
   Proof. reflexivity. Qed.
 
-  Definition rclear (a : list Addr) (p : Perm) (r : list RegName) : iProp Σ :=
-      ([∗ list] k↦a_i;w_i ∈ a;(rclear_instrs r), a_i ↦ₐ[p] w_i)%I.
+  Definition rclear (a : list Addr) (r : list RegName) : iProp Σ :=
+      ([∗ list] k↦a_i;w_i ∈ a;(rclear_instrs r), a_i ↦ₐ w_i)%I.
 
-  Lemma rclear_spec (a : list Addr) (r: list RegName) (rmap : gmap RegName Word) p p' g b e a1 an φ :
+  Lemma rclear_spec (a : list Addr) (r: list RegName) (rmap : gmap RegName Word) p b e a1 an φ :
     contiguous_between a a1 an →
     ¬ PC ∈ r → hd_error a = Some a1 →
-    isCorrectPC_range p g b e a1 an →
-    PermFlows p p' →
+    isCorrectPC_range p b e a1 an →
     list_to_set r = dom (gset RegName) rmap →
 
       ▷ ([∗ map] r_i↦w_i ∈ rmap, r_i ↦ᵣ w_i)
-    ∗ ▷ PC ↦ᵣ inr ((p,g),b,e,a1)
-    ∗ ▷ rclear a p' r
-    ∗ ▷ (PC ↦ᵣ inr ((p,g),b,e,an) ∗ ([∗ map] r_i↦_ ∈ rmap, r_i ↦ᵣ inl 0%Z)
-            ∗ rclear a p' r -∗
+    ∗ ▷ PC ↦ᵣ inr (p,b,e,a1)
+    ∗ ▷ rclear a r
+    ∗ ▷ (PC ↦ᵣ inr (p,b,e,an) ∗ ([∗ map] r_i↦_ ∈ rmap, r_i ↦ᵣ inl 0%Z)
+            ∗ rclear a r -∗
             WP Seq (Instr Executable) {{ φ }})
     ⊢ WP Seq (Instr Executable) {{ φ }}.
   Proof.
-    iIntros (Ha Hne Hhd Hvpc Hfl Hrdom) "(>Hreg & >HPC & >Hrclear & Hφ)".
+    iIntros (Ha Hne Hhd Hvpc Hrdom) "(>Hreg & >HPC & >Hrclear & Hφ)".
     iDestruct (big_sepL2_length with "Hrclear") as %Har.
     iRevert (Hne Har Hhd Hvpc Ha Hrdom).
     iInduction (a) as [| a1'] "IH" forall (r rmap a1 an).
@@ -883,8 +658,7 @@ Section stack_macros.
     iDestruct (big_sepM_delete _ _ r with "Hreg") as "[Hr Hreg]". eauto.
     pose proof (contiguous_between_cons_inv _ _ _ _ Ha) as [-> [a2 [? Hcont'] ] ].
     iApply (wp_move_success_z with "[$HPC $Hr $Ha1]");
-      [apply decode_encode_instrW_inv|apply Hfl|iCorrectPC a1 an|eauto|..].
-    { apply (not_elem_of_cons) in Hne as [Hne _]. apply Hne. }
+      [apply decode_encode_instrW_inv|iCorrectPC a1 an|eauto|..].
     iNext. iIntros "(HPC & Ha1 & Hr)". iApply wp_pure_step_later; auto. iNext.
     destruct a.
     { iApply "Hφ". iFrame. inversion Hcont'; subst. iFrame.
@@ -950,63 +724,61 @@ Section stack_macros.
       move_z r_t6 0].
 
   (* Next we define mclear in memory, using a list of addresses of size 23 *)
-  Definition mclear (a : list Addr) (p : Perm) (r : RegName) : iProp Σ :=
+  Definition mclear (a : list Addr) (r : RegName) : iProp Σ :=
     if ((length a) =? (length (mclear_instrs r)))%nat then
-      ([∗ list] k↦a_i;w_i ∈ a;(mclear_instrs r), a_i ↦ₐ[p] w_i)%I
+      ([∗ list] k↦a_i;w_i ∈ a;(mclear_instrs r), a_i ↦ₐ w_i)%I
     else
       False%I.
 
   Lemma mclear_iter_spec (a1 a2 a3 a4 a5 a6 b_r e_r a_r (* e_r' *) : Addr) ws (z : nat)
-        p p' g b e rt rt1 rt2 rt3 rt4 rt5 a_end (p_r p_r' : Perm) (g_r : Locality) φ :
-        isCorrectPC (inr ((p,g),b,e,a1))
-      ∧ isCorrectPC (inr ((p,g),b,e,a2))
-      ∧ isCorrectPC (inr ((p,g),b,e,a3))
-      ∧ isCorrectPC (inr ((p,g),b,e,a4))
-      ∧ isCorrectPC (inr ((p,g),b,e,a5))
-      ∧ isCorrectPC (inr ((p,g),b,e,a6)) →
+        p b e rt rt1 rt2 rt3 rt4 rt5 a_end (p_r : Perm) φ :
+        isCorrectPC (inr (p,b,e,a1))
+      ∧ isCorrectPC (inr (p,b,e,a2))
+      ∧ isCorrectPC (inr (p,b,e,a3))
+      ∧ isCorrectPC (inr (p,b,e,a4))
+      ∧ isCorrectPC (inr (p,b,e,a5))
+      ∧ isCorrectPC (inr (p,b,e,a6)) →
         (a1 + 1)%a = Some a2
       ∧ (a2 + 1)%a = Some a3
       ∧ (a3 + 1)%a = Some a4
       ∧ (a4 + 1)%a = Some a5
       ∧ (a5 + 1)%a = Some a6 →
-        ((b_r + z < e_r)%Z → withinBounds ((p_r,g_r),b_r,e_r,a_r) = true) →
+        ((b_r + z < e_r)%Z → withinBounds (p_r,b_r,e_r,a_r) = true) →
         writeAllowed p_r = true →
         (* (e_r + 1)%a = Some e_r' → *)
         (b_r + z)%a = Some a_r →
-        PermFlows p p' ->
-        PermFlows p_r p_r' ->
-      ([[a_r,e_r]] ↦ₐ[p_r'] [[ws]]
-     ∗ ▷ PC ↦ᵣ inr ((p,g),b,e,a1)
-     ∗ ▷ rt ↦ᵣ inr ((p_r,g_r),b_r,e_r,a_r)
+      ([[a_r,e_r]] ↦ₐ [[ws]]
+     ∗ ▷ PC ↦ᵣ inr (p,b,e,a1)
+     ∗ ▷ rt ↦ᵣ inr (p_r,b_r,e_r,a_r)
      ∗ ▷ rt1 ↦ᵣ inl (b_r + z)%Z
      ∗ ▷ rt2 ↦ᵣ inl ((z_of e_r) - 1)%Z
      ∗ ▷ (∃ w, rt3 ↦ᵣ w)
-     ∗ ▷ rt4 ↦ᵣ inr (p, g, b, e, a_end)
-     ∗ ▷ rt5 ↦ᵣ inr (p, g, b, e, a1)
+     ∗ ▷ rt4 ↦ᵣ inr (p, b, e, a_end)
+     ∗ ▷ rt5 ↦ᵣ inr (p, b, e, a1)
      ∗ ▷ ([∗ list] a_i;w_i ∈ [a1;a2;a3;a4;a5;a6];[lt_r_r rt3 rt2 rt1;
                                                   jnz rt4 rt3;
                                                   store_z rt 0;
                                                   lea_z rt 1;
                                                   add_r_z rt1 rt1 1;
-                                                  jmp rt5], a_i ↦ₐ[p'] w_i)
-     ∗ ▷ (PC ↦ᵣ updatePcPerm (inr ((p,g),b,e,a_end))
-             ∗ [[ a_r , e_r ]] ↦ₐ[p_r'] [[ region_addrs_zeroes a_r e_r ]]
-             ∗ (∃ a_r, rt ↦ᵣ inr (p_r, g_r, b_r, e_r, a_r))
-             ∗ rt5 ↦ᵣ inr (p, g, b, e, a1)
-             ∗ a3 ↦ₐ[p'] store_z rt 0
-             ∗ a4 ↦ₐ[p'] lea_z rt 1
-             ∗ a5 ↦ₐ[p'] add_r_z rt1 rt1 1
-             ∗ a6 ↦ₐ[p'] jmp rt5
-             ∗ a1 ↦ₐ[p'] lt_r_r rt3 rt2 rt1
+                                                  jmp rt5], a_i ↦ₐ w_i)
+     ∗ ▷ (PC ↦ᵣ updatePcPerm (inr (p,b,e,a_end))
+             ∗ [[ a_r , e_r ]] ↦ₐ [[ region_addrs_zeroes a_r e_r ]]
+             ∗ (∃ a_r, rt ↦ᵣ inr (p_r, b_r, e_r, a_r))
+             ∗ rt5 ↦ᵣ inr (p, b, e, a1)
+             ∗ a3 ↦ₐ store_z rt 0
+             ∗ a4 ↦ₐ lea_z rt 1
+             ∗ a5 ↦ₐ add_r_z rt1 rt1 1
+             ∗ a6 ↦ₐ jmp rt5
+             ∗ a1 ↦ₐ lt_r_r rt3 rt2 rt1
              ∗ rt2 ↦ᵣ inl ((z_of e_r) - 1)%Z
              ∗ (∃ z, rt1 ↦ᵣ inl (b_r + z)%Z)
-             ∗ a2 ↦ₐ[p'] jnz rt4 rt3
-             ∗ rt4 ↦ᵣ inr (p, g, b, e, a_end)
+             ∗ a2 ↦ₐ jnz rt4 rt3
+             ∗ rt4 ↦ᵣ inr (p, b, e, a_end)
              ∗ rt3 ↦ᵣ inl 1%Z
               -∗ WP Seq (Instr Executable) {{ φ }})
      ⊢ WP Seq (Instr Executable) {{ φ }})%I.
   Proof.
-    iIntros (Hvpc Hnext Hwb Hwa (* Her' *) Hprogress Hfl1 Hfl2)
+    iIntros (Hvpc Hnext Hwb Hwa (* Her' *) Hprogress)
             "(Hbe & >HPC & >Hrt & >Hr_t1 & >Hr_t2 & >Hr_t3 & >Hr_t4 & >Hr_t5 & >Hprog & Hφ)".
     iRevert (Hwb Hprogress).
     iLöb as "IH" forall (a_r ws z).
@@ -1032,8 +804,8 @@ Section stack_macros.
     (* lt rt3 rt2 rt1 *)
     iDestruct "Hprog" as "[Hi Hprog]".
     iApply (wp_bind (fill [SeqCtx])).
-    iApply (wp_add_sub_lt_success_r_r _ rt3 _ _ _ _ a1 _ _ _ rt2 _ rt1 _ _
-      with "[Hi HPC Hr_t3 Hr_t1 Hr_t2]"); [apply decode_encode_instrW_inv | | | apply Hfl1 | ..]; eauto.
+    iApply (wp_add_sub_lt_success_r_r _ rt3 _ _ _ a1 _ _ _ rt2 _ rt1 _ _
+      with "[Hi HPC Hr_t3 Hr_t1 Hr_t2]"); [apply decode_encode_instrW_inv | | | ..]; eauto.
     iFrame.
     iEpilogue "(HPC & Ha1 & Hr_t2 & Hr_t1 & Hr_t3)".
     rewrite /region_mapsto /region_addrs.
@@ -1045,8 +817,8 @@ Section stack_macros.
       (* jnz rt4 rt3 *)
       iDestruct "Hprog" as "[Hi Hprog]".
       iApply (wp_bind (fill [SeqCtx])).
-      iApply (wp_jnz_success_next _ rt4 rt3 _ _ _ _ a2 a3 with "[HPC Hi Hr_t3 Hr_t4]");
-        first apply decode_encode_instrW_inv; first apply Hfl1;eauto.
+      iApply (wp_jnz_success_next _ rt4 rt3 _ _ _ a2 a3 with "[HPC Hi Hr_t3 Hr_t4]");
+        first apply decode_encode_instrW_inv; eauto.
       iFrame. iEpilogue "(HPC & Ha2 & Hr_t4 & Hr_t3)".
       (* store rt 0 *)
       rewrite/ withinBounds in Hwb.
@@ -1056,7 +828,7 @@ Section stack_macros.
       iDestruct "Hbe" as "[Ha_r Hbe]".
       iDestruct "Hprog" as "[Hi Hprog]".
       iApply (wp_bind (fill [SeqCtx])).
-      iApply (wp_store_success_z _ _ _ _ _ a3 a4 _ rt 0 _ p_r g_r b_r e_r a_r with "[HPC Hi Hrt Ha_r]"); first apply decode_encode_instrW_inv; first apply Hfl1; eauto.
+      iApply (wp_store_success_z _ _ _ _  a3 a4 _ rt 0 _ p_r b_r e_r a_r with "[HPC Hi Hrt Ha_r]"); first apply decode_encode_instrW_inv; eauto.
       { split;[auto|]. rewrite /withinBounds andb_true_iff; split;[auto|].
           by apply Z.leb_le. by apply Z.ltb_lt. }
       iFrame. iEpilogue "(HPC & Ha3 & Hrt & Ha_r)".
@@ -1065,29 +837,28 @@ Section stack_macros.
       { apply addr_next_lt with e_r. apply incr_addr_of_z_i in Hprogress. lia. }
       iDestruct "Hprog" as "[Hi Hprog]".
       iApply (wp_bind (fill [SeqCtx])).
-      iApply (wp_lea_success_z _ _ _ _ _ a4 a5 _ rt p_r _ _ _ a_r 1 a_r' with "[HPC Hi Hrt]"); first apply decode_encode_instrW_inv; first apply Hfl1; eauto.
+      iApply (wp_lea_success_z _ _ _ _ a4 a5 _ rt p_r _ _ a_r 1 a_r' with "[HPC Hi Hrt]"); first apply decode_encode_instrW_inv; eauto.
       { destruct p_r; auto. }
-      { destruct p_r;inversion Hwa;auto. }
       iFrame. iEpilogue "(HPC & Ha4 & Hrt)".
       (* add rt1 rt1 1 *)
       iDestruct "Hprog" as "[Hi Hprog]".
       iApply (wp_bind (fill [SeqCtx])).
-      iApply (wp_add_sub_lt_success_dst_z _ rt1 _ _ _ _ a5 _ _ _ with "[HPC Hi Hr_t1]"); try iFrame;
-        [ apply decode_encode_instrW_inv | | | apply Hfl1 | ..]; eauto.
+      iApply (wp_add_sub_lt_success_dst_z _ rt1 _ _ _ a5 _ _ _ with "[HPC Hi Hr_t1]"); try iFrame;
+        [ apply decode_encode_instrW_inv | | |..]; eauto.
       iEpilogue "(HPC & Ha5 & Hr_t1)".
       (* jmp rt5 *)
       iDestruct "Hprog" as "[Hi _]".
       iApply (wp_bind (fill [SeqCtx])).
-      iApply (wp_jmp_success _ _ _ _ _ a6 with "[HPC Hi Hr_t5]");
-        first apply decode_encode_instrW_inv; first apply Hfl1; eauto.
+      iApply (wp_jmp_success _ _ _ _ a6 with "[HPC Hi Hr_t5]");
+        first apply decode_encode_instrW_inv; eauto.
       iFrame. iEpilogue "(HPC & Ha6 & Hr_t5)".
       iApply ("IH" $! a_r' ws (z + 1)%nat with
                   "[Hbe] [HPC] [Hrt] [Hr_t1] [Hr_t2] [Hr_t3] [Hr_t4] [Hr_t5] [Ha1 Ha2 Ha3 Ha4 Ha5 Ha6] [Hφ Ha_r]")
       ; iFrame. all: auto.
       + by rewrite Ha_r'.
-      + assert (updatePcPerm (inr (p, g, b, e, a1)) = (inr (p, g, b, e, a1))).
+      + assert (updatePcPerm (inr (p, b, e, a1)) = (inr (p, b, e, a1))).
         { rewrite /updatePcPerm. destruct p; auto.
-          inversion Hvpc1; destruct H5 as [Hc | [Hc | Hc] ]; inversion Hc. }
+          inversion Hvpc1; destruct H4 as [Hc | Hc ]; inversion Hc. }
         rewrite H. iFrame.
       + cbn. assert (b_r + z + 1 = b_r + (z + 1)%nat)%Z as ->;[lia|]. iFrame.
       + iNext.
@@ -1112,7 +883,7 @@ Section stack_macros.
       (* jnz *)
       iDestruct "Hprog" as "[Hi Hprog]".
       iApply (wp_bind (fill [SeqCtx])).
-      iApply (wp_jnz_success_jmp _ rt4 rt3 _ _ _ _ a2 _ _ (inl 1%Z) with "[HPC Hi Hr_t3 Hr_t4]"); first apply decode_encode_instrW_inv; first apply Hfl1; eauto.
+      iApply (wp_jnz_success_jmp _ rt4 rt3 _ _ _ a2 _ _ (inl 1%Z) with "[HPC Hi Hr_t3 Hr_t4]"); first apply decode_encode_instrW_inv; eauto.
       iFrame. iEpilogue "(HPC & Ha2 & Hr_t4 & Hr_t3)".
       iApply "Hφ". iDestruct "Hprog" as "(Ha3 & Ha4 & Ha5 & Ha6 & _)".
       rewrite /region_addrs_zeroes region_size_0 //=. iFrame.
@@ -1120,43 +891,42 @@ Section stack_macros.
   Qed.
 
   Lemma mclear_spec (a : list Addr) (r : RegName)
-        (a_first a6' a_end : Addr) p p' g b e p_r p_r' g_r (b_r e_r a_r : Addr) a'
+        (a_first a6' a_end : Addr) p b e p_r (b_r e_r a_r : Addr) a'
         w1 w2 w3 w4 w5 w6 ws φ :
     contiguous_between a a_first a' →
     (* We will assume that we are not trying to clear memory in a *)
     r ≠ PC ∧ writeAllowed p_r = true →
     (a !! 7 = Some a6' ∧ (a6' + 10)%a = Some a_end ∧ a !! 17 = Some a_end) →
 
-    isCorrectPC_range p g b e a_first a' →
-    PermFlows p p' → PermFlows p_r p_r' ->
+    isCorrectPC_range p b e a_first a' →
 
     (* We will also assume the region to clear is non empty *)
     (b_r ≤ e_r)%Z →
 
-     (mclear a p' r
-    ∗ ▷ PC ↦ᵣ inr ((p,g),b,e,a_first)
-    ∗ ▷ r ↦ᵣ inr ((p_r,g_r),b_r,e_r,a_r)
+     (mclear a r
+    ∗ ▷ PC ↦ᵣ inr (p,b,e,a_first)
+    ∗ ▷ r ↦ᵣ inr (p_r,b_r,e_r,a_r)
     ∗ ▷ r_t4 ↦ᵣ w4
     ∗ ▷ r_t1 ↦ᵣ w1
     ∗ ▷ r_t2 ↦ᵣ w2
     ∗ ▷ r_t3 ↦ᵣ w3
     ∗ ▷ r_t5 ↦ᵣ w5
     ∗ ▷ r_t6 ↦ᵣ w6
-    ∗ ▷ ([[ b_r , e_r ]] ↦ₐ[p_r'] [[ ws ]])
-    ∗ ▷ (PC ↦ᵣ inr ((p,g),b,e,a')
+    ∗ ▷ ([[ b_r , e_r ]] ↦ₐ [[ ws ]])
+    ∗ ▷ (PC ↦ᵣ inr (p,b,e,a')
             ∗ r_t1 ↦ᵣ inl 0%Z
             ∗ r_t2 ↦ᵣ inl 0%Z
             ∗ r_t3 ↦ᵣ inl 0%Z
             ∗ r_t4 ↦ᵣ inl 0%Z
             ∗ r_t5 ↦ᵣ inl 0%Z
             ∗ r_t6 ↦ᵣ inl 0%Z
-            ∗ r ↦ᵣ inr ((p_r,g_r),b_r,e_r,a_r)
-            ∗ [[ b_r , e_r ]] ↦ₐ[p_r'] [[region_addrs_zeroes b_r e_r]]
-            ∗ mclear a p' r -∗
+            ∗ r ↦ᵣ inr (p_r,b_r,e_r,a_r)
+            ∗ [[ b_r , e_r ]] ↦ₐ [[region_addrs_zeroes b_r e_r]]
+            ∗ mclear a r -∗
             WP Seq (Instr Executable) {{ φ }})
     ⊢ WP Seq (Instr Executable) {{ φ }})%I.
   Proof.
-    iIntros (Hnext [Hne Hwa] Hjnz_off Hvpc Hfl1 Hfl2 Hle)
+    iIntros (Hnext [Hne Hwa] Hjnz_off Hvpc Hle)
             "(Hmclear & >HPC & >Hr & >Hr_t4 & >Hr_t1 & >Hr_t2 & >Hr_t3 & >Hr_t5 & >Hr_t6 & >Hregion & Hφ)".
     iAssert (⌜((length a) =? (length (mclear_instrs r)) = true)%nat⌝)%I as %Hlen.
     { destruct (((length a) =? (length (mclear_instrs r)))%nat) eqn:Hlen; auto.
@@ -1166,22 +936,22 @@ Section stack_macros.
     move: (contiguous_between_cons_inv_first _ _ _ _ Hnext).
     match goal with |- (?a = _) -> _ => intro; subst a end.
     iPrologue "Hmclear".
-    iApply (wp_move_success_reg _ _ _ _ _ a_first _ _ r_t4 _ r with "[HPC Hr Hr_t4 Hi]");
-      first apply decode_encode_instrW_inv; first apply Hfl1; first iCorrectPC a_first a'; eauto.
+    iApply (wp_move_success_reg _ _ _ _ a_first _ _ r_t4 _ r with "[HPC Hr Hr_t4 Hi]");
+      first apply decode_encode_instrW_inv; first iCorrectPC a_first a'; eauto.
     { iContiguous_next Hnext 0. }
     iFrame. iEpilogue "(HPC & Ha_first & Hr_t4 & Hr)".
     (* getb r_t1 r_t4 *)
     iPrologue "Hprog".
-    iApply (wp_Get_success _ _ r_t1 r_t4 _ _ _ _ a0 _ _ _ a1 with "[$HPC $Hi $Hr_t1 $Hr_t4]");
-      first eapply decode_encode_instrW_inv; first eauto; first apply Hfl1; first iCorrectPC a_first a'; eauto.
+    iApply (wp_Get_success _ _ r_t1 r_t4 _ _ _ a0 _ _ _ a1 with "[$HPC $Hi $Hr_t1 $Hr_t4]");
+      first eapply decode_encode_instrW_inv; first eauto; first iCorrectPC a_first a'; eauto.
     { iContiguous_next Hnext 1. }
     iFrame. iEpilogue "(HPC & Ha0 & Hr_t4 & Hr_t1)".
     destruct (reg_eq_dec PC r_t4) as [Hcontr | _]; [inversion Hcontr|].
     iCombine "Ha0 Ha_first" as "Hprog_done".
     (* geta r_t2 r_t4 *)
     iPrologue "Hprog".
-    iApply (wp_Get_success _ _ r_t2 r_t4 _ _ _ _ a1 _ _ _ a2 with "[HPC Hi Hr_t2 Hr_t4]");
-      first eapply decode_encode_instrW_inv; first eauto; first eapply Hfl1; first iCorrectPC a_first a'; auto.
+    iApply (wp_Get_success _ _ r_t2 r_t4 _ _ _ a1 _ _ _ a2 with "[HPC Hi Hr_t2 Hr_t4]");
+      first eapply decode_encode_instrW_inv; first eauto; first iCorrectPC a_first a'; auto.
     { iContiguous_next Hnext 2. }
     iFrame. iEpilogue "(HPC & Ha1 & Hr_t4 & Hr_t2)".
     destruct (reg_eq_dec PC r_t4) as [Hcontr | _]; [inversion Hcontr|].
@@ -1189,8 +959,8 @@ Section stack_macros.
     (* sub r_t2 r_t1 r_t2 *)
     iPrologue "Hprog".
     (* destruct b_r eqn:Hb_r. *)
-    iApply (wp_add_sub_lt_success_r_dst _ _ _ _ _ _ a2 _ _ r_t1 with "[HPC Hi Hr_t1 Hr_t2]"); try iFrame;
-      [ apply decode_encode_instrW_inv | | | apply Hfl1 | ..]; eauto. 2: by iCorrectPC a_first a'.
+    iApply (wp_add_sub_lt_success_r_dst _ _ _ _ _ a2 _ _ r_t1 with "[HPC Hi Hr_t1 Hr_t2]"); try iFrame;
+      [ apply decode_encode_instrW_inv | | |..]; eauto. 2: by iCorrectPC a_first a'.
     assert ((a2 + 1) = Some a3)%a as ->. { iContiguous_next Hnext 3. } by eauto.
     iEpilogue "(HPC & Ha2 & Hr_t1 & Hr_t2)".
     iCombine "Ha2 Hprog_done" as "Hprog_done".
@@ -1198,17 +968,16 @@ Section stack_macros.
     iPrologue "Hprog".
     assert (a_r + (b_r - a_r) = b_r)%Z as Haddmin; first lia.
     assert ((a_r + (b_r - a_r))%a = Some b_r) as Ha_rb_r by solve_addr.
-    iApply (wp_lea_success_reg _ _ _ _ _ a3 a4 _ r_t4 r_t2 p_r _ _ _ a_r (b_r - a_r) with "[HPC Hi Hr_t4 Hr_t2]");
-      first apply decode_encode_instrW_inv; first apply Hfl1; first iCorrectPC a_first a'; eauto.
+    iApply (wp_lea_success_reg _ _ _ _ a3 a4 _ r_t4 r_t2 p_r _ _ a_r (b_r - a_r) with "[HPC Hi Hr_t4 Hr_t2]");
+      first apply decode_encode_instrW_inv; first iCorrectPC a_first a'; eauto.
     { iContiguous_next Hnext 4. }
-    { destruct p_r; inversion Hwa; auto. }
     { destruct p_r; inversion Hwa; auto. }
     by iFrame. iEpilogue "(HPC & Ha3 & Hr_t2 & Hr_t4)".
     iCombine "Ha3 Hprog_done" as "Hprog_done".
     (* gete r_t2 r_t4 *)
     iPrologue "Hprog".
-    iApply (wp_Get_success _ _ r_t5 r_t4 _ _ _ _ a4 _ _ _ a5 with "[HPC Hi Hr_t5 Hr_t4]"); try iFrame;
-      first apply decode_encode_instrW_inv; first eauto; first apply Hfl1; first iCorrectPC a_first a'; eauto.
+    iApply (wp_Get_success _ _ r_t5 r_t4 _ _ _ a4 _ _ _ a5 with "[HPC Hi Hr_t5 Hr_t4]"); try iFrame;
+      first apply decode_encode_instrW_inv; first eauto; first iCorrectPC a_first a'; eauto.
     { iContiguous_next Hnext 5. }
     destruct (reg_eq_dec PC r_t4) as [Hcontr | _]; [inversion Hcontr|].
     destruct (reg_eq_dec r_t4 r_t5) as [Hcontr | _]; [inversion Hcontr|].
@@ -1217,54 +986,45 @@ Section stack_macros.
     (* sub r_t5 r_t5 1 *)
     iPrologue "Hprog".
     iApply (wp_add_sub_lt_success_dst_z with "[$HPC $Hi Hr_t5]");
-      [apply decode_encode_instrW_inv| | | apply Hfl1|iCorrectPC a_first a'|..]; eauto.
+      [apply decode_encode_instrW_inv| | |iCorrectPC a_first a'|..]; eauto.
     assert ((a5 + 1)%a = Some a6) as ->. { iContiguous_next Hnext 6. } eauto.
     iEpilogue "(HPC & Ha5 & Hr_t5)".
     iCombine "Ha5 Hprog_done" as "Hprog_done".
     (* move r_t2 PC *)
     iPrologue "Hprog".
-    iApply (wp_move_success_reg_fromPC _ _ _ _ _ a6 a7 _ r_t2 with "[HPC Hi Hr_t2]");
-      first apply decode_encode_instrW_inv; first apply Hfl1; first iCorrectPC a_first a'; eauto.
+    iApply (wp_move_success_reg_fromPC _ _ _ _ a6 a7 _ r_t2 with "[HPC Hi Hr_t2]");
+      first apply decode_encode_instrW_inv; first iCorrectPC a_first a'; eauto.
     { iContiguous_next Hnext 7. }
     iFrame. iEpilogue "(HPC & Ha6 & Hr_t2)".
     iCombine "Ha6 Hprog_done" as "Hprog_done".
     (* lea r_t2 mclear_off_end *)
     iPrologue "Hprog".
     assert (p ≠ E) as Hpne.
-    { have: (isCorrectPC (inr (p, g, b, e, a_first))).
+    { have: (isCorrectPC (inr (p, b, e, a_first))).
       { apply Hvpc. eapply contiguous_between_middle_bounds'; eauto. constructor. }
       inversion 1; subst.
-      destruct H15 as [? | [? | ?] ]; subst; auto. }
-    iApply (wp_lea_success_z _ _ _ _ _ a7 a8 _ r_t2 p _ _ _ a6 10 a_end with "[HPC Hi Hr_t2]");
-      first apply decode_encode_instrW_inv; first apply Hfl1; first iCorrectPC a_first a'; auto.
+      destruct H14 as [? | ? ]; subst; auto. }
+    iApply (wp_lea_success_z _ _ _ _ a7 a8 _ r_t2 p _ _ a6 10 a_end with "[HPC Hi Hr_t2]");
+      first apply decode_encode_instrW_inv; first iCorrectPC a_first a'; auto.
     { iContiguous_next Hnext 8. }
     { destruct Hjnz_off as (Ha7' & Hmclear_off_end & Ha_end). simpl in Ha7'. congruence. }
-    { have: (isCorrectPC (inr (p, g, b, e, a_first))).
-      { apply Hvpc. eapply contiguous_between_middle_bounds'; eauto. constructor. }
-      inversion 1; subst.
-      destruct H15 as [? | [? | ?] ]; subst; auto.
-    }
     iFrame. iEpilogue "(HPC & Ha7 & Hr_t2)".
     iCombine "Ha7 Hprog_done" as "Hprog_done".
     (* move r_t3 PC *)
     iPrologue "Hprog".
-    iApply (wp_move_success_reg_fromPC _ _ _ _ _ a8 a9 _ r_t3 with "[HPC Hi Hr_t3]");
-      first apply decode_encode_instrW_inv; first apply Hfl1; first iCorrectPC a_first a'; auto.
+    iApply (wp_move_success_reg_fromPC _ _ _ _ a8 a9 _ r_t3 with "[HPC Hi Hr_t3]");
+      first apply decode_encode_instrW_inv; first iCorrectPC a_first a'; auto.
     { iContiguous_next Hnext 9. }
     iFrame. iEpilogue "(HPC & Ha8 & Hr_t3)".
     iCombine "Ha8 Hprog_done" as "Hprog_done".
     (* lea r_t3 mclear_off_iter *)
     iPrologue "Hprog".
-    iApply (wp_lea_success_z _ _ _ _ _ a9 a10 _ r_t3 p _ _ _ a8 2 a10 with "[HPC Hi Hr_t3]");
-      first apply decode_encode_instrW_inv; first apply Hfl1; first iCorrectPC a_first a'; auto.
+    iApply (wp_lea_success_z _ _ _ _ a9 a10 _ r_t3 p _ _ a8 2 a10 with "[HPC Hi Hr_t3]");
+      first apply decode_encode_instrW_inv; first iCorrectPC a_first a'; auto.
     { iContiguous_next Hnext 10. }
     { assert (2 = 1 + 1)%Z as ->; auto.
       apply incr_addr_trans with a9. iContiguous_next Hnext 9.
       iContiguous_next Hnext 10. }
-    { have: (isCorrectPC (inr (p, g, b, e, a_first))).
-      { apply Hvpc. eapply contiguous_between_middle_bounds'; eauto. constructor. }
-      inversion 1; subst.
-      destruct H17 as [? | [? | ?] ]; subst; auto. }
     iFrame. iEpilogue "(HPC & Ha9 & Hr_t3)".
     iCombine "Ha9 Hprog_done" as "Hprog_done".
     (* iter *)
@@ -1277,7 +1037,7 @@ Section stack_macros.
     iDestruct "Hprog" as "[Hi5 Hprog]".
     iDestruct "Hprog" as "[Hi6 Hprog]".
     iApply (mclear_iter_spec a10 a11 a12 a13 a14 a15 b_r e_r b_r _
-                        0 p p' g b e r_t4 r_t1 r_t5 r_t6 r_t2 r_t3 _ p_r p_r' g_r
+                        0 p b e r_t4 r_t1 r_t5 r_t6 r_t2 r_t3 _ p_r
               with "[-]"); auto.
     - repeat apply conj; iCorrectPC a_first a'.
     - repeat split; solve [
@@ -1307,44 +1067,44 @@ Section stack_macros.
         by inversion Hend.
       }
       destruct a as [| a17 a]; inversion Hlen.
-      iApply (wp_move_success_z _ _ _ _ _ a16 a17 _ r_t4 _ 0 with "[HPC Hi Hr_t4]");
-        first apply decode_encode_instrW_inv; first apply Hfl1;
+      iApply (wp_move_success_z _ _ _ _ a16 a17 _ r_t4 _ 0 with "[HPC Hi Hr_t4]");
+        first apply decode_encode_instrW_inv;
         first iCorrectPC a_first a'; auto.
       { iContiguous_next Hnext 17; auto. }
       { rewrite Ha16. destruct p; iFrame. contradiction. }
       iEpilogue "(HPC & Ha16 & Hr_t4)".
       (* move r_t1 0 *)
       iPrologue "Hprog".
-      iApply (wp_move_success_z _ _ _ _ _ a17 a18 _ r_t1 _ 0 with "[HPC Hi Hr_t1]");
-        first apply decode_encode_instrW_inv; first apply Hfl1;
+      iApply (wp_move_success_z _ _ _ _ a17 a18 _ r_t1 _ 0 with "[HPC Hi Hr_t1]");
+        first apply decode_encode_instrW_inv; 
         first iCorrectPC a_first a'; auto.
       { iContiguous_next Hnext 18. }
       iFrame. iEpilogue "(HPC & Ha17 & Hr_t1)".
       (* move r_t2 0 *)
       iPrologue "Hprog".
-      iApply (wp_move_success_z _ _ _ _ _ a18 a19 _ r_t2 _ 0 with "[HPC Hi Hr_t2]");
-        first apply decode_encode_instrW_inv; first apply Hfl1;
+      iApply (wp_move_success_z _ _ _ _ a18 a19 _ r_t2 _ 0 with "[HPC Hi Hr_t2]");
+        first apply decode_encode_instrW_inv;
         first iCorrectPC a_first a'; auto.
       { iContiguous_next Hnext 19. }
       iFrame. iEpilogue "(HPC & Ha18 & Hr_t2)".
       (* move r_t3 0 *)
       iPrologue "Hprog".
-      iApply (wp_move_success_z _ _ _ _ _ a19 a20 _ r_t3 _ 0 with "[HPC Hi Hr_t3]");
-        first apply decode_encode_instrW_inv; first apply Hfl1;
+      iApply (wp_move_success_z _ _ _ _ a19 a20 _ r_t3 _ 0 with "[HPC Hi Hr_t3]");
+        first apply decode_encode_instrW_inv;
         first iCorrectPC a_first a'; auto.
       { iContiguous_next Hnext 20. }
       iFrame. iEpilogue "(HPC & Ha19 & Hr_t3)".
       (* move r_t5 0 *)
       iPrologue "Hprog".
-      iApply (wp_move_success_z _ _ _ _ _ a20 a21 _ r_t5 _ 0 with "[HPC Hi Hr_t5]");
-        first apply decode_encode_instrW_inv; first apply Hfl1;
+      iApply (wp_move_success_z _ _ _ _ a20 a21 _ r_t5 _ 0 with "[HPC Hi Hr_t5]");
+        first apply decode_encode_instrW_inv; 
         first iCorrectPC a_first a'; auto.
       { iContiguous_next Hnext 21. }
       iFrame. iEpilogue "(HPC & Ha20 & Hr_t5)".
       (* move r_t6 0 *)
       iPrologue "Hprog".
-      iApply (wp_move_success_z _ _ _ _ _ a21 a' _ r_t6 _ 0 with "[HPC Hi Hr_t6]");
-        first apply decode_encode_instrW_inv; first apply Hfl1;
+      iApply (wp_move_success_z _ _ _ _ a21 a' _ r_t6 _ 0 with "[HPC Hi Hr_t6]");
+        first apply decode_encode_instrW_inv;
         first iCorrectPC a_first a'; auto.
       { eapply contiguous_between_last. eapply Hnext. reflexivity. }
       iFrame. iEpilogue "(HPC & Ha21 & Hr_t6)".
@@ -1355,38 +1115,27 @@ Section stack_macros.
   Qed.
 
 
-  (* -------------------------------------- REQGLOB ----------------------------------- *)
-  (* the following macro requires that a given registers contains a global capability. If 
-     this is not the case, the macro goes to fail, otherwise it continues               *)
-
-  Definition reqglob_instrs r :=
-    [getl r_t1 r;
-    sub_r_z r_t1 r_t1 (encodeLoc Global);
-    move_r r_t2 PC;
-    lea_z r_t2 6;
-    jnz r_t2 r_t1;
-    move_r r_t2 PC;
-    lea_z r_t2 4;
-    jmp r_t2;
-    fail_end;
-    move_z r_t1 0;
-    move_z r_t2 0].
+  
+  (* -------------------------------------- REQPERM ----------------------------------- *)
+  (* the following macro requires that a given registers contains a capability with a 
+     given (encoded) permission. If this is not the case, the macro goes to fail,
+     otherwise it continues *)  
 
   (* TODO: move this to the rules_Get.v file. small issue with the spec of failure: it does not actually 
      require/leave a trace on dst! It would be good if req_regs of a failing get does not include dst (if possible) *)
-  Lemma wp_Get_fail E get_i dst src pc_p pc_g pc_b pc_e pc_a w zsrc wdst pc_p' :
+  Lemma wp_Get_fail E get_i dst src pc_p pc_b pc_e pc_a w zsrc wdst :
     decodeInstrW w = get_i →
     is_Get get_i dst src →
-    PermFlows pc_p pc_p' → isCorrectPC (inr ((pc_p,pc_g),pc_b,pc_e,pc_a)) →
+    isCorrectPC (inr (pc_p,pc_b,pc_e,pc_a)) →
 
-    {{{ ▷ PC ↦ᵣ inr ((pc_p,pc_g),pc_b,pc_e,pc_a)
-      ∗ ▷ pc_a ↦ₐ[pc_p'] w
+    {{{ ▷ PC ↦ᵣ inr (pc_p,pc_b,pc_e,pc_a)
+      ∗ ▷ pc_a ↦ₐ w
       ∗ ▷ dst ↦ᵣ wdst
       ∗ ▷ src ↦ᵣ inl zsrc }}}
       Instr Executable @ E
       {{{ RET FailedV; True }}}.
   Proof.
-    iIntros (Hdecode Hinstr Hfl Hvpc φ) "(>HPC & >Hpc_a & >Hsrc & >Hdst) Hφ".
+    iIntros (Hdecode Hinstr Hvpc φ) "(>HPC & >Hpc_a & >Hsrc & >Hdst) Hφ".
     iDestruct (map_of_regs_3 with "HPC Hsrc Hdst") as "[Hmap (%&%&%)]".
     iApply (wp_Get with "[$Hmap Hpc_a]"); eauto; simplify_map_eq; eauto.
       by erewrite regs_of_is_Get; eauto; rewrite !dom_insert; set_solver+.
@@ -1396,145 +1145,33 @@ Section stack_macros.
     { (* Failure, done *) by iApply "Hφ". }
   Qed.
 
-  (* ------------------------------- *)
-
-  Definition reqglob r a p : iProp Σ :=
-    ([∗ list] a_i;w_i ∈ a;(reqglob_instrs r), a_i ↦ₐ[p] w_i)%I.
-
-  Lemma reqglob_spec r a w pc_p pc_p' pc_g pc_b pc_e a_first a_last φ :
-    isCorrectPC_range pc_p pc_g pc_b pc_e a_first a_last ->
-    PermFlows pc_p pc_p' ->
-    contiguous_between a a_first a_last ->
-
-      ▷ reqglob r a pc_p'
-    ∗ ▷ PC ↦ᵣ inr (pc_p,pc_g,pc_b,pc_e,a_first)
-    ∗ ▷ r ↦ᵣ w
-    ∗ ▷ (∃ w, r_t1 ↦ᵣ w)
-    ∗ ▷ (∃ w, r_t2 ↦ᵣ w)
-    (* if the capability is global, we want to be able to continue *)
-    (* if w is not a global capability, we will fail, and must now show that Phi holds at failV *)
-    ∗ ▷ (if isGlobalWord w then
-           ∃ g b e a', ⌜w = inr (g,Global,b,e,a')⌝ ∧
-          (PC ↦ᵣ inr (pc_p,pc_g,pc_b,pc_e,a_last) ∗ reqglob r a pc_p' ∗
-            r ↦ᵣ inr (g,Global,b,e,a') ∗ r_t1 ↦ᵣ inl 0%Z ∗ r_t2 ↦ᵣ inl 0%Z
-            -∗ WP Seq (Instr Executable) {{ φ }})
-        else φ FailedV)
-    ⊢
-      WP Seq (Instr Executable) {{ φ }}.
+  (* TODO: move this to the rules_Lea.v file. *)
+  Lemma wp_Lea_fail_none Ep pc_p pc_b pc_e pc_a w r1 rv p b e a z :
+    decodeInstrW w = Lea r1 (inr rv) →
+    isCorrectPC (inr (pc_p,pc_b,pc_e,pc_a)) →
+    (a + z)%a = None ->
+     
+     {{{ ▷ PC ↦ᵣ inr (pc_p,pc_b,pc_e,pc_a)
+           ∗ ▷ pc_a ↦ₐ w
+           ∗ ▷ r1 ↦ᵣ inr (p,b,e,a)
+           ∗ ▷ rv ↦ᵣ inl z }}}
+       Instr Executable @ Ep
+     {{{ RET FailedV; True }}}.
   Proof.
-    iIntros (Hvpc Hfl Hcont) "(>Hprog & >HPC & >Hr & >Hr_t1 & >Hr_t2 & Hcont)".
-    iDestruct (big_sepL2_length with "Hprog") as %Hlength. simpl in *.
-    iDestruct ("Hr_t1") as (w1) "Hr_t1".
-    iAssert (⌜r ≠ PC⌝)%I as %Hne.
-    { destruct (decide (r = PC)); auto; subst. iDestruct (regname_dupl_false with "HPC Hr") as %Hcontr. done. }
-    iPrologue "Hprog".
-    apply contiguous_between_cons_inv_first in Hcont as Heq. subst.
-    destruct w. 
-    { (* if w is an integer, the getL will fail *)
-      iApply (wp_Get_fail with "[$HPC $Hi $Hr_t1 $Hr]");
-        [apply decode_encode_instrW_inv|auto|apply Hfl|iCorrectPC a_first a_last|..].
-      iEpilogue "_ /=". 
-      iApply wp_value. done. 
-    }
-    (* if w is a capability, the getL will succeed *)
-    destruct a as [|a l];[done|]. 
-    iApply (wp_Get_success with "[$HPC $Hi $Hr $Hr_t1]");
-      [apply decode_encode_instrW_inv|auto|apply Hfl|iCorrectPC a_first a_last|iContiguous_next Hcont 0|auto..].
-    iEpilogue "(HPC & Hi & Hr & Hr_t1)". iRename "Hi" into "Hprog_done".
-    destruct c,p,p,p. iSimpl in "Hr_t1". 
-    (* sub r_t1 r_t1 (encodeLoc Global) *)
-    destruct l;[done|].
-    iPrologue "Hprog". 
-    iApply (wp_add_sub_lt_success_dst_z with "[$HPC $Hi $Hr_t1]");
-      [apply decode_encode_instrW_inv|auto|iContiguous_next Hcont 1|apply Hfl|iCorrectPC a_first a_last|..].
-    iEpilogue "(HPC & Hi & Hr_t1)". iCombine "Hi" "Hprog_done" as "Hprog_done". 
-    iSimpl in "Hr_t1".
-    (* move r_t2 PC *)
-    destruct l;[done|]. 
-    iPrologue "Hprog".
-    iDestruct "Hr_t2" as (w2) "Hr_t2". 
-    iApply (wp_move_success_reg_fromPC with "[$HPC $Hi $Hr_t2]");
-      [apply decode_encode_instrW_inv|apply Hfl|iCorrectPC a_first a_last|iContiguous_next Hcont 2|auto|..].
-    iEpilogue "(HPC & Hi & Hr_t2)"; iCombine "Hi" "Hprog_done" as "Hprog_done". 
-    (* lea r_t2 6 *)
-    do 7 (destruct l;[done|]). destruct l; [|done]. 
-    assert ((a3 + 6)%a = Some a9) as Hlea. 
-    { apply (contiguous_between_incr_addr_middle _ _ _ 2 6 a3 a9) in Hcont; auto. }
-    assert (pc_p ≠ E) as HneE.
-    { apply isCorrectPC_range_perm in Hvpc as [Heq | [Heq | Heq] ]; subst; auto.
-      apply (contiguous_between_middle_bounds _ 0 a_first) in Hcont as [_ Hlt]; auto. }
-    iPrologue "Hprog". 
-    iApply (wp_lea_success_z with "[$HPC $Hi $Hr_t2]");
-      [apply decode_encode_instrW_inv|apply Hfl|iCorrectPC a_first a_last|iContiguous_next Hcont 3|apply Hlea|auto..].
-    { apply isCorrectPC_range_perm in Hvpc as [Heq | [Heq | Heq] ]; subst; auto.
-      apply (contiguous_between_middle_bounds _ 0 a_first) in Hcont as [_ Hlt]; auto. }
-    iEpilogue "(HPC & Hi & Hr_t2)"; iCombine "Hi" "Hprog_done" as "Hprog_done". 
-    destruct (decide (encodeLoc l0 - encodeLoc Global = 0))%Z.
-    - (* l is Global *)
-      rewrite e. assert (l0 = Global);[apply encodeLoc_inj;lia|subst]. 
-      iSimpl in "Hcont". iDestruct "Hcont" as (g b e0 a' Heq) "Hφ". inversion Heq; subst.
-      iPrologue "Hprog". 
-      iApply (wp_jnz_success_next with "[$HPC $Hi $Hr_t2 $Hr_t1]");
-        [apply decode_encode_instrW_inv|apply Hfl|iCorrectPC a_first a_last|iContiguous_next Hcont 4|..].
-      iEpilogue "(HPC & Hi & Hr_t2 & Hr_t1)";iCombine "Hi" "Hprog_done" as "Hprog_done". 
-      (* move_r r_t2 PC *)
-      iPrologue "Hprog".
-      iApply (wp_move_success_reg_fromPC with "[$HPC $Hi $Hr_t2]");
-        [apply decode_encode_instrW_inv|apply Hfl|iCorrectPC a_first a_last|iContiguous_next Hcont 5|auto|..].
-      iEpilogue "(HPC & Hi & Hr_t2)"; iCombine "Hi" "Hprog_done" as "Hprog_done". 
-      (* lea r_t2 3 *)
-      assert ((a6 + 4)%a = Some a10) as Hlea'. 
-      { apply (contiguous_between_incr_addr_middle _ _ _ 5 4 a6 a10) in Hcont; auto. }
-      iPrologue "Hprog". 
-      iApply (wp_lea_success_z with "[$HPC $Hi $Hr_t2]");
-        [apply decode_encode_instrW_inv|apply Hfl|iCorrectPC a_first a_last|iContiguous_next Hcont 6|apply Hlea'|auto..].
-      { apply isCorrectPC_range_perm in Hvpc as [Heq' | [Heq' | Heq'] ]; subst; auto.
-        apply (contiguous_between_middle_bounds _ 0 a_first) in Hcont as [_ Hlt]; auto. }
-      iEpilogue "(HPC & Hi & Hr_t2)"; iCombine "Hi" "Hprog_done" as "Hprog_done". 
-      (* jmp r_t2 *)
-      iPrologue "Hprog".
-      iApply (wp_jmp_success with "[$HPC $Hi $Hr_t2]");
-        [apply decode_encode_instrW_inv|apply Hfl|iCorrectPC a_first a_last|..].
-      iEpilogue "(HPC & Hi & Hr_t2)"; iCombine "Hi" "Hprog_done" as "Hprog_done". 
-      assert (updatePcPerm (inr (pc_p, pc_g, pc_b, pc_e, a10)) = (inr (pc_p, pc_g, pc_b, pc_e, a10))) as ->.
-      { destruct pc_p; auto. congruence. }
-      iDestruct "Hprog" as "[Hi Hprog]". iCombine "Hi" "Hprog_done" as "Hprog_done". 
-      (* move r_t1 0 *)
-      iPrologue "Hprog".
-      iApply (wp_move_success_z with "[$HPC $Hi $Hr_t1]"); 
-        [apply decode_encode_instrW_inv|apply Hfl|iCorrectPC a_first a_last|iContiguous_next Hcont 9|auto|..].
-      iEpilogue "(HPC & Hi & Hr_t1)"; iCombine "Hi" "Hprog_done" as "Hprog_done". 
-      (* move r_t2 0 *)
-      iPrologue "Hprog".
-      apply contiguous_between_last with (ai:=a11) in Hcont as Hnext;[|auto]. 
-      iApply (wp_move_success_z with "[$HPC $Hi $Hr_t2]"); 
-        [apply decode_encode_instrW_inv|apply Hfl|iCorrectPC a_first a_last|apply Hnext|auto|..].
-      iEpilogue "(HPC & Hi & Hr_t2)"; iCombine "Hi" "Hprog_done" as "Hprog_done". 
-      iApply "Hφ". iFrame "HPC Hr Hr_t1 Hr_t2".
-      repeat (iDestruct "Hprog_done" as "[Hi Hprog_done]"; iFrame "Hi"). 
-      iFrame.
-    - destruct l0;[lia|iSimpl in "Hcont"]. 
-      (* jnz r_t2 r_t1 *)
-      iPrologue "Hprog".
-      iApply (wp_jnz_success_jmp with "[$HPC $Hi $Hr_t2 $Hr_t1]");
-        [apply decode_encode_instrW_inv|apply Hfl|iCorrectPC a_first a_last|..].
-      { intros Hcontr. inversion Hcontr. done. }
-      iEpilogue "(HPC & Hi & Hr_t2 & Hr_t1)"; iCombine "Hi" "Hprog_done" as "Hprog_done". 
-      do 3 (iDestruct "Hprog" as "[Hi Hprog]"; iCombine "Hi" "Hprog_done" as "Hprog_done"). 
-      (* fail *)
-      iPrologue "Hprog".
-      assert (updatePcPerm (inr (pc_p, pc_g, pc_b, pc_e, a9)) = (inr (pc_p, pc_g, pc_b, pc_e, a9))) as ->.
-      { destruct pc_p; auto. congruence. }
-      iApply (wp_fail with "[$HPC $Hi]");
-        [apply decode_encode_instrW_inv|apply Hfl|iCorrectPC a_first a_last|].
-      iEpilogue "(HPC & Hi)". iApply wp_value. iApply "Hcont". 
+    iIntros (Hdecode Hvpc Hz φ) "(>HPC & >Hpc_a & >Hsrc & >Hdst) Hφ".
+    iDestruct (map_of_regs_3 with "HPC Hsrc Hdst") as "[Hmap (%&%&%)]".
+    iApply (wp_lea with "[$Hmap Hpc_a]"); eauto; simplify_map_eq; eauto.
+      by rewrite !dom_insert; set_solver+.
+    iNext. iIntros (regs' retv) "(#Hspec & Hpc_a & Hmap)".
+    iDestruct "Hspec" as %Hspec.
+    destruct Hspec as [* Hsucc |].
+    { (* Success (contradiction) *) simplify_map_eq. }
+    { (* Failure, done *) by iApply "Hφ". }
   Qed.
 
-  (* -------------------------------------- REQPERM ----------------------------------- *)
-  (* the following macro requires that a given registers contains a capability with a 
-     given (encoded) permission. If this is not the case, the macro goes to fail,
-     otherwise it continues *)  
+  (* ------------------------------- *)
 
+  
   Definition reqperm_instrs r z :=
     [getp r_t1 r;
     sub_r_z r_t1 r_t1 z;
@@ -1547,33 +1184,29 @@ Section stack_macros.
     fail_end;
     move_z r_t1 0;
     move_z r_t2 0].
-
-
-  (* ------------------------------- *)
   
-  Definition reqperm r z a p : iProp Σ :=
-    ([∗ list] a_i;w_i ∈ a;(reqperm_instrs r z), a_i ↦ₐ[p] w_i)%I.
+  Definition reqperm r z a : iProp Σ :=
+    ([∗ list] a_i;w_i ∈ a;(reqperm_instrs r z), a_i ↦ₐ w_i)%I.
 
-  Lemma reqperm_spec r perm a w pc_p pc_p' pc_g pc_b pc_e a_first a_last φ :
-    isCorrectPC_range pc_p pc_g pc_b pc_e a_first a_last ->
-    PermFlows pc_p pc_p' ->
+  Lemma reqperm_spec r perm a w pc_p pc_b pc_e a_first a_last φ :
+    isCorrectPC_range pc_p pc_b pc_e a_first a_last ->
     contiguous_between a a_first a_last ->
 
-      ▷ reqperm r (encodePerm perm) a pc_p'
-    ∗ ▷ PC ↦ᵣ inr (pc_p,pc_g,pc_b,pc_e,a_first)
+      ▷ reqperm r (encodePerm perm) a
+    ∗ ▷ PC ↦ᵣ inr (pc_p,pc_b,pc_e,a_first)
     ∗ ▷ r ↦ᵣ w
     ∗ ▷ (∃ w, r_t1 ↦ᵣ w)
     ∗ ▷ (∃ w, r_t2 ↦ᵣ w)
     ∗ ▷ (if isPermWord w perm then
-           ∃ l b e a', ⌜w = inr (perm,l,b,e,a')⌝ ∧
-          (PC ↦ᵣ inr (pc_p,pc_g,pc_b,pc_e,a_last) ∗ reqperm r (encodePerm perm) a pc_p' ∗
-            r ↦ᵣ inr (perm,l,b,e,a') ∗ r_t1 ↦ᵣ inl 0%Z ∗ r_t2 ↦ᵣ inl 0%Z
+           ∃ b e a', ⌜w = inr (perm,b,e,a')⌝ ∧
+          (PC ↦ᵣ inr (pc_p,pc_b,pc_e,a_last) ∗ reqperm r (encodePerm perm) a ∗
+            r ↦ᵣ inr (perm,b,e,a') ∗ r_t1 ↦ᵣ inl 0%Z ∗ r_t2 ↦ᵣ inl 0%Z
             -∗ WP Seq (Instr Executable) {{ φ }})
         else φ FailedV)
     ⊢
       WP Seq (Instr Executable) {{ φ }}.
   Proof.
-    iIntros (Hvpc Hfl Hcont) "(>Hprog & >HPC & >Hr & >Hr_t1 & >Hr_t2 & Hcont)".
+    iIntros (Hvpc Hcont) "(>Hprog & >HPC & >Hr & >Hr_t1 & >Hr_t2 & Hcont)".
     iDestruct (big_sepL2_length with "Hprog") as %Hlength. simpl in *.
     iDestruct ("Hr_t1") as (w1) "Hr_t1".
     iAssert (⌜r ≠ PC⌝)%I as %Hne.
@@ -1583,21 +1216,21 @@ Section stack_macros.
     destruct w. 
     { (* if w is an integer, the getL will fail *)
       iApply (wp_Get_fail with "[$HPC $Hi $Hr_t1 $Hr]");
-        [apply decode_encode_instrW_inv|auto|apply Hfl|iCorrectPC a_first a_last|..].
+        [apply decode_encode_instrW_inv|auto|iCorrectPC a_first a_last|..].
       iEpilogue "_ /=". 
       iApply wp_value. done. 
     }
     (* if w is a capability, the getL will succeed *)
     destruct a as [|a l];[done|]. 
     iApply (wp_Get_success with "[$HPC $Hi $Hr $Hr_t1]");
-      [apply decode_encode_instrW_inv|auto|apply Hfl|iCorrectPC a_first a_last|iContiguous_next Hcont 0|auto..].
+      [apply decode_encode_instrW_inv|auto|iCorrectPC a_first a_last|iContiguous_next Hcont 0|auto..].
     iEpilogue "(HPC & Hi & Hr & Hr_t1)". iRename "Hi" into "Hprog_done".
-    destruct c,p,p,p. iSimpl in "Hr_t1". 
+    destruct c,p,p. iSimpl in "Hr_t1". 
     (* sub r_t1 r_t1 (encodeLoc Global) *)
     destruct l;[done|].
     iPrologue "Hprog". 
     iApply (wp_add_sub_lt_success_dst_z with "[$HPC $Hi $Hr_t1]");
-      [apply decode_encode_instrW_inv|auto|iContiguous_next Hcont 1|apply Hfl|iCorrectPC a_first a_last|..].
+      [apply decode_encode_instrW_inv|auto|iContiguous_next Hcont 1|iCorrectPC a_first a_last|..].
     iEpilogue "(HPC & Hi & Hr_t1)". iCombine "Hi" "Hprog_done" as "Hprog_done". 
     iSimpl in "Hr_t1".
     (* move r_t2 PC *)
@@ -1605,64 +1238,60 @@ Section stack_macros.
     iPrologue "Hprog".
     iDestruct "Hr_t2" as (w2) "Hr_t2". 
     iApply (wp_move_success_reg_fromPC with "[$HPC $Hi $Hr_t2]");
-      [apply decode_encode_instrW_inv|apply Hfl|iCorrectPC a_first a_last|iContiguous_next Hcont 2|auto|..].
+      [apply decode_encode_instrW_inv|iCorrectPC a_first a_last|iContiguous_next Hcont 2|auto|..].
     iEpilogue "(HPC & Hi & Hr_t2)"; iCombine "Hi" "Hprog_done" as "Hprog_done". 
     (* lea r_t2 6 *)
     do 7 (destruct l;[done|]). destruct l; [|done]. 
     assert ((a3 + 6)%a = Some a9) as Hlea. 
     { apply (contiguous_between_incr_addr_middle _ _ _ 2 6 a3 a9) in Hcont; auto. }
     assert (pc_p ≠ E) as HneE.
-    { apply isCorrectPC_range_perm in Hvpc as [Heq | [Heq | Heq] ]; subst; auto.
+    { apply isCorrectPC_range_perm in Hvpc as [Heq | Heq ]; subst; auto.
       apply (contiguous_between_middle_bounds _ 0 a_first) in Hcont as [_ Hlt]; auto. }
     iPrologue "Hprog". 
     iApply (wp_lea_success_z with "[$HPC $Hi $Hr_t2]");
-      [apply decode_encode_instrW_inv|apply Hfl|iCorrectPC a_first a_last|iContiguous_next Hcont 3|apply Hlea|auto..].
-    { apply isCorrectPC_range_perm in Hvpc as [Heq | [Heq | Heq] ]; subst; auto.
-      apply (contiguous_between_middle_bounds _ 0 a_first) in Hcont as [_ Hlt]; auto.  }
+      [apply decode_encode_instrW_inv|iCorrectPC a_first a_last|iContiguous_next Hcont 3|apply Hlea|auto..].
     iEpilogue "(HPC & Hi & Hr_t2)"; iCombine "Hi" "Hprog_done" as "Hprog_done". 
     destruct (decide (encodePerm p - encodePerm perm = 0))%Z.
     - (* p is perm *)
       rewrite e. assert (p = perm);[apply encodePerm_inj;lia|subst]. 
-      iSimpl in "Hcont". rewrite isPerm_refl. iDestruct "Hcont" as (l b e0 a' Heq) "Hφ". inversion Heq; subst.
+      iSimpl in "Hcont". rewrite isPerm_refl. iDestruct "Hcont" as (b e0 a' Heq) "Hφ". inversion Heq; subst.
       iPrologue "Hprog". 
       iApply (wp_jnz_success_next with "[$HPC $Hi $Hr_t2 $Hr_t1]");
-        [apply decode_encode_instrW_inv|apply Hfl|iCorrectPC a_first a_last|iContiguous_next Hcont 4|..].
+        [apply decode_encode_instrW_inv|iCorrectPC a_first a_last|iContiguous_next Hcont 4|..].
       iEpilogue "(HPC & Hi & Hr_t2 & Hr_t1)";iCombine "Hi" "Hprog_done" as "Hprog_done". 
       (* move_r r_t2 PC *)
       iPrologue "Hprog".
       iApply (wp_move_success_reg_fromPC with "[$HPC $Hi $Hr_t2]");
-        [apply decode_encode_instrW_inv|apply Hfl|iCorrectPC a_first a_last|iContiguous_next Hcont 5|auto|..].
+        [apply decode_encode_instrW_inv|iCorrectPC a_first a_last|iContiguous_next Hcont 5|auto|..].
       iEpilogue "(HPC & Hi & Hr_t2)"; iCombine "Hi" "Hprog_done" as "Hprog_done". 
       (* lea r_t2 3 *)
       assert ((a6 + 4)%a = Some a10) as Hlea'. 
       { apply (contiguous_between_incr_addr_middle _ _ _ 5 4 a6 a10) in Hcont; auto. }
       iPrologue "Hprog". 
       iApply (wp_lea_success_z with "[$HPC $Hi $Hr_t2]");
-        [apply decode_encode_instrW_inv|apply Hfl|iCorrectPC a_first a_last|iContiguous_next Hcont 6|apply Hlea'|auto..].
-      { apply isCorrectPC_range_perm in Hvpc as [Heq' | [Heq' | Heq'] ]; subst; auto.
-      apply (contiguous_between_middle_bounds _ 0 a_first) in Hcont as [_ Hlt]; auto.  }
+        [apply decode_encode_instrW_inv|iCorrectPC a_first a_last|iContiguous_next Hcont 6|apply Hlea'|auto..].
       iEpilogue "(HPC & Hi & Hr_t2)"; iCombine "Hi" "Hprog_done" as "Hprog_done". 
       (* jmp r_t2 *)
       iPrologue "Hprog".
       iApply (wp_jmp_success with "[$HPC $Hi $Hr_t2]");
-        [apply decode_encode_instrW_inv|apply Hfl|iCorrectPC a_first a_last|..].
+        [apply decode_encode_instrW_inv|iCorrectPC a_first a_last|..].
       iEpilogue "(HPC & Hi & Hr_t2)"; iCombine "Hi" "Hprog_done" as "Hprog_done". 
-      assert (updatePcPerm (inr (pc_p, pc_g, pc_b, pc_e, a10)) = (inr (pc_p, pc_g, pc_b, pc_e, a10))) as ->.
+      assert (updatePcPerm (inr (pc_p, pc_b, pc_e, a10)) = (inr (pc_p, pc_b, pc_e, a10))) as ->.
       { destruct pc_p; auto. congruence. }
       iDestruct "Hprog" as "[Hi Hprog]". iCombine "Hi" "Hprog_done" as "Hprog_done". 
       (* move r_t1 0 *)
       iPrologue "Hprog".
       iApply (wp_move_success_z with "[$HPC $Hi $Hr_t1]"); 
-        [apply decode_encode_instrW_inv|apply Hfl|iCorrectPC a_first a_last|iContiguous_next Hcont 9|auto|..].
+        [apply decode_encode_instrW_inv|iCorrectPC a_first a_last|iContiguous_next Hcont 9|auto|..].
       iEpilogue "(HPC & Hi & Hr_t1)"; iCombine "Hi" "Hprog_done" as "Hprog_done". 
       (* move r_t2 0 *)
       iPrologue "Hprog".
       apply contiguous_between_last with (ai:=a11) in Hcont as Hnext;[|auto]. 
       iApply (wp_move_success_z with "[$HPC $Hi $Hr_t2]"); 
-        [apply decode_encode_instrW_inv|apply Hfl|iCorrectPC a_first a_last|apply Hnext|auto|..].
+        [apply decode_encode_instrW_inv|iCorrectPC a_first a_last|apply Hnext|auto|..].
       iEpilogue "(HPC & Hi & Hr_t2)"; iCombine "Hi" "Hprog_done" as "Hprog_done". 
       iApply "Hφ". iFrame "HPC Hr Hr_t1 Hr_t2".
-      repeat (iDestruct "Hprog_done" as "[Hi Hprog_done]"; iFrame "Hi"). 
+      do 10 (iDestruct "Hprog_done" as "[Hi Hprog_done]"; iFrame "Hi"). 
       iFrame.
     - assert (p ≠ perm) as HneP.
       { intros Hcontr. subst. lia. }
@@ -1670,16 +1299,16 @@ Section stack_macros.
       (* jnz r_t2 r_t1 *)
       iPrologue "Hprog".
       iApply (wp_jnz_success_jmp with "[$HPC $Hi $Hr_t2 $Hr_t1]");
-        [apply decode_encode_instrW_inv|apply Hfl|iCorrectPC a_first a_last|..].
+        [apply decode_encode_instrW_inv|iCorrectPC a_first a_last|..].
       { intros Hcontr. inversion Hcontr. done. }
       iEpilogue "(HPC & Hi & Hr_t2 & Hr_t1)"; iCombine "Hi" "Hprog_done" as "Hprog_done". 
       do 3 (iDestruct "Hprog" as "[Hi Hprog]"; iCombine "Hi" "Hprog_done" as "Hprog_done"). 
       (* fail *)
       iPrologue "Hprog".
-      assert (updatePcPerm (inr (pc_p, pc_g, pc_b, pc_e, a9)) = (inr (pc_p, pc_g, pc_b, pc_e, a9))) as ->.
+      assert (updatePcPerm (inr (pc_p, pc_b, pc_e, a9)) = (inr (pc_p, pc_b, pc_e, a9))) as ->.
       { destruct pc_p; auto. congruence. }
       iApply (wp_fail with "[$HPC $Hi]");
-        [apply decode_encode_instrW_inv|apply Hfl|iCorrectPC a_first a_last|].
+        [apply decode_encode_instrW_inv|iCorrectPC a_first a_last|].
       iEpilogue "(HPC & Hi)". iApply wp_value. iApply "Hcont". 
   Qed.
 
@@ -1697,24 +1326,23 @@ Section stack_macros.
      jnz r_t2 r_t1;
      fail_end].
 
-  Definition reqsize r minsize a p : iProp Σ :=
-    ([∗ list] a_i;w_i ∈ a;(reqsize_instrs r minsize), a_i ↦ₐ[p] w_i)%I.
+  Definition reqsize r minsize a : iProp Σ :=
+    ([∗ list] a_i;w_i ∈ a;(reqsize_instrs r minsize), a_i ↦ₐ w_i)%I.
 
-  Lemma reqsize_spec r minsize a pc_p pc_p' pc_g pc_b pc_e a_first a_last r_p r_g r_b r_e r_a w1 w2 φ :
-    isCorrectPC_range pc_p pc_g pc_b pc_e a_first a_last →
-    PermFlows pc_p pc_p' →
+  Lemma reqsize_spec r minsize a pc_p pc_b pc_e a_first a_last r_p r_b r_e r_a w1 w2 φ :
+    isCorrectPC_range pc_p pc_b pc_e a_first a_last →
     contiguous_between a a_first a_last →
 
-      ▷ reqsize r minsize a pc_p'
-    ∗ ▷ PC ↦ᵣ inr (pc_p,pc_g,pc_b,pc_e,a_first)
-    ∗ ▷ r ↦ᵣ inr (r_p, r_g, r_b, r_e, r_a)
+      ▷ reqsize r minsize a 
+    ∗ ▷ PC ↦ᵣ inr (pc_p,pc_b,pc_e,a_first)
+    ∗ ▷ r ↦ᵣ inr (r_p, r_b, r_e, r_a)
     ∗ ▷ r_t1 ↦ᵣ w1
     ∗ ▷ r_t2 ↦ᵣ w2
     ∗ ▷ (if (minsize <? (r_e - r_b)%a)%Z then
            (∃ w1 w2,
-            reqsize r minsize a pc_p'
-            ∗ PC ↦ᵣ inr (pc_p,pc_g,pc_b,pc_e,a_last)
-            ∗ r ↦ᵣ inr (r_p, r_g, r_b, r_e, r_a)
+            reqsize r minsize a 
+            ∗ PC ↦ᵣ inr (pc_p,pc_b,pc_e,a_last)
+            ∗ r ↦ᵣ inr (r_p, r_b, r_e, r_a)
             ∗ r_t1 ↦ᵣ w1
             ∗ r_t2 ↦ᵣ w2)
            -∗ WP Seq (Instr Executable) {{ φ }}
@@ -1722,7 +1350,7 @@ Section stack_macros.
     ⊢
     WP Seq (Instr Executable) {{ φ }}.
   Proof.
-    iIntros (Hvpc Hfl Hcont) "(>Hprog & >HPC & >Hr & >Hr1 & >Hr2 & Hcont)".
+    iIntros (Hvpc Hcont) "(>Hprog & >HPC & >Hr & >Hr1 & >Hr2 & Hcont)".
     iDestruct (big_sepL2_length with "Hprog") as %Hlength. simpl in *.
     iAssert (⌜r ≠ PC⌝)%I as %Hne.
     { iIntros (->). iApply (regname_dupl_false with "HPC Hr"). }
@@ -1736,238 +1364,62 @@ Section stack_macros.
     destruct l as [| ? l];[done|].
     iPrologue "Hprog".
     iApply (wp_Get_success with "[$HPC $Hi $Hr $Hr1]");
-      [apply decode_encode_instrW_inv|auto|apply Hfl|iCorrectPC a_first a_last|iContiguous_next Hcont 0|auto..];
+      [apply decode_encode_instrW_inv|auto|iCorrectPC a_first a_last|iContiguous_next Hcont 0|auto..];
       simpl.
     iEpilogue "(HPC & Hi & Hr & Hr1)". iRename "Hi" into "Hprog_done".
     (* gete r_t2 r *)
     destruct l as [| ? l];[done|].
     iPrologue "Hprog".
     iApply (wp_Get_success with "[$HPC $Hi $Hr $Hr2]");
-      [apply decode_encode_instrW_inv|auto|apply Hfl|iCorrectPC a_first a_last|iContiguous_next Hcont 1|auto..];
+      [apply decode_encode_instrW_inv|auto|iCorrectPC a_first a_last|iContiguous_next Hcont 1|auto..];
       simpl.
     iEpilogue "(HPC & Hi & Hr & Hr2)". iCombine "Hi" "Hprog_done" as "Hprog_done".
     (* sub_r_r r_t1 r_t2 r_t1 *)
     destruct l as [| ? l];[done|].
     iPrologue "Hprog".
     iApply (wp_add_sub_lt_success_r_dst with "[$HPC $Hi $Hr2 $Hr1]");
-      [apply decode_encode_instrW_inv|done|iContiguous_next Hcont 2|apply Hfl|iCorrectPC a_first a_last|..];
+      [apply decode_encode_instrW_inv|done|iContiguous_next Hcont 2|iCorrectPC a_first a_last|..];
       simpl.
     iEpilogue "(HPC & Hi & Hr2 & Hr1)". iCombine "Hi" "Hprog_done" as "Hprog_done".
     (* lt_z_r r_t1 minsize r_t1 *)
     destruct l as [| ? l];[done|].
     iPrologue "Hprog".
     iApply (wp_add_sub_lt_success_z_dst with "[$HPC $Hi $Hr1]");
-      [apply decode_encode_instrW_inv|done|iContiguous_next Hcont 3|apply Hfl|iCorrectPC a_first a_last|..];
+      [apply decode_encode_instrW_inv|done|iContiguous_next Hcont 3|iCorrectPC a_first a_last|..];
       simpl.
     iEpilogue "(HPC & Hi & Hr1)". iCombine "Hi" "Hprog_done" as "Hprog_done".
     (* move_r r_t2 PC *)
     destruct l as [| ? l];[done|].
     iPrologue "Hprog".
     iApply (wp_move_success_reg_fromPC with "[$HPC $Hi $Hr2]");
-      [apply decode_encode_instrW_inv|apply Hfl|iCorrectPC a_first a_last|iContiguous_next Hcont 4|auto..].
+      [apply decode_encode_instrW_inv|iCorrectPC a_first a_last|iContiguous_next Hcont 4|auto..].
     iEpilogue "(HPC & Hi & Hr2)". iCombine "Hi" "Hprog_done" as "Hprog_done".
     (* lea_z r_t2 4 *)
     destruct l as [| ? l];[done|].
     iPrologue "Hprog".
     iApply (wp_lea_success_z with "[$HPC $Hi $Hr2]");
-      [apply decode_encode_instrW_inv|apply Hfl|iCorrectPC a_first a_last|iContiguous_next Hcont 5|try done..].
+      [apply decode_encode_instrW_inv|iCorrectPC a_first a_last|iContiguous_next Hcont 5|try done..].
     { change 4%Z with (Z.of_nat (4%nat)).
       (* FIXME: a bit annoying to have to specify the index manually *)
       eapply (contiguous_between_middle_to_end _ _ _ 4); eauto. }
-    { assert (isCorrectPC (inr (pc_p, pc_g, pc_b, pc_e, a_first))) as HH.
-      iCorrectPC a_first a_last. inversion HH; subst. 
-      repeat match goal with H: _ ∨ _ |- _ => destruct H end; subst; auto. }
     iEpilogue "(HPC & Hi & Hr2)". iCombine "Hi" "Hprog_done" as "Hprog_done".
     (* jnz r_t2 r_t1 *)
     destruct l as [| ? l];[done|].
     iPrologue "Hprog".
     destruct (minsize <? r_e - r_b)%Z eqn:Htest; simpl.
     { iApply (wp_jnz_success_jmp with "[$HPC $Hr2 $Hr1 $Hi]");
-        [apply decode_encode_instrW_inv|apply Hfl|iCorrectPC a_first a_last|done|..].
+        [apply decode_encode_instrW_inv|iCorrectPC a_first a_last|done|..].
       iEpilogue "(HPC & Hi & Hr2 & Hr1)". iApply "Hcont". iExists _,_.
       rewrite updatePcPerm_cap_non_E //. iFrame.
       iDestruct "Hprog_done" as "(?&?&?&?&?&?)". iFrame. }
     { iApply (wp_jnz_success_next with "[$HPC $Hr2 $Hr1 $Hi]");
-        [apply decode_encode_instrW_inv|apply Hfl|iCorrectPC a_first a_last|iContiguous_next Hcont 6|..].
+        [apply decode_encode_instrW_inv|iCorrectPC a_first a_last|iContiguous_next Hcont 6|..].
       iEpilogue "(HPC & Hi & Hr2 & Hr1)". iCombine "Hi" "Hprog_done" as "Hprog_done".
       (* fail_end *)
       iPrologue "Hprog".
       iApply (wp_fail with "[$HPC $Hi]");
-        [apply decode_encode_instrW_inv|apply Hfl|iCorrectPC a_first a_last|..].
+        [apply decode_encode_instrW_inv|iCorrectPC a_first a_last|..].
       iEpilogue "(HPC & Hi)". iApply wp_value. iApply "Hcont". }
-  Qed.
-
-  (* -------------------------------------- PREPSTACK ---------------------------------- *)
-  (* The following macro first checks whether r is a capability with permission RWLX. Next
-     if it is, it will move the pointer to the bottom of its range *)
-
-  Definition prepstack_instrs r (minsize: Z) :=
-    reqperm_instrs r (encodePerm RWLX) ++
-    reqsize_instrs r minsize ++
-    [getb r_t1 r;
-    geta r_t2 r;
-    sub_r_r r_t1 r_t1 r_t2;
-    lea_r r r_t1;
-    sub_z_z r_t1 0 1;
-    lea_r r r_t1;
-    move_z r_t1 0;
-    move_z r_t2 0].
-
-  Definition prepstack r minsize a p : iProp Σ :=
-    ([∗ list] a_i;w_i ∈ a;(prepstack_instrs r minsize), a_i ↦ₐ[p] w_i)%I.
-
-  Definition bound_check (w : Word) : option Addr :=
-    match w with 
-    | inr (_,_,b,_,_) => (b + (-1))%a
-    | _ => None
-    end. 
-
-  (* TODO: move this to the rules_Lea.v file. *)
-  Lemma wp_Lea_fail_none Ep pc_p pc_g pc_b pc_e pc_a w r1 rv p g b e a z pc_p' :
-    decodeInstrW w = Lea r1 (inr rv) →
-    PermFlows pc_p pc_p' → isCorrectPC (inr ((pc_p,pc_g),pc_b,pc_e,pc_a)) →
-    (a + z)%a = None ->
-     
-     {{{ ▷ PC ↦ᵣ inr ((pc_p,pc_g),pc_b,pc_e,pc_a)
-           ∗ ▷ pc_a ↦ₐ[pc_p'] w
-           ∗ ▷ r1 ↦ᵣ inr ((p,g),b,e,a)
-           ∗ ▷ rv ↦ᵣ inl z }}}
-       Instr Executable @ Ep
-     {{{ RET FailedV; True }}}.
-  Proof.
-    iIntros (Hdecode Hfl Hvpc Hz φ) "(>HPC & >Hpc_a & >Hsrc & >Hdst) Hφ".
-    iDestruct (map_of_regs_3 with "HPC Hsrc Hdst") as "[Hmap (%&%&%)]".
-    iApply (wp_lea with "[$Hmap Hpc_a]"); eauto; simplify_map_eq; eauto.
-      by rewrite !dom_insert; set_solver+.
-    iNext. iIntros (regs' retv) "(#Hspec & Hpc_a & Hmap)".
-    iDestruct "Hspec" as %Hspec.
-    destruct Hspec as [* Hsucc |].
-    { (* Success (contradiction) *) simplify_map_eq. }
-    { (* Failure, done *) by iApply "Hφ". }
-  Qed.
-  
-  Lemma prepstack_spec r minsize a w pc_p pc_p' pc_g pc_b pc_e a_first a_last φ :
-    isCorrectPC_range pc_p pc_g pc_b pc_e a_first a_last ->
-    PermFlows pc_p pc_p' ->
-    contiguous_between a a_first a_last ->
-
-      ▷ prepstack r minsize a pc_p'
-    ∗ ▷ PC ↦ᵣ inr (pc_p,pc_g,pc_b,pc_e,a_first)
-    ∗ ▷ r ↦ᵣ w
-    ∗ ▷ (∃ w, r_t1 ↦ᵣ w)
-    ∗ ▷ (∃ w, r_t2 ↦ᵣ w)
-    (* if the capability is global, we want to be able to continue *)
-    (* if w is not a global capability, we will fail, and must now show that Phi holds at failV *)
-    ∗ ▷ (if isPermWord w RWLX then
-           if (minsize <? cap_size w)%Z then
-             if (decide (is_Some (bound_check w))) then 
-               (∃ l b e a' b', ⌜w = inr (RWLX,l,b,e,a')⌝ ∧ ⌜(b' + 1)%a = Some b⌝ ∧
-                PC ↦ᵣ inr (pc_p,pc_g,pc_b,pc_e,a_last) ∗ prepstack r minsize a pc_p' ∗
-                   r ↦ᵣ inr (RWLX,l,b,e,b') ∗ r_t1 ↦ᵣ inl 0%Z ∗ r_t2 ↦ᵣ inl 0%Z)
-                 -∗ WP Seq (Instr Executable) {{ φ }}
-             else φ FailedV
-           else φ FailedV
-        else φ FailedV)
-    ⊢
-      WP Seq (Instr Executable) {{ φ }}.
-  Proof.
-    iIntros (Hvpc Hfl Hcont) "(>Hprog & >HPC & >Hr & >Hr_t1 & >Hr_t2 & Hφ)".
-    iDestruct (big_sepL2_length with "Hprog") as %Hlength. simpl in *.
-    iAssert (⌜r ≠ PC⌝)%I as %Hne.
-    { destruct (decide (r = PC)); auto; subst. iDestruct (regname_dupl_false with "HPC Hr") as %Hcontr. done. }
-    (* reqperm *)
-    iDestruct (contiguous_between_program_split with "Hprog") as (reqperm_prog rest link)
-                                                                   "(Hreqperm & Hprog & #Hcont)";[apply Hcont|].
-    iDestruct "Hcont" as %(Hcont_reqperm & Hcont_rest & Heqapp & Hlink).
-    iApply (reqperm_spec with "[$HPC $Hreqperm $Hr $Hr_t1 $Hr_t2 Hφ Hprog]"); [|apply Hfl|apply Hcont_reqperm|]. 
-    { intros mid Hmid. apply isCorrectPC_inrange with a_first a_last; auto.
-      apply contiguous_between_bounds in Hcont_rest. solve_addr. }
-    iNext. destruct (isPermWord w RWLX) eqn:Hperm; auto.
-    destruct w as [z | [ [ [ [p g] b] e] a'] ];[inversion Hperm|].
-    destruct p;inversion Hperm.
-    iExists _,_,_,_;iSplit;[eauto|]. 
-    iIntros "(HPC & Hprog_done & Hr & Hr_t1 & Hr_t2)".
-    assert (isCorrectPC_range pc_p pc_g pc_b pc_e link a_last) as Hvpc_rest.
-    { intros mid Hmid. apply isCorrectPC_inrange with a_first a_last; auto.
-      apply contiguous_between_bounds in Hcont_rest. solve_addr. }
-    (* reqsize *)
-    iDestruct (contiguous_between_program_split with "Hprog")
-      as (reqsize_prog rest' link') "(Hreqsize & Hprog & #Hcont)";[apply Hcont_rest|].
-    iDestruct "Hcont" as %(Hcont_reqsize & Hcont_rest' & Heqapp' & Hlink').
-    iApply (reqsize_spec with "[- $HPC $Hreqsize $Hr $Hr_t1 $Hr_t2]");
-      [|apply Hfl|eauto|].
-    { intros mid Hmid. apply isCorrectPC_inrange with a_first a_last; auto.
-      apply contiguous_between_bounds in Hcont_rest'. solve_addr. }
-    iNext. simpl. destruct (minsize <? e - b)%Z; auto.
-    iIntros "H". iDestruct "H" as (w1 w2) "(Hreqsize & HPC & Hr & Hr_t1 & Hr_t2)".
-    assert (isCorrectPC_range pc_p pc_g pc_b pc_e link' a_last) as Hvpc_rest'.
-    { intros mid Hmid. apply isCorrectPC_inrange with a_first a_last; auto.
-      apply contiguous_between_bounds in Hcont_rest. solve_addr. }
-    (* getb r_t1 r *)
-    iDestruct (big_sepL2_length with "Hprog") as %Hlength'.
-    do 2 (destruct rest';[inversion Hlength'|]). 
-    iPrologue "Hprog".
-    apply contiguous_between_cons_inv_first in Hcont_rest' as Heq; subst.
-    iApply (wp_Get_success with "[$HPC $Hi $Hr $Hr_t1]");
-      [apply decode_encode_instrW_inv|auto|apply Hfl|iCorrectPC link' a_last|iContiguous_next Hcont_rest' 0|auto..].
-    iEpilogue "(HPC & Hi & Hr & Hr_t1) /="; iCombine "Hi" "Hprog_done" as "Hprog_done". 
-    (* geta r_t2 r *)
-    destruct rest';[inversion Hlength'|].
-    iPrologue "Hprog".
-    iApply (wp_Get_success with "[$HPC $Hi $Hr $Hr_t2]");
-      [apply decode_encode_instrW_inv|auto|apply Hfl|iCorrectPC link' a_last|iContiguous_next Hcont_rest' 1|auto..].
-    iEpilogue "(HPC & Hi & Hr & Hr_t2) /="; iCombine "Hi" "Hprog_done" as "Hprog_done". 
-    (* sub r_t1 r_t1 r_t2 *)
-    destruct rest';[inversion Hlength'|].
-    iPrologue "Hprog".
-    iApply (wp_add_sub_lt_success_dst_r with "[$HPC $Hi $Hr_t2 $Hr_t1]");
-      [apply decode_encode_instrW_inv|auto|iContiguous_next Hcont_rest' 2|apply Hfl|iCorrectPC link' a_last|..].
-    iEpilogue "(HPC & Hi & Hr_t2 & Hr_t1) /="; iCombine "Hi" "Hprog_done" as "Hprog_done". 
-    (* lea r r_t1 *)
-    destruct rest';[inversion Hlength'|].
-    iPrologue "Hprog".
-    assert ((a' + (b - a'))%a = Some b) as Hlea;[solve_addr|].
-    iApply (wp_lea_success_reg with "[$HPC $Hi $Hr_t1 $Hr]");
-      [apply decode_encode_instrW_inv|apply Hfl|iCorrectPC link' a_last|iContiguous_next Hcont_rest' 3|apply Hlea|auto..].
-    { simpl;auto. }
-    iEpilogue "(HPC & Hi & Hr_t1 & Hr)"; iCombine "Hi" "Hprog_done" as "Hprog_done". 
-    (* sub r_t1 0 1 *)
-    destruct rest';[inversion Hlength'|].
-    iPrologue "Hprog".
-    iApply (wp_add_sub_lt_success_z_z with "[$HPC $Hi $Hr_t1]");
-      [apply decode_encode_instrW_inv|auto|iContiguous_next Hcont_rest' 4|apply Hfl|iCorrectPC link' a_last|..].
-    iEpilogue "(HPC & Hi & Hr_t1) /="; iCombine "Hi" "Hprog_done" as "Hprog_done". 
-    (* lea r r_t1 *)
-    destruct rest';[inversion Hlength'|].
-    iPrologue "Hprog".
-    (* if lea fails we go to φ FailedV *)
-    destruct (b + -1)%a as [b'|] eqn:Hb; simpl.
-    2: { iApply (wp_Lea_fail_none with "[$HPC $Hi $Hr_t1 $Hr]");
-           [apply decode_encode_instrW_inv|apply Hfl|iCorrectPC link' a_last|apply Hb|..].
-         iEpilogue "_". iApply wp_value. iApply "Hφ". }
-    assert ((b + (0 - 1))%a = Some b') as Hlea';[revert Hb;clear;solve_addr|].
-    iApply (wp_lea_success_reg with "[$HPC $Hi $Hr_t1 $Hr]");
-      [apply decode_encode_instrW_inv|apply Hfl|iCorrectPC link' a_last|iContiguous_next Hcont_rest' 5|apply Hlea'|auto..].
-    { simpl;auto. }
-    iEpilogue "(HPC & Hi & Hr_t1 & Hr)"; iCombine "Hi" "Hprog_done" as "Hprog_done". 
-    (* move r_t1 0 *)
-    destruct rest';[inversion Hlength'|].
-    iPrologue "Hprog".
-    iApply (wp_move_success_z with "[$HPC $Hi $Hr_t1]"); 
-      [apply decode_encode_instrW_inv|apply Hfl|iCorrectPC link' a_last|iContiguous_next Hcont_rest' 6|auto|..].
-    iEpilogue "(HPC & Hi & Hr_t1)"; iCombine "Hi" "Hprog_done" as "Hprog_done". 
-    (* move r_t2 0 *)
-    destruct rest';[|inversion Hlength'].
-    iPrologue "Hprog".
-    apply contiguous_between_last with (ai:=a12) in Hcont_rest' as Hlast;[|auto].
-    iApply (wp_move_success_z with "[$HPC $Hi $Hr_t2]"); 
-      [apply decode_encode_instrW_inv|apply Hfl|iCorrectPC link' a_last|apply Hlast|auto|..].
-    iEpilogue "(HPC & Hi & Hr_t2)"; iCombine "Hi" "Hprog_done" as "Hprog_done".
-    assert ((b' + 1)%a = Some b) as Hb';[revert Hlea';clear;solve_addr|]. 
-    iApply "Hφ". iExists _,_,_,_,_. iSplit;[eauto|]. iSplit;[iPureIntro;apply Hb'|]. 
-    iFrame. rewrite Heqapp. 
-    repeat (iDestruct "Hprog_done" as "[Hi Hprog_done]"; iFrame "Hi"). 
-    iFrame "Hprog_done". iFrame. done.
   Qed.
 
   (* ---------------------------------------- CRTCLS ------------------------------------ *)
@@ -2009,46 +1461,40 @@ Section stack_macros.
     store_r r_t1 r_t7;
     move_z r_t7 0;
     lea_z r_t1 (-7)%Z;
-    restrict_z r_t1 global_e].
+    restrict_z r_t1 e].
 
-  Definition crtcls f_m a p : iProp Σ :=
-    ([∗ list] a_i;w_i ∈ a;(crtcls_instrs f_m), a_i ↦ₐ[p] w_i)%I.
+  Definition crtcls f_m a : iProp Σ :=
+    ([∗ list] a_i;w_i ∈ a;(crtcls_instrs f_m), a_i ↦ₐ w_i)%I.
 
   (* crtcls spec *)
-  Lemma crtcls_spec W f_m wvar wcode a pc_p pc_p' pc_g pc_b pc_e
+  Lemma crtcls_spec f_m wvar wcode a pc_p pc_b pc_e
         a_first a_last b_link a_link e_link a_entry b_m e_m mallocN EN rmap cont φ :
-    isCorrectPC_range pc_p pc_g pc_b pc_e a_first a_last →
-    PermFlows pc_p pc_p' →
+    isCorrectPC_range pc_p pc_b pc_e a_first a_last →
     contiguous_between a a_first a_last →
-    withinBounds (RW, Global, b_link, e_link, a_entry) = true →
+    withinBounds (RW, b_link, e_link, a_entry) = true →
     (a_link + f_m)%a = Some a_entry →
     dom (gset RegName) rmap = all_registers_s ∖ {[ PC; r_t0; r_t1; r_t2 ]} →
-    isLocalWord wcode = false → (* the closure must be a Global Word! *)
-    isLocalWord wvar = false → (* the closure must be a Global Word! *)
     ↑mallocN ⊆ EN →
 
-      ▷ crtcls f_m a pc_p'
-    ∗ ▷ PC ↦ᵣ inr (pc_p,pc_g,pc_b,pc_e,a_first)
+      ▷ crtcls f_m a
+    ∗ ▷ PC ↦ᵣ inr (pc_p,pc_b,pc_e,a_first)
     ∗ na_inv logrel_nais mallocN (malloc_inv b_m e_m)
     ∗ na_own logrel_nais EN
     (* we need to assume that the malloc capability is in the linking table at offset 0 *)
-    ∗ ▷ pc_b ↦ₐ[pc_p'] inr (RO,Global,b_link,e_link,a_link)
-    ∗ ▷ a_entry ↦ₐ[RO] inr (E,Global,b_m,e_m,b_m)
+    ∗ ▷ pc_b ↦ₐ inr (RO,b_link,e_link,a_link)
+    ∗ ▷ a_entry ↦ₐ inr (E,b_m,e_m,b_m)
     (* register state *)
     ∗ ▷ r_t0 ↦ᵣ cont
     ∗ ▷ r_t1 ↦ᵣ wcode
     ∗ ▷ r_t2 ↦ᵣ wvar
     ∗ ▷ ([∗ map] r_i↦w_i ∈ rmap, r_i ↦ᵣ w_i)
-    (* current world *)
-    ∗ ▷ region W
-    ∗ ▷ sts_full_world W
     (* continuation *)
-    ∗ ▷ (PC ↦ᵣ inr (pc_p,pc_g,pc_b,pc_e,a_last) ∗ crtcls f_m a pc_p'
-         ∗ pc_b ↦ₐ[pc_p'] inr (RO,Global,b_link,e_link,a_link)
-         ∗ a_entry ↦ₐ[RO] inr (E,Global,b_m,e_m,b_m)
+    ∗ ▷ (PC ↦ᵣ inr (pc_p,pc_b,pc_e,a_last) ∗ crtcls f_m a 
+         ∗ pc_b ↦ₐ inr (RO,b_link,e_link,a_link)
+         ∗ a_entry ↦ₐ inr (E,b_m,e_m,b_m)
          (* the newly allocated region *)
-         ∗ (∃ (b e : Addr), ⌜(b + 8)%a = Some e⌝ ∧ r_t1 ↦ᵣ inr (E,Global,b,e,b)
-         ∗ [[b,e]] ↦ₐ[RWX] [[ [inl v1;inl v2;inl v3;inl v4;inl v5;inl v6;wcode;wvar] ]]
+         ∗ (∃ (b e : Addr), ⌜(b + 8)%a = Some e⌝ ∧ r_t1 ↦ᵣ inr (E,b,e,b)
+         ∗ [[b,e]] ↦ₐ [[ [inl v1;inl v2;inl v3;inl v4;inl v5;inl v6;wcode;wvar] ]]
          ∗ r_t0 ↦ᵣ cont
          ∗ r_t2 ↦ᵣ inl 0%Z
          ∗ na_own logrel_nais EN
@@ -2056,17 +1502,13 @@ Section stack_macros.
                                (<[r_t4:=inl 0%Z]>
                                 (<[r_t5:=inl 0%Z]>
                                  (<[r_t6:=inl 0%Z]>
-                                  (<[r_t7:=inl 0%Z]> rmap)))), r_i ↦ᵣ w_i)
-         (* the newly allocated region is fresh in the current world *)
-         (* ∗ ⌜Forall (λ a, a ∉ dom (gset Addr) (std W)) (region_addrs b e)⌝ *)
-         ∗ region W
-         ∗ sts_full_world W)
+                                  (<[r_t7:=inl 0%Z]> rmap)))), r_i ↦ᵣ w_i))
          -∗ WP Seq (Instr Executable) {{ φ }})
     ⊢
       WP Seq (Instr Executable) {{ λ v, φ v ∨ ⌜v = FailedV⌝ }}.
   Proof.
-    iIntros (Hvpc Hfl Hcont Hwb Ha_entry Hrmap_dom Hlocal Hlocal' HmallocN)
-            "(>Hprog & >HPC & #Hmalloc & Hna & >Hpc_b & >Ha_entry & >Hr_t0 & >Hr_t1 & >Hr_t2 & >Hregs & Hr & Hsts & Hφ)".
+    iIntros (Hvpc Hcont Hwb Ha_entry Hrmap_dom HmallocN)
+            "(>Hprog & >HPC & #Hmalloc & Hna & >Hpc_b & >Ha_entry & >Hr_t0 & >Hr_t1 & >Hr_t2 & >Hregs & Hφ)".
     (* get some registers out of regs *)
     iDestruct (big_sepL2_length with "Hprog") as %Hlength.
     assert (is_Some (rmap !! r_t6)) as [rv6 ?]. by rewrite elem_of_gmap_dom Hrmap_dom; set_solver.
@@ -2079,13 +1521,13 @@ Section stack_macros.
     destruct l;[inversion Hlength|].
     iPrologue "Hprog".
     iApply (wp_move_success_reg with "[$HPC $Hi $Hr_t6 $Hr_t1]");
-      [apply decode_encode_instrW_inv|apply Hfl|iCorrectPC a_first a_last|iContiguous_next Hcont 0|auto|].
+      [apply decode_encode_instrW_inv|iCorrectPC a_first a_last|iContiguous_next Hcont 0|].
     iEpilogue "(HPC & Hprog_done & Hr_t6 & Hr_t1)".
     (* move r_t7 r_t2 *)
     destruct l;[inversion Hlength|].
     iPrologue "Hprog".
     iApply (wp_move_success_reg with "[$HPC $Hi $Hr_t7 $Hr_t2]");
-      [apply decode_encode_instrW_inv|apply Hfl|iCorrectPC a_first a_last|iContiguous_next Hcont 1|auto|].
+      [apply decode_encode_instrW_inv|iCorrectPC a_first a_last|iContiguous_next Hcont 1|].
     iEpilogue "(HPC & Hi & Hr_t7 & Hr_t2)"; iCombine "Hi Hprog_done" as "Hprog_done".
     assert (contiguous_between (a0 :: l) a0 a_last) as Hcont'.
     { apply contiguous_between_cons_inv in Hcont as [_ (? & ? & Hcont)].
@@ -2111,8 +1553,8 @@ Section stack_macros.
       by rewrite !lookup_insert_ne //; apply Hnotin_rmap; set_solver.
     (* apply the malloc spec *)
     rewrite -/(malloc _ _ _ _).
-    iApply (malloc_spec with "[- $HPC $Hmalloc $Hna $Hpc_b $Ha_entry $Hr_t0 $Hregs $Hr $Hsts $Hmalloc_prog]");
-      [|apply Hfl|apply Hcont_fetch|apply Hwb|apply Ha_entry| |auto|lia|..].
+    iApply (malloc_spec with "[- $HPC $Hmalloc $Hna $Hpc_b $Ha_entry $Hr_t0 $Hregs $Hmalloc_prog]");
+      [|apply Hcont_fetch|apply Hwb|apply Ha_entry| |auto|lia|..].
     { intros mid Hmid. apply isCorrectPC_inrange with a_first a_last; auto.
       apply contiguous_between_bounds in Hcont_rest.
       apply contiguous_between_incr_addr with (i:=2) (ai:=a0) in Hcont;auto.
@@ -2120,7 +1562,7 @@ Section stack_macros.
     { rewrite !dom_insert_L. rewrite Hrmap_dom.
       repeat (rewrite singleton_union_difference_L all_registers_union_l).
       f_equal. clear; set_solver. }
-    iNext. iIntros "(HPC & Hmalloc_prog & Hpc_b & Ha_entry & Hbe & Hr_t0 & Hna & Hregs & Hr & Hsts)".
+    iNext. iIntros "(HPC & Hmalloc_prog & Hpc_b & Ha_entry & Hbe & Hr_t0 & Hna & Hregs)".
     iDestruct "Hbe" as (b e Hbe) "(Hr_t1 & Hbe)".
     rewrite delete_insert_delete.
     rewrite (delete_insert_ne _ r_t1 r_t2) //.
@@ -2138,7 +1580,7 @@ Section stack_macros.
     simpl.
     (* prepare the execution of the rest of the program *)
     iDestruct (big_sepL2_length with "Hprog") as %Hlength_rest.
-    assert (isCorrectPC_range pc_p pc_g pc_b pc_e link a_last) as Hvpc_rest.
+    assert (isCorrectPC_range pc_p pc_b pc_e link a_last) as Hvpc_rest.
     { intros mid Hmid. apply isCorrectPC_inrange with a_first a_last; auto.
       apply contiguous_between_incr_addr with (i:=2) (ai:=a0) in Hcont;auto.
       revert Hcont Hmid Hlink;clear. solve_addr. }
@@ -2148,7 +1590,7 @@ Section stack_macros.
     destruct h;[inversion Hlengthbe|]. 
     apply region_addrs_first in Hlt as Hfirst. rewrite -Heqh in Hfirst; inversion Hfirst. subst a2.
     apply contiguous_between_cons_inv_first in Hcontbe as Heq. subst b'. 
-    assert (∀ i a', (b :: h) !! i = Some a' -> withinBounds (RWX, Global, b, e, a') = true) as Hwbbe.
+    assert (∀ i a', (b :: h) !! i = Some a' -> withinBounds (RWX, b, e, a') = true) as Hwbbe.
     { intros i a' Hsome. apply andb_true_intro.
       apply contiguous_between_incr_addr with (i:=i) (ai:=a') in Hcontbe;[|congruence].
       apply lookup_lt_Some in Hsome. rewrite Heqh region_addrs_length in Hsome. 
@@ -2160,7 +1602,7 @@ Section stack_macros.
     iPrologue "Hprog". 
     iDestruct "Hbe" as "[Hb Hbe]". 
     iApply (wp_store_success_z with "[$HPC $Hi $Hr_t1 $Hb]");
-      [apply decode_encode_instrW_inv|apply Hfl|apply PermFlows_refl|iCorrectPC a1 a_last|iContiguous_next Hcont_rest 0|..].
+      [apply decode_encode_instrW_inv|iCorrectPC a1 a_last|iContiguous_next Hcont_rest 0|..].
     { split;auto. apply Hwbbe with 0. auto. }
     iEpilogue "(HPC & Hi & Hr_t1 & Heb)"; iCombine "Hi" "Hprog_done" as "Hprog_done". 
     (* lea r_t1 1 *)
@@ -2168,14 +1610,14 @@ Section stack_macros.
     destruct h;[inversion Hlengthbe|]. 
     iPrologue "Hprog". 
     iApply (wp_lea_success_z with "[$HPC $Hi $Hr_t1]");
-      [apply decode_encode_instrW_inv|apply Hfl|iCorrectPC a1 a_last|iContiguous_next Hcont_rest 1|iContiguous_next Hcontbe 0|simpl;auto..].
+      [apply decode_encode_instrW_inv|iCorrectPC a1 a_last|iContiguous_next Hcont_rest 1|iContiguous_next Hcontbe 0|simpl;auto..].
     iEpilogue "(HPC & Hi & Hr_t1)"; iCombine "Hi" "Hprog_done" as "Hprog_done". 
     (* store r_t1 v2 *)
     destruct l';[inversion Hlength_rest|]. 
     iPrologue "Hprog". 
     iDestruct "Hbe" as "[Hb Hbe]". 
     iApply (wp_store_success_z with "[$HPC $Hi $Hr_t1 $Hb]");
-      [apply decode_encode_instrW_inv|apply Hfl|apply PermFlows_refl|iCorrectPC a1 a_last|iContiguous_next Hcont_rest 2|..].
+      [apply decode_encode_instrW_inv|iCorrectPC a1 a_last|iContiguous_next Hcont_rest 2|..].
     { split;auto. apply Hwbbe with 1. auto. }
     iEpilogue "(HPC & Hi & Hr_t1 & Hb)"; iCombine "Hi" "Hprog_done" as "Hprog_done"; iCombine "Hb" "Heb" as "Heb". 
     (* lea r_t1 1 *)
@@ -2183,14 +1625,14 @@ Section stack_macros.
     destruct h;[inversion Hlengthbe|]. 
     iPrologue "Hprog". 
     iApply (wp_lea_success_z with "[$HPC $Hi $Hr_t1]");
-      [apply decode_encode_instrW_inv|apply Hfl|iCorrectPC a1 a_last|iContiguous_next Hcont_rest 3|iContiguous_next Hcontbe 1|simpl;auto..].
+      [apply decode_encode_instrW_inv|iCorrectPC a1 a_last|iContiguous_next Hcont_rest 3|iContiguous_next Hcontbe 1|simpl;auto..].
     iEpilogue "(HPC & Hi & Hr_t1)"; iCombine "Hi" "Hprog_done" as "Hprog_done". 
     (* store r_t1 v3 *)
     destruct l';[inversion Hlength_rest|]. 
     iPrologue "Hprog". 
     iDestruct "Hbe" as "[Hb Hbe]". 
     iApply (wp_store_success_z with "[$HPC $Hi $Hr_t1 $Hb]");
-      [apply decode_encode_instrW_inv|apply Hfl|apply PermFlows_refl|iCorrectPC a1 a_last|iContiguous_next Hcont_rest 4|..].
+      [apply decode_encode_instrW_inv|iCorrectPC a1 a_last|iContiguous_next Hcont_rest 4|..].
     { split;auto. apply Hwbbe with 2. auto. }
     iEpilogue "(HPC & Hi & Hr_t1 & Hb)"; iCombine "Hi" "Hprog_done" as "Hprog_done"; iCombine "Hb" "Heb" as "Heb". 
     (* lea r_t1 1 *)
@@ -2198,14 +1640,14 @@ Section stack_macros.
     destruct h;[inversion Hlengthbe|]. 
     iPrologue "Hprog". 
     iApply (wp_lea_success_z with "[$HPC $Hi $Hr_t1]");
-      [apply decode_encode_instrW_inv|apply Hfl|iCorrectPC a1 a_last|iContiguous_next Hcont_rest 5|iContiguous_next Hcontbe 2|simpl;auto..].
+      [apply decode_encode_instrW_inv|iCorrectPC a1 a_last|iContiguous_next Hcont_rest 5|iContiguous_next Hcontbe 2|simpl;auto..].
     iEpilogue "(HPC & Hi & Hr_t1)"; iCombine "Hi" "Hprog_done" as "Hprog_done". 
     (* store r_t1 v4 *)
     destruct l';[inversion Hlength_rest|]. 
     iPrologue "Hprog". 
     iDestruct "Hbe" as "[Hb Hbe]". 
     iApply (wp_store_success_z with "[$HPC $Hi $Hr_t1 $Hb]");
-      [apply decode_encode_instrW_inv|apply Hfl|apply PermFlows_refl|iCorrectPC a1 a_last|iContiguous_next Hcont_rest 6|..].
+      [apply decode_encode_instrW_inv|iCorrectPC a1 a_last|iContiguous_next Hcont_rest 6|..].
     { split;auto. apply Hwbbe with 3. auto. }
     iEpilogue "(HPC & Hi & Hr_t1 & Hb)"; iCombine "Hi" "Hprog_done" as "Hprog_done"; iCombine "Hb" "Heb" as "Heb". 
     (* lea r_t1 1 *)
@@ -2213,14 +1655,14 @@ Section stack_macros.
     destruct h;[inversion Hlengthbe|]. 
     iPrologue "Hprog". 
     iApply (wp_lea_success_z with "[$HPC $Hi $Hr_t1]");
-      [apply decode_encode_instrW_inv|apply Hfl|iCorrectPC a1 a_last|iContiguous_next Hcont_rest 7|iContiguous_next Hcontbe 3|simpl;auto..].
+      [apply decode_encode_instrW_inv|iCorrectPC a1 a_last|iContiguous_next Hcont_rest 7|iContiguous_next Hcontbe 3|simpl;auto..].
     iEpilogue "(HPC & Hi & Hr_t1)"; iCombine "Hi" "Hprog_done" as "Hprog_done". 
     (* store r_t1 v5 *)
     destruct l';[inversion Hlength_rest|]. 
     iPrologue "Hprog". 
     iDestruct "Hbe" as "[Hb Hbe]". 
     iApply (wp_store_success_z with "[$HPC $Hi $Hr_t1 $Hb]");
-      [apply decode_encode_instrW_inv|apply Hfl|apply PermFlows_refl|iCorrectPC a1 a_last|iContiguous_next Hcont_rest 8|..].
+      [apply decode_encode_instrW_inv|iCorrectPC a1 a_last|iContiguous_next Hcont_rest 8|..].
     { split;auto. apply Hwbbe with 4. auto. }
     iEpilogue "(HPC & Hi & Hr_t1 & Hb)"; iCombine "Hi" "Hprog_done" as "Hprog_done"; iCombine "Hb" "Heb" as "Heb". 
     (* lea r_t1 1 *)
@@ -2228,14 +1670,14 @@ Section stack_macros.
     destruct h;[inversion Hlengthbe|]. 
     iPrologue "Hprog". 
     iApply (wp_lea_success_z with "[$HPC $Hi $Hr_t1]");
-      [apply decode_encode_instrW_inv|apply Hfl|iCorrectPC a1 a_last|iContiguous_next Hcont_rest 9|iContiguous_next Hcontbe 4|simpl;auto..].
+      [apply decode_encode_instrW_inv|iCorrectPC a1 a_last|iContiguous_next Hcont_rest 9|iContiguous_next Hcontbe 4|simpl;auto..].
     iEpilogue "(HPC & Hi & Hr_t1)"; iCombine "Hi" "Hprog_done" as "Hprog_done". 
     (* store r_t1 v6 *)
     destruct l';[inversion Hlength_rest|]. 
     iPrologue "Hprog". 
     iDestruct "Hbe" as "[Hb Hbe]". 
     iApply (wp_store_success_z with "[$HPC $Hi $Hr_t1 $Hb]");
-      [apply decode_encode_instrW_inv|apply Hfl|apply PermFlows_refl|iCorrectPC a1 a_last|iContiguous_next Hcont_rest 10|..].
+      [apply decode_encode_instrW_inv|iCorrectPC a1 a_last|iContiguous_next Hcont_rest 10|..].
     { split;auto. apply Hwbbe with 5. auto. }
     iEpilogue "(HPC & Hi & Hr_t1 & Hb)"; iCombine "Hi" "Hprog_done" as "Hprog_done"; iCombine "Hb" "Heb" as "Heb". 
     (* lea r_t1 1 *)
@@ -2243,7 +1685,7 @@ Section stack_macros.
     destruct h;[inversion Hlengthbe|]. 
     iPrologue "Hprog". 
     iApply (wp_lea_success_z with "[$HPC $Hi $Hr_t1]");
-      [apply decode_encode_instrW_inv|apply Hfl|iCorrectPC a1 a_last|iContiguous_next Hcont_rest 11|iContiguous_next Hcontbe 5|simpl;auto..].
+      [apply decode_encode_instrW_inv|iCorrectPC a1 a_last|iContiguous_next Hcont_rest 11|iContiguous_next Hcontbe 5|simpl;auto..].
     iEpilogue "(HPC & Hi & Hr_t1)"; iCombine "Hi" "Hprog_done" as "Hprog_done". 
     (* store r_t1 r_t6 *)
     (* first we must extract r_t6 *)
@@ -2254,22 +1696,21 @@ Section stack_macros.
     iPrologue "Hprog". 
     iDestruct "Hbe" as "[Hb Hbe]". 
     iApply (wp_store_success_reg with "[$HPC $Hi $Hr_t6 $Hr_t1 $Hb]");
-      [apply decode_encode_instrW_inv|apply Hfl|apply PermFlows_refl|iCorrectPC a1 a_last|iContiguous_next Hcont_rest 12|..].
+      [apply decode_encode_instrW_inv|iCorrectPC a1 a_last|iContiguous_next Hcont_rest 12|..].
     { split;auto. apply Hwbbe with 6. auto. }
-    { auto. }
     iEpilogue "(HPC & Hi & Hr_t6 & Hr_t1 & Hb)"; iCombine "Hi" "Hprog_done" as "Hprog_done"; iCombine "Hb" "Heb" as "Heb".
     (* move r_t6 0 *)
     destruct l';[inversion Hlength_rest|]. 
     iPrologue "Hprog". 
     iApply (wp_move_success_z with "[$HPC $Hi $Hr_t6]");
-      [apply decode_encode_instrW_inv|apply Hfl|iCorrectPC a1 a_last|iContiguous_next Hcont_rest 13|auto..].
+      [apply decode_encode_instrW_inv|iCorrectPC a1 a_last|iContiguous_next Hcont_rest 13|auto..].
     iEpilogue "(HPC & Hi & Hr_t6)"; iCombine "Hi" "Hprog_done" as "Hprog_done".
     (* lea r_t1 1 *)
     destruct l';[inversion Hlength_rest|].
     destruct h;[inversion Hlengthbe|]. 
     iPrologue "Hprog". 
     iApply (wp_lea_success_z with "[$HPC $Hi $Hr_t1]");
-      [apply decode_encode_instrW_inv|apply Hfl|iCorrectPC a1 a_last|iContiguous_next Hcont_rest 14|iContiguous_next Hcontbe 6|simpl;auto..].
+      [apply decode_encode_instrW_inv|iCorrectPC a1 a_last|iContiguous_next Hcont_rest 14|iContiguous_next Hcontbe 6|simpl;auto..].
     iEpilogue "(HPC & Hi & Hr_t1)"; iCombine "Hi" "Hprog_done" as "Hprog_done". 
     (* store r_t1 r_t7 *)
     (* first we must extract r_t7 *)
@@ -2281,15 +1722,14 @@ Section stack_macros.
     iPrologue "Hprog". 
     iDestruct "Hbe" as "[Hb Hbe]". 
     iApply (wp_store_success_reg with "[$HPC $Hi $Hr_t7 $Hr_t1 $Hb]");
-      [apply decode_encode_instrW_inv|apply Hfl|apply PermFlows_refl|iCorrectPC a1 a_last|iContiguous_next Hcont_rest 15|..].
+      [apply decode_encode_instrW_inv|iCorrectPC a1 a_last|iContiguous_next Hcont_rest 15|..].
     { split;auto. apply Hwbbe with 7. auto. }
-    { auto. }
     iEpilogue "(HPC & Hi & Hr_t7 & Hr_t1 & Hb)"; iCombine "Hi" "Hprog_done" as "Hprog_done"; iCombine "Hb" "Heb" as "Heb".
     (* move r_t7 0 *)
     destruct l';[inversion Hlength_rest|]. 
     iPrologue "Hprog". 
     iApply (wp_move_success_z with "[$HPC $Hi $Hr_t7]");
-      [apply decode_encode_instrW_inv|apply Hfl|iCorrectPC a1 a_last|iContiguous_next Hcont_rest 16|auto..].
+      [apply decode_encode_instrW_inv|iCorrectPC a1 a_last|iContiguous_next Hcont_rest 16|auto..].
     iEpilogue "(HPC & Hi & Hr_t7)"; iCombine "Hi" "Hprog_done" as "Hprog_done".
     (* put r_t6 and r_t7 back *)
     iDestruct (big_sepM_insert with "[$Hregs $Hr_t7]") as "Hregs". by rewrite lookup_delete.
@@ -2305,30 +1745,30 @@ Section stack_macros.
     assert ((a23 + (-7))%a = Some b) as Hlea.
     { apply contiguous_between_length in Hcontbe. revert Hbe Hnext Hcontbe; clear. solve_addr. }
     iApply (wp_lea_success_z with "[$HPC $Hi $Hr_t1]");
-      [apply decode_encode_instrW_inv|apply Hfl|iCorrectPC a1 a_last|iContiguous_next Hcont_rest 17|apply Hlea|simpl;auto..].
+      [apply decode_encode_instrW_inv|iCorrectPC a1 a_last|iContiguous_next Hcont_rest 17|apply Hlea|simpl;auto..].
     iEpilogue "(HPC & Hi & Hr_t1)";iCombine "Hi" "Hprog_done" as "Hprog_done". 
     (* restrict r_t1 (Global,E) *)
     destruct l';[|inversion Hlength_rest].
     apply contiguous_between_last with (ai:=a26) in Hcont_rest as Hlast; auto.
     iPrologue "Hprog". iClear "Hprog". 
     iApply (wp_restrict_success_z with "[$HPC $Hi $Hr_t1]");
-      [apply decode_encode_instrW_inv|apply Hfl|iCorrectPC a1 a_last|apply Hlast|auto..].
-    { rewrite decode_encode_permPair_inv. auto. }
-    rewrite decode_encode_permPair_inv.
+      [apply decode_encode_instrW_inv|iCorrectPC a1 a_last|apply Hlast|auto..].
+    { rewrite decode_encode_perm_inv. auto. }
+    rewrite decode_encode_perm_inv.
     iEpilogue "(HPC & Hi & Hr_t1)"; iCombine "Hi" "Hprog_done" as "Hprog_done".
     (* continuation *)
     iApply "Hφ".
     iFrame "HPC Hpc_b Ha_entry". iSplitL "Hprog_done".
     { rewrite Heqapp.
-      repeat iDestruct "Hprog_done" as "[$ Hprog_done]". iFrame. done. 
+      do 21 iDestruct "Hprog_done" as "[$ Hprog_done]". iFrame. done. 
     }
     iExists b,e. iSplitR;auto.
     iFrame "Hr_t1 Hr_t0".
     iSplitL "Heb".
-    { rewrite -Heqh. repeat iDestruct "Heb" as "[$ Heb]". iFrame. done. }
+    { rewrite -Heqh. do 7 iDestruct "Heb" as "[$ Heb]". iFrame. done. }
     iDestruct (big_sepM_delete _ _ r_t2 with "Hregs") as "[Hr_t2 Hregs]".
       by do 2 (rewrite lookup_insert_ne //); rewrite lookup_insert //.
-    iFrame "Hr Hsts Hr_t2 Hna".
+    iFrame "Hr_t2 Hna".
     repeat (rewrite delete_insert_ne //; []). rewrite delete_insert_delete.
     rewrite !delete_insert_ne // !delete_notin; [| apply Hnotin_rmap; set_solver ..].
     repeat (rewrite (insert_commute _ r_t6) //;[]). rewrite insert_insert.
@@ -2337,24 +1777,23 @@ Section stack_macros.
 
   (* ------------------------------- Closure Activation --------------------------------- *)
 
-  Lemma closure_activation_spec pc_p pc_g b_cls e_cls r1v renvv wcode wenv φ :
-    PermFlows pc_p RWX →
+  Lemma closure_activation_spec pc_p b_cls e_cls r1v renvv wcode wenv φ :
     readAllowed pc_p = true →
-    isCorrectPC_range pc_p pc_g b_cls e_cls b_cls e_cls →
+    isCorrectPC_range pc_p b_cls e_cls b_cls e_cls →
     pc_p ≠ E →
-    PC ↦ᵣ inr (pc_p, pc_g, b_cls, e_cls, b_cls)
+    PC ↦ᵣ inr (pc_p, b_cls, e_cls, b_cls)
     ∗ r_t1 ↦ᵣ r1v
     ∗ r_env ↦ᵣ renvv
-    ∗ [[b_cls, e_cls]]↦ₐ[RWX][[ [inl v1; inl v2; inl v3; inl v4; inl v5; inl v6; wcode; wenv] ]]
+    ∗ [[b_cls, e_cls]]↦ₐ[[ [inl v1; inl v2; inl v3; inl v4; inl v5; inl v6; wcode; wenv] ]]
     ∗ (  PC ↦ᵣ updatePcPerm wcode
        ∗ r_t1 ↦ᵣ wcode
        ∗ r_env ↦ᵣ wenv
-       ∗ [[b_cls, e_cls]]↦ₐ[RWX][[ [inl v1; inl v2; inl v3; inl v4; inl v5; inl v6; wcode; wenv] ]]
+       ∗ [[b_cls, e_cls]]↦ₐ[[ [inl v1; inl v2; inl v3; inl v4; inl v5; inl v6; wcode; wenv] ]]
        -∗ WP Seq (Instr Executable) {{ φ }})
     ⊢
       WP Seq (Instr Executable) {{ φ }}.
   Proof.
-    iIntros (Hfl Hrpc Hvpc HnpcE) "(HPC & Hr1 & Hrenv & Hcls & Hcont)".
+    iIntros (Hrpc Hvpc HnpcE) "(HPC & Hr1 & Hrenv & Hcls & Hcont)".
     rewrite /region_mapsto.
     iDestruct (big_sepL2_length with "Hcls") as %Hcls_len. simpl in Hcls_len.
     assert (b_cls + 8 = Some e_cls)%a as Hbe.
@@ -2373,17 +1812,16 @@ Section stack_macros.
     (* move r_t1 PC *)
     iPrologue "Hcls_code".
     iApply (wp_move_success_reg_fromPC with "[$HPC $Hi $Hr1]");
-      [apply decode_encode_instrW_inv| done | iCorrectPC b_cls e_cls |
-       iContiguous_next Hcont_cls 0 | done | ..].
+      [apply decode_encode_instrW_inv| iCorrectPC b_cls e_cls |
+       iContiguous_next Hcont_cls 0 |..].
     iEpilogue "(HPC & Hprog_done & Hr1)".
     (* lea r_t1 7 *)
     iPrologue "Hprog".
     iApply (wp_lea_success_z with "[$HPC $Hi $Hr1]");
-      [apply decode_encode_instrW_inv| done | iCorrectPC b_cls e_cls |
-       iContiguous_next Hcont_cls 1 | | done | done | ..].
+      [apply decode_encode_instrW_inv | iCorrectPC b_cls e_cls |
+       iContiguous_next Hcont_cls 1 | | done | ..].
     { eapply contiguous_between_incr_addr_middle' with (i:=0); eauto.
       cbn. clear. lia. }
-    { destruct pc_p; simpl in *; try discriminate; auto. }
     iEpilogue "(HPC & Hi & Hr1)". iCombine "Hi Hprog_done" as "Hprog_done".
     (* load r_env r_t1 *)
     iPrologue "Hprog".
@@ -2392,21 +1830,20 @@ Section stack_macros.
     { apply Z.eqb_neq. intros Heqb. assert (a5 = a0) as ->. revert Heqb; clear; solve_addr.
       exfalso. by pose proof (NoDup_lookup _ 2 7 _ Hcls_nodup eq_refl eq_refl). }
     iApply (wp_load_success with "[$HPC $Hi $Hrenv $Hr1 Hcls_env]");
-      [apply decode_encode_instrW_inv | done | iCorrectPC b_cls e_cls |
+      [apply decode_encode_instrW_inv | iCorrectPC b_cls e_cls |
        split;[done|] | iContiguous_next Hcont_cls 2 | ..].
     { eapply contiguous_between_middle_bounds' in Hcont_cls as [? ?].
       by eapply le_addr_withinBounds; eauto. repeat constructor. }
-    { rewrite H_5_0. iFrame. eauto. }
+    { rewrite H_5_0. iFrame. }
     iEpilogue "(HPC & Hrenv & Hi & Hr1 & Hcls_env)". rewrite H_5_0.
     iCombine "Hi Hprog_done" as "Hprog_done".
     (* lea r_t1 (-1) *)
     iPrologue "Hprog".
     iApply (wp_lea_success_z with "[$HPC $Hi $Hr1]");
-      [apply decode_encode_instrW_inv | done | iCorrectPC b_cls e_cls |
-       iContiguous_next Hcont_cls 3 | | done | done | ..].
+      [apply decode_encode_instrW_inv | iCorrectPC b_cls e_cls |
+       iContiguous_next Hcont_cls 3 | | done | ..].
     { assert ((a4 + 1)%a = Some a5) as HH. by iContiguous_next Hcont_cls 6.
       instantiate (1 := a4). revert HH. clear; solve_addr. }
-    { destruct pc_p; simpl in *; try discriminate; auto. }
     iEpilogue "(HPC & Hi & Hr1)". iCombine "Hi Hprog_done" as "Hprog_done".
     (* load r_t1 r_t1 *)
     iPrologue "Hprog".
@@ -2415,20 +1852,20 @@ Section stack_macros.
     { apply Z.eqb_neq. intros Heqb. assert (a4 = a2) as ->. revert Heqb; clear; solve_addr.
       exfalso. by pose proof (NoDup_lookup _ 4 6 _ Hcls_nodup eq_refl eq_refl). }
     iApply (wp_load_success_same with "[$HPC $Hi $Hr1 Hcls_ptr]");
-      [(* FIXME *) auto | apply decode_encode_instrW_inv | done | iCorrectPC b_cls e_cls |
+      [(* FIXME *) auto | apply decode_encode_instrW_inv | iCorrectPC b_cls e_cls |
        split;[done|] | iContiguous_next Hcont_cls 4 | ..].
     { eapply contiguous_between_middle_bounds' in Hcont_cls as [? ?].
       by eapply le_addr_withinBounds; eauto. repeat constructor. }
-    { rewrite H_4_2. iFrame. eauto. }
+    { rewrite H_4_2. iFrame. }
     iEpilogue "(HPC & Hr1 & Hi & Hcls_ptr)". rewrite H_4_2.
     iCombine "Hi Hprog_done" as "Hprog_done".
     (* jmp r_t1 *)
     iPrologue "Hprog".
     iApply (wp_jmp_success with "[$HPC $Hi $Hr1]");
-      [apply decode_encode_instrW_inv | done | iCorrectPC b_cls e_cls | .. ].
+      [apply decode_encode_instrW_inv | iCorrectPC b_cls e_cls | .. ].
     iEpilogue "(HPC & Hi & Hr1)".
 
-    iApply "Hcont". repeat (iDestruct "Hprog_done" as "(? & Hprog_done)"). iFrame.
+    iApply "Hcont". do 4 (iDestruct "Hprog_done" as "(? & Hprog_done)"). iFrame.
   Qed.
 
-End stack_macros.
+End macros.
