theories/examples/macros_helpers.v
@@ -8,45 +8,45 @@ Section helpers.
 
   (* ---------------------------- Helper Lemmas --------------------------------------- *)
 
-  Definition isCorrectPC_range p g b e a0 an :=
-    ∀ ai, (a0 <= ai)%a ∧ (ai < an)%a → isCorrectPC (inr (p, g, b, e, ai)).
+  Definition isCorrectPC_range p b e a0 an :=
+    ∀ ai, (a0 <= ai)%a ∧ (ai < an)%a → isCorrectPC (inr (p, b, e, ai)).
 
-  Lemma isCorrectPC_inrange p g b (e a0 an a: Addr) :
-    isCorrectPC_range p g b e a0 an →
+  Lemma isCorrectPC_inrange p b (e a0 an a: Addr) :
+    isCorrectPC_range p b e a0 an →
     (a0 <= a < an)%Z →
-    isCorrectPC (inr (p, g, b, e, a)).
+    isCorrectPC (inr (p, b, e, a)).
   Proof.
     unfold isCorrectPC_range. move=> /(_ a) HH ?. apply HH. eauto.
   Qed.
 
-  Lemma isCorrectPC_contiguous_range p g b e a0 an a l :
-    isCorrectPC_range p g b e a0 an →
+  Lemma isCorrectPC_contiguous_range p b e a0 an a l :
+    isCorrectPC_range p b e a0 an →
     contiguous_between l a0 an →
     a ∈ l →
-    isCorrectPC (inr (p, g, b, e, a)).
+    isCorrectPC (inr (p, b, e, a)).
   Proof.
     intros Hr Hc Hin.
     eapply isCorrectPC_inrange; eauto.
     eapply contiguous_between_middle_bounds'; eauto.
   Qed.
 
-  Lemma isCorrectPC_range_perm p g b e a0 an :
-    isCorrectPC_range p g b e a0 an →
+  Lemma isCorrectPC_range_perm p b e a0 an :
+    isCorrectPC_range p b e a0 an →
     (a0 < an)%a →
-    p = RX ∨ p = RWX ∨ p = RWLX.
+    p = RX ∨ p = RWX.
   Proof.
     intros Hr H0n.
-    assert (isCorrectPC (inr (p, g, b, e, a0))) as HH by (apply Hr; solve_addr).
+    assert (isCorrectPC (inr (p, b, e, a0))) as HH by (apply Hr; solve_addr).
     inversion HH; auto.
   Qed.
 
-  Lemma isCorrectPC_range_npE p g b e a0 an :
-    isCorrectPC_range p g b e a0 an →
+  Lemma isCorrectPC_range_npE p b e a0 an :
+    isCorrectPC_range p b e a0 an →
     (a0 < an)%a →
     p ≠ E.
   Proof.
     intros HH1 HH2.
-    destruct (isCorrectPC_range_perm _ _ _ _ _ _ HH1 HH2) as [?| [?|?] ];
+    destruct (isCorrectPC_range_perm _ _ _ _ _ HH1 HH2) as [?| ? ];
       congruence.
   Qed.
 
