theories/examples/malloc.v
@@ -19,8 +19,7 @@ From cap_machine.examples Require Import contiguous.
 
 Section SimpleMalloc.
   Context {Σ:gFunctors} {memg:memG Σ} {regg:regG Σ}
-          {stsg : STSG Addr region_type Σ} {heapg : heapG Σ}
-          `{MonRef: MonRefG (leibnizO _) CapR_rtc Σ} {nainv: logrel_na_invs Σ}
+          {nainv: logrel_na_invs Σ}
           `{MP: MachineParameters}.
 
   Definition malloc_subroutine_instrs' (offset: Z) :=
@@ -78,9 +77,9 @@ Section SimpleMalloc.
 
   Definition malloc_inv (b e : Addr) : iProp Σ :=
     (∃ b_m a_m,
-       [[b, b_m]] ↦ₐ[RX] [[ malloc_subroutine_instrs ]]
-     ∗ b_m ↦ₐ[RWX] (inr (RWX, Global, b_m, e, a_m))
-     ∗ [[a_m, e]] ↦ₐ[RWX] [[ region_addrs_zeroes a_m e ]]
+       [[b, b_m]] ↦ₐ [[ malloc_subroutine_instrs ]]
+     ∗ b_m ↦ₐ (inr (RWX, b_m, e, a_m))
+     ∗ [[a_m, e]] ↦ₐ [[ region_addrs_zeroes a_m e ]]
      ∗ ⌜(b_m < a_m)%a ∧ (a_m <= e)%a⌝
     )%I.
 
@@ -92,7 +91,7 @@ Section SimpleMalloc.
      ∗ na_own logrel_nais E
      ∗ ([∗ map] r↦w ∈ rmap, r ↦ᵣ w)
      ∗ r_t0 ↦ᵣ cont
-     ∗ PC ↦ᵣ inr (RX, Global, b, e, b)
+     ∗ PC ↦ᵣ inr (RX, b, e, b)
      ∗ r_t1 ↦ᵣ inl size
      ∗ ▷ ((na_own logrel_nais E
           ∗ [∗ map] r↦w ∈ <[r_t2 := inl 0%Z]>
@@ -103,8 +102,8 @@ Section SimpleMalloc.
           ∗ PC ↦ᵣ updatePcPerm cont
           ∗ (∃ (ba ea : Addr),
             ⌜(ba + size)%a = Some ea⌝
-            ∗ r_t1 ↦ᵣ inr (RWX, Global, ba, ea, ba)
-            ∗ [[ba, ea]] ↦ₐ[RWX] [[region_addrs_zeroes ba ea]])
+            ∗ r_t1 ↦ᵣ inr (RWX, ba, ea, ba)
+            ∗ [[ba, ea]] ↦ₐ [[region_addrs_zeroes ba ea]])
           -∗ WP Seq (Instr Executable) {{ φ }}))
     ⊢ WP Seq (Instr Executable) {{ λ v, φ v ∨ ⌜v = FailedV⌝ }}%I.
   Proof.
@@ -139,7 +138,7 @@ Section SimpleMalloc.
     { apply contiguous_between_of_region_addrs; eauto.
       rewrite /malloc_subroutine_instrs_length in Hb_bm. solve_addr. }
 
-    assert (HPC: ∀ a, a ∈ ai → isCorrectPC (inr (RX, Global, b, e, a))).
+    assert (HPC: ∀ a, a ∈ ai → isCorrectPC (inr (RX, b, e, a))).
     { intros a Ha.
       pose proof (contiguous_between_middle_bounds' _ _ _ _ Hcont Ha) as [? ?].
       constructor; eauto. solve_addr. }
@@ -150,16 +149,15 @@ Section SimpleMalloc.
     pose proof (contiguous_between_cons_inv_first _ _ _ _ Hcont) as ->.
     iPrologue "Hprog".
     iApply (wp_move_success_reg_fromPC with "[$HPC $Hi $Hr2]");
-      [apply decode_encode_instrW_inv|done| |iContiguous_next Hcont 0|done|..].
+      [apply decode_encode_instrW_inv| |iContiguous_next Hcont 0| |..].
     { apply HPC; repeat constructor. }
     iEpilogue "(HPC & Hprog_done & Hr2)".
     (* lea r_t2 malloc_instrs_length *)
     destruct l as [|? l];[inversion Hprog_len|].
     iPrologue "Hprog".
     iApply (wp_lea_success_z with "[$HPC $Hi $Hr2]");
-      [apply decode_encode_instrW_inv|done| |iContiguous_next Hcont 1|done|done|done|..].
+      [apply decode_encode_instrW_inv| |iContiguous_next Hcont 1|done|done|..].
     { apply HPC; repeat constructor. }
-    { simpl; auto. }
     iEpilogue "(HPC & Hi & Hr2)". iCombine "Hi" "Hprog_done" as "Hprog_done".
     (* load r_t2 r_t2 *)
     destruct l as [|? l];[inversion Hprog_len|].
@@ -170,21 +168,21 @@ Section SimpleMalloc.
       pose proof (contiguous_between_middle_bounds _ 2 a _ _ Hcont eq_refl) as [? ?].
       solve_addr. }
     iApply (wp_load_success_same with "[$HPC $Hi $Hr2 Hmemptr]");
-      [auto(*FIXME*)|apply decode_encode_instrW_inv|done| |split;try done
+      [auto(*FIXME*)|apply decode_encode_instrW_inv| |split;try done
        |iContiguous_next Hcont 2|..].
     { apply HPC; repeat constructor. }
     { apply le_addr_withinBounds.
       - generalize (contiguous_between_length _ _ _ Hcont). cbn.
         clear; solve_addr.
       - revert Hbm_am Ham_e; solve_addr. }
-    { rewrite Hbm_a; iFrame. done. }
+    { rewrite Hbm_a; iFrame. }
     rewrite Hbm_a. iEpilogue "(HPC & Hr2 & Hi & Hmemptr)".
     iCombine "Hi" "Hprog_done" as "Hprog_done".
     (* geta r_t3 r_t2 *)
     destruct l as [|? l];[inversion Hprog_len|].
     iPrologue "Hprog".
     iApply (wp_Get_success with "[$HPC $Hi $Hr3 $Hr2]");
-      [apply decode_encode_instrW_inv|done|done| |iContiguous_next Hcont 3|done|done|..].
+      [apply decode_encode_instrW_inv|done| |iContiguous_next Hcont 3|..].
     { apply HPC; repeat constructor. }
     iEpilogue "(HPC & Hi & Hr2 & Hr3)". iCombine "Hi" "Hprog_done" as "Hprog_done".
     cbn [rules_Get.denote].
@@ -201,7 +199,7 @@ Section SimpleMalloc.
       iDestruct (big_sepM_insert with "[$Hregs $Hr2]") as "Hregs".
         by rewrite !lookup_insert_ne // lookup_empty.
       iApply (wp_lea with "[$Hregs $Hi]");
-        [apply decode_encode_instrW_inv|done| |done|..].
+        [apply decode_encode_instrW_inv| |done|..].
       { apply HPC; repeat constructor. }
       { rewrite /regs_of /regs_of_argument !dom_insert_L dom_empty_L. set_solver-. }
       iNext. iIntros (regs' retv) "(Hspec & ? & ?)". iDestruct "Hspec" as %Hspec.
@@ -210,15 +208,14 @@ Section SimpleMalloc.
       { cbn. iApply wp_pure_step_later; auto. iNext.
         iApply wp_value. auto. } }
     iApply (wp_lea_success_reg with "[$HPC $Hi $Hr2 $Hr1]");
-      [apply decode_encode_instrW_inv|done| |iContiguous_next Hcont 4|done|done|done|..].
+      [apply decode_encode_instrW_inv| |iContiguous_next Hcont 4|done|done|..].
     { apply HPC; repeat constructor. }
-    { simpl; auto. }
     iEpilogue "(HPC & Hi & Hr1 & Hr2)". iCombine "Hi" "Hprog_done" as "Hprog_done".
     (* geta r_t1 r_t2 *)
     destruct l as [|? l];[inversion Hprog_len|].
     iPrologue "Hprog".
     iApply (wp_Get_success with "[$HPC $Hi $Hr1 $Hr2]");
-      [apply decode_encode_instrW_inv|done|done| |iContiguous_next Hcont 5|done|done|..].
+      [apply decode_encode_instrW_inv|done| |iContiguous_next Hcont 5|..].
     { apply HPC; repeat constructor. }
     iEpilogue "(HPC & Hi & Hr2 & Hr1)". iCombine "Hi" "Hprog_done" as "Hprog_done".
     cbn [rules_Get.denote].
@@ -226,7 +223,7 @@ Section SimpleMalloc.
     destruct l as [|? l];[inversion Hprog_len|].
     iPrologue "Hprog".
     iApply (wp_move_success_reg with "[$HPC $Hi $Hr4 $Hr2]");
-      [apply decode_encode_instrW_inv|done| |iContiguous_next Hcont 6|done|..].
+      [apply decode_encode_instrW_inv| |iContiguous_next Hcont 6|..].
     { apply HPC; repeat constructor. }
     iEpilogue "(HPC & Hi & Hr4 & Hr2)". iCombine "Hi" "Hprog_done" as "Hprog_done".
     (* subseg r_t4 r_t3 r_t1 *)
@@ -244,7 +241,7 @@ Section SimpleMalloc.
       iDestruct (big_sepM_insert with "[$Hregs $Hr4]") as "Hregs".
         by rewrite !lookup_insert_ne // lookup_empty.
       iApply (wp_Subseg with "[$Hregs $Hi]");
-        [apply decode_encode_instrW_inv|done| |done|..].
+        [apply decode_encode_instrW_inv| |done|..].
       { apply HPC; repeat constructor. }
       { rewrite /regs_of /regs_of_argument !dom_insert_L dom_empty_L. set_solver-. }
       iNext. iIntros (regs' retv) "(Hspec & ? & ?)". iDestruct "Hspec" as %Hspec.
@@ -254,7 +251,7 @@ Section SimpleMalloc.
         congruence. }
       { cbn. iApply wp_pure_step_later; auto. iNext. iApply wp_value. auto. } }
     iApply (wp_subseg_success with "[$HPC $Hi $Hr4 $Hr3 $Hr1]");
-      [apply decode_encode_instrW_inv|done| |split;apply z_to_addr_z_of|done|done|done|..].
+      [apply decode_encode_instrW_inv| |split;apply z_to_addr_z_of|done|done|..].
     { apply HPC; repeat constructor. }
     { iContiguous_next Hcont 7. }
     iEpilogue "(HPC & Hi & Hr3 & Hr1 & Hr4)". iCombine "Hi" "Hprog_done" as "Hprog_done".
@@ -262,7 +259,7 @@ Section SimpleMalloc.
     destruct l as [|? l];[inversion Hprog_len|].
     iPrologue "Hprog".
     iApply (wp_add_sub_lt_success_dst_r with "[$HPC $Hi $Hr1 $Hr3]");
-      [apply decode_encode_instrW_inv|done|iContiguous_next Hcont 8|done|..].
+      [apply decode_encode_instrW_inv|done|iContiguous_next Hcont 8|..].
     { apply HPC; repeat constructor. }
     iEpilogue "(HPC & Hi & Hr1 & Hr3)". iCombine "Hi" "Hprog_done" as "Hprog_done".
     cbn [denote].
@@ -270,23 +267,22 @@ Section SimpleMalloc.
     destruct l as [|? l];[inversion Hprog_len|].
     iPrologue "Hprog".
     iApply (wp_lea_success_reg with "[$HPC $Hi $Hr4 $Hr3]");
-      [apply decode_encode_instrW_inv|done| |iContiguous_next Hcont 9| |done|done|..].
+      [apply decode_encode_instrW_inv| |iContiguous_next Hcont 9| |done|..].
     { apply HPC; repeat constructor. }
     { transitivity (Some a_m); auto. clear; solve_addr. }
-    { simpl; auto. }
     iEpilogue "(HPC & Hi & Hr3 & Hr4)". iCombine "Hi" "Hprog_done" as "Hprog_done".
     (* move r_t3 r_t2 *)
     destruct l as [|? l];[inversion Hprog_len|].
     iPrologue "Hprog".
     iApply (wp_move_success_reg with "[$HPC $Hi $Hr3 $Hr2]");
-      [apply decode_encode_instrW_inv|done| |iContiguous_next Hcont 10|done|..].
+      [apply decode_encode_instrW_inv| |iContiguous_next Hcont 10|..].
     { apply HPC; repeat constructor. }
     iEpilogue "(HPC & Hi & Hr3 & Hr2)". iCombine "Hi" "Hprog_done" as "Hprog_done".
     (* sub r_t1 0 r_t1 *)
     destruct l as [|? l];[inversion Hprog_len|].
     iPrologue "Hprog".
     iApply (wp_add_sub_lt_success_z_dst with "[$HPC $Hi $Hr1]");
-      [apply decode_encode_instrW_inv|done|iContiguous_next Hcont 11|done|..].
+      [apply decode_encode_instrW_inv|done|iContiguous_next Hcont 11|..].
     { apply HPC; repeat constructor. }
     iEpilogue "(HPC & Hi & Hr1)". iCombine "Hi" "Hprog_done" as "Hprog_done".
     cbn [denote].
@@ -294,16 +290,15 @@ Section SimpleMalloc.
     destruct l as [|? l];[inversion Hprog_len|].
     iPrologue "Hprog".
     iApply (wp_lea_success_reg with "[$HPC $Hi $Hr3 $Hr1]");
-      [apply decode_encode_instrW_inv|done| |iContiguous_next Hcont 12| |done|done|..].
+      [apply decode_encode_instrW_inv| |iContiguous_next Hcont 12| |done|..].
     { apply HPC; repeat constructor. }
     { transitivity (Some 0)%a; auto. clear; solve_addr. }
-    { simpl; auto. }
     iEpilogue "(HPC & Hi & Hr1 & Hr3)". iCombine "Hi" "Hprog_done" as "Hprog_done".
     (* getb r_t1 r_t3 *)
     destruct l as [|? l];[inversion Hprog_len|].
     iPrologue "Hprog".
     iApply (wp_Get_success with "[$HPC $Hi $Hr1 $Hr3]");
-      [apply decode_encode_instrW_inv|done|done| |iContiguous_next Hcont 13|done|done|..].
+      [apply decode_encode_instrW_inv|done| |iContiguous_next Hcont 13|..].
     { apply HPC; repeat constructor. }
     iEpilogue "(HPC & Hi & Hr3 & Hr1)". iCombine "Hi" "Hprog_done" as "Hprog_done".
     cbn [rules_Get.denote].
@@ -311,16 +306,15 @@ Section SimpleMalloc.
     destruct l as [|? l];[inversion Hprog_len|].
     iPrologue "Hprog".
     iApply (wp_lea_success_reg with "[$HPC $Hi $Hr3 $Hr1]");
-      [apply decode_encode_instrW_inv|done| |iContiguous_next Hcont 14| |done|done|..].
+      [apply decode_encode_instrW_inv| |iContiguous_next Hcont 14| |done|..].
     { apply HPC; repeat constructor. }
     { transitivity (Some b_m)%a; auto. clear; solve_addr. }
-    { simpl; auto. }
     iEpilogue "(HPC & Hi & Hr1 & Hr3)". iCombine "Hi" "Hprog_done" as "Hprog_done".
     (* store r_t3 r_t2 *)
     destruct l as [|? l];[inversion Hprog_len|].
     iPrologue "Hprog".
     iApply (wp_store_success_reg with "[$HPC $Hi $Hr2 $Hr3 $Hmemptr]");
-      [apply decode_encode_instrW_inv|done|done| |iContiguous_next Hcont 15|split;try done|auto|..].
+      [apply decode_encode_instrW_inv| |iContiguous_next Hcont 15|split;try done|auto|..].
     { apply HPC; repeat constructor. }
     { apply le_addr_withinBounds.
       - generalize (contiguous_between_length _ _ _ Hcont). cbn.
@@ -331,34 +325,34 @@ Section SimpleMalloc.
     destruct l as [|? l];[inversion Hprog_len|].
     iPrologue "Hprog".
     iApply (wp_move_success_reg with "[$HPC $Hi $Hr1 $Hr4]");
-      [apply decode_encode_instrW_inv|done| |iContiguous_next Hcont 16|done|..].
+      [apply decode_encode_instrW_inv| |iContiguous_next Hcont 16|..].
     { apply HPC; repeat constructor. }
     iEpilogue "(HPC & Hi & Hr1 & Hr4)". iCombine "Hi" "Hprog_done" as "Hprog_done".
     (* move r_t2 0 *)
     destruct l as [|? l];[inversion Hprog_len|].
     iPrologue "Hprog".
     iApply (wp_move_success_z with "[$HPC $Hi $Hr2]");
-      [apply decode_encode_instrW_inv|done| |iContiguous_next Hcont 17|done|..].
+      [apply decode_encode_instrW_inv| |iContiguous_next Hcont 17|..].
     { apply HPC; repeat constructor. }
     iEpilogue "(HPC & Hi & Hr2)". iCombine "Hi" "Hprog_done" as "Hprog_done".
     (* move r_t3 0 *)
     destruct l as [|? l];[inversion Hprog_len|].
     iPrologue "Hprog".
     iApply (wp_move_success_z with "[$HPC $Hi $Hr3]");
-      [apply decode_encode_instrW_inv|done| |iContiguous_next Hcont 18|done|..].
+      [apply decode_encode_instrW_inv| |iContiguous_next Hcont 18|..].
     { apply HPC; repeat constructor. }
     iEpilogue "(HPC & Hi & Hr3)". iCombine "Hi" "Hprog_done" as "Hprog_done".
     (* move r_t4 0 *)
     destruct l as [|? l];[inversion Hprog_len|].
     iPrologue "Hprog".
     iApply (wp_move_success_z with "[$HPC $Hi $Hr4]");
-      [apply decode_encode_instrW_inv|done| |iContiguous_next Hcont 19|done|..].
+      [apply decode_encode_instrW_inv| |iContiguous_next Hcont 19|..].
     { apply HPC; repeat constructor. }
     iEpilogue "(HPC & Hi & Hr4)". iCombine "Hi" "Hprog_done" as "Hprog_done".
     (* jmp r_t0 *)
     iPrologue "Hprog".
     iApply (wp_jmp_success with "[$HPC $Hi $Hr0]");
-      [apply decode_encode_instrW_inv|done| |..].
+      [apply decode_encode_instrW_inv|..].
     { apply HPC; repeat constructor. }
     iEpilogue "(HPC & Hi & Hr0)". iCombine "Hi" "Hprog_done" as "Hprog_done".
     (* continuation *)
@@ -374,7 +368,7 @@ Section SimpleMalloc.
     { iNext. iExists b_m, a_m'. iFrame.
       rewrite /malloc_subroutine_instrs /malloc_subroutine_instrs'.
       unfold region_mapsto. rewrite Hai. cbn.
-      repeat iDestruct "Hprog_done" as "[? Hprog_done]". iFrame.
+      do 20 iDestruct "Hprog_done" as "[? Hprog_done]". iFrame.
       iPureIntro.
       unfold isWithin in Ha_m'_within. (* FIXME? *)
       rewrite andb_true_iff !Z.leb_le in Ha_m'_within |- *.
